### Ontology file generated from ML_Ontology.xlsx.
### 2024-05-21 19:10:55.380753


# PREFIXES

@prefix : <http://h-da.de/ml-ontology/> .
@prefix rdf: <http://www.w3.org/1999/02/22-rdf-syntax-ns#> .
@prefix rdfs: <http://www.w3.org/2000/01/rdf-schema#> .
@prefix xsd: <http://www.w3.org/2001/XMLSchema#> .
@prefix skos: <http://www.w3.org/2004/02/skos/core#> .
@prefix sp: <http://spinrdf.org/sp#> .


# rdfsClass

:ML_area a rdfs:Class ;
    skos:prefLabel "ML area" ;
    rdfs:comment "Broad category of ML, depending on the nature of the feedback available to the learning system; e.g., feedback by supervisor (supervised learning), without feedback (unsupervised learning), feedback by software application (reinforcement learning)." .
:ML_task a rdfs:Class ;
    skos:prefLabel "ML task" ;
    rdfs:comment "Problem that is to be solved by ML, e.g., assign categories to data records (classification), predict numeric values (regression), group data records (clustering), etc." .
:ML_approach a rdfs:Class ;
    skos:prefLabel "ML approach" ;
    rdfs:comment "A set of technologies suitable for solving ML tasks, e.g., artificial neural networks (including gradient descent, backpropagation, etc.)" .
:Preprocessing_approach a rdfs:Class ;
    skos:prefLabel "Preprocessing approach" ;
    rdfs:comment "A set of technologies suited for preprossing ML datasets" .
:Metric a rdfs:Class ;
    skos:prefLabel "Metric" ;
    rdfs:comment "Metric for assessing the prediction quality of a ML system based on a dataset, e.g., for classification tasks measures on values in a confusion matrix like accuracy, F1 score etc." .
:ML_library a rdfs:Class ;
    skos:prefLabel "ML library" ;
    rdfs:comment "Examples: scikit-learn, Tensorflow, Keras" .
:AutoML_solution a rdfs:Class ;
    skos:prefLabel "AutoML solution" ;
    rdfs:comment "Examples: Autosklearn for Scikit-learn, Auto-Keras for Keras, and Google AutoML for Tensorﬂow" .
:Configuration_item a rdfs:Class ;
    skos:prefLabel "Configuration item" ;
    rdfs:comment "Example configuration items for AutoML solutions: metric, time limit, memory limit etc." .
:Enum a rdfs:Class ;
    skos:prefLabel "Enum" ;
    rdfs:comment "Enumeration values for different categories" .


# rdfProperty

:automl_solution a rdf:Property ;
    skos:prefLabel "AutoML solution" ;
    rdfs:comment "Denotes which AutoML solution a configuration item belongs to. Domain / range: :Configuration_item -> :AutoML_solution" .
:belongs_to a rdf:Property ;
    skos:prefLabel "belongs to" ;
    :inheritance :broader_inherited ;
    rdfs:comment "Denotes which ML area an ML task or an ML approach belongs to. Domain / range: { :ML_task, ML_approach} -> :ML_area" .
:can_perform a rdf:Property ;
    skos:prefLabel "can perform" ;
    rdfs:comment "Denotes which ML task an AutoML solution is able to perform. Domain / range: :AutoML_solution -> :ML_task" .
:category a rdf:Property ;
    skos:prefLabel "category" ;
    rdfs:comment "Categorizes entities via enums. Domain / range: {:Configuration_item, :Enum} -> :Enum" .
:has_dataset_type a rdf:Property ;
    skos:prefLabel "has dataset type" ;
    rdfs:comment "Assigns a dataset type to an ML task. Domain / range: :ML_task -> :Enum" .
:has_datatype a rdf:Property ;
    skos:prefLabel "has datatype" ;
    rdfs:comment "Assigns a datatype to a parameter configuration. Domain / range: :Configuration_item -> :Enum" .
:inheritance a rdf:Property ;
    skos:prefLabel "inheritance" ;
    rdfs:comment "Specifies inheritance behaviour for a property which may be used for SPARQL inferencing. Domain / range: rdf:Property -> :Enum(:inheritance_type)" .
:ml_task a rdf:Property ;
    skos:prefLabel "ML task" ;
    rdfs:comment "Assigns the ML task to a task configuration. Domain / range: :configuration_item -> :ML_task" .
:not_possible_if a rdf:Property ;
    skos:prefLabel "not possible if" ;
    :inheritance :broader_inherited ;
    rdfs:comment "Specifies a situation under which an approach must not be used. Domain / range: {:ML_approach; :Preprocessing_approach} -> :Enum" .
:not_recommended_if a rdf:Property ;
    skos:prefLabel "not recommended if" ;
    :inheritance :broader_inherited ;
    rdfs:comment "Specifies a situation under which an approach should not be used. {:ML_approach; :Metric} -> :Enum" .
:parameter_value a rdf:Property ;
    skos:prefLabel "parameter value" ;
    rdfs:comment "Specifies parameter values. Domain / range: :Configuration_item -> {:Configuraiton_item; :Enum; :ML_approach; :Metric; :Proprocessing_approach}" .
:performance a rdf:Property ;
    skos:prefLabel "performance" ;
    :inheritance :broader_inherited ;
    rdfs:comment "Specifies performance characteristics of approaches regarding runtime and prediction performance. Domain / range: {:ML_approach; :Preprocessing_approach} -> :Enum" .
:possible_if a rdf:Property ;
    skos:prefLabel "possible if" ;
    :inheritance :broader_inherited ;
    rdfs:comment "Specifies a situation under which an approach may be used. Domain / range: {:ML_approach; :Preprocessing_approach} -> :Enum" .
:recommended_if a rdf:Property ;
    skos:prefLabel "recommended if" ;
    :inheritance :broader_inherited ;
    rdfs:comment "Specifies a situation under which an approach should be used. Domain / range: :Metric -> :Enum" .
:required a rdf:Property ;
    skos:prefLabel "required" ;
    rdfs:comment "Specifies whether a parameter is required or not. Domain / range: :Configuration_item -> boolean" .
:supported_by_oma_ml a rdf:Property ;
    skos:prefLabel "supported by OMA-ML" ;
    rdfs:comment "Marker specific for the OMA-ML platform. Domain / range: :AutoML_solution -> boolean" .
:used_for a rdf:Property ;
    skos:prefLabel "used for" ;
    :inheritance :broader_inherited ;
    rdfs:comment "Specifies which approaches may be used for which tasks or systems. Domain / range: {:ML_approach, :Metric, :Preprocessing_approach} -> :ML_task; :AutoML_solution -> :ML_library" .


# ML_area

:supervised_learning a :ML_area ;
    skos:prefLabel "supervised learning" ;
    skos:altLabel "SL" ;
    rdfs:comment "Supervised learning (SL) is the machine learning area of learning a function that maps an input to an output based on example input-output pairs." ;
    rdfs:seeAlso <https://www.wikidata.org/entity/Q334384> .
:unsupervised_learning a :ML_area ;
    skos:prefLabel "unsupervised learning" ;
    skos:altLabel "UL" ;
    rdfs:comment "Unsupervised learning (UL) is the machine learning area for learning patterns from unlabeled data." ;
    rdfs:seeAlso <https://www.wikidata.org/entity/Q1152135> .
:reinforcement_learning a :ML_area ;
    skos:prefLabel "reinforcement learning" ;
    skos:altLabel "RL" ;
    rdfs:comment "Reinforcement learning (RL) is an area of machine learning concerned with how intelligent agents ought to take actions in an environment in order to maximize the notion of cumulative reward." ;
    rdfs:seeAlso <https://www.wikidata.org/entity/Q830687> .


# ML_task

:action_recognition a :ML_task ;
    skos:prefLabel "action recognition" ;
    skos:altLabel "activity recognition" ;
    :belongs_to :supervised_learning ;
    :has_dataset_type :video ;
    rdfs:comment "Predicting the movement of a person based on sensor data, e.g. an accelerometer in a smartphone." .
:anomaly_detection a :ML_task ;
    skos:prefLabel "anomaly detection" ;
    skos:altLabel "outlier detection" ;
    :belongs_to :supervised_learning , :unsupervised_learning ;
    rdfs:comment "The identification of rare items, events or observations which raise suspicions by differing significantly from the expected or majority of the data" ;
    rdfs:seeAlso <https://www.wikidata.org/entity/Q3560506> .
:association_rule_learning a :ML_task ;
    skos:prefLabel "association rule learning" ;
    :belongs_to :supervised_learning ;
    :has_dataset_type :tabular ;
    rdfs:comment "Discovering interesting relations between variables in large databases" ;
    rdfs:seeAlso <https://www.wikidata.org/entity/Q386780> .
:audio_classification a :ML_task ;
    skos:prefLabel "audio classification" ;
    skos:broader :classification ;
    :belongs_to :supervised_learning ;
    :has_dataset_type :audio ;
    rdfs:comment "Predicting classes for audio files" .
:audio_regression a :ML_task ;
    skos:prefLabel "audio regression" ;
    skos:broader :regression ;
    :belongs_to :supervised_learning ;
    :has_dataset_type :audio ;
    rdfs:comment "Predicting numeric values for audio files" .
:binary_classification a :ML_task ;
    skos:prefLabel "binary classification" ;
    skos:broader :classification ;
    :belongs_to :supervised_learning ;
    rdfs:comment "Classifying the elements of a given set into two groups, i.e., predicting which group each one belongs to" ;
    rdfs:seeAlso <https://www.wikidata.org/entity/Q3560506> .
:classification a :ML_task ;
    skos:prefLabel "classification" ;
    :belongs_to :supervised_learning ;
    rdfs:comment "Prediction of discrete categorical values (classes)" .
:clustering a :ML_task ;
    skos:prefLabel "clustering" ;
    :belongs_to :unsupervised_learning ;
    rdfs:comment "Grouping a set of objects in such a way that objects in the same group (called a cluster) are more similar (in some sense or another) to each other than to those in other groups" ;
    rdfs:seeAlso <https://www.wikidata.org/entity/Q622825> .
:community_detection a :ML_task ;
    skos:prefLabel "community detection" ;
    :belongs_to :supervised_learning ;
    :has_dataset_type :graph ;
    rdfs:comment "Organization of vertices in clusters, with many edges joining vertices of the same cluster and comparatively few edges joining vertices of different clusters." ;
    rdfs:seeAlso <https://www.wikidata.org/entity/Q105222918> .
:feature_extraction a :ML_task ;
    skos:prefLabel "feature extraction" ;
    skos:broader :feature_reduction ;
    :belongs_to :unsupervised_learning ;
    rdfs:comment "Building informative, nonredundant derived values from an initial set of measured data to facilitate learning, generalization and interpretation" ;
    rdfs:seeAlso <https://www.wikidata.org/entity/Q1026626> .
:feature_reduction a :ML_task ;
    skos:prefLabel "feature reduction" ;
    skos:altLabel "dimension reduction" ;
    :belongs_to :unsupervised_learning ;
    rdfs:comment "Reducing the number of features in a dataset without losing important information." ;
    rdfs:seeAlso <https://www.wikidata.org/entity/Q446488> .
:feature_selection a :ML_task ;
    skos:prefLabel "feature selection" ;
    skos:altLabel "attribute selection" , "variable selection" ;
    skos:broader :feature_reduction ;
    :belongs_to :unsupervised_learning ;
    rdfs:comment "Omitting features in a dataset without losing important information." ;
    rdfs:seeAlso <https://www.wikidata.org/entity/Q446488> .
:graph_matching a :ML_task ;
    skos:prefLabel "graph matching" ;
    :belongs_to :supervised_learning ;
    :has_dataset_type :graph ;
    rdfs:comment "Finding similarity between graphs" ;
    rdfs:seeAlso <https://www.wikidata.org/entity/Q39045684> .
:image_classification a :ML_task ;
    skos:prefLabel "image classification" ;
    skos:broader :classification ;
    :belongs_to :supervised_learning ;
    :has_dataset_type :image ;
    rdfs:comment "Predicting categories (classes) for images" ;
    rdfs:seeAlso <https://www.wikidata.org/entity/Q98526763> ;
    :supported_by_oma_ml "true"^^xsd:boolean .
:image_regression a :ML_task ;
    skos:prefLabel "image regression" ;
    skos:broader :regression ;
    :belongs_to :supervised_learning ;
    :has_dataset_type :image ;
    rdfs:comment "Predicting numeric values for images" .
:image_segmentation a :ML_task ;
    skos:prefLabel "image segmentation" ;
    :belongs_to :supervised_learning , :unsupervised_learning ;
    :has_dataset_type :image ;
    rdfs:comment "Division of an image into sets of pixels for further processing" ;
    rdfs:seeAlso <https://www.wikidata.org/entity/Q56933> .
:link_prediction a :ML_task ;
    skos:prefLabel "link prediction" ;
    :belongs_to :supervised_learning ;
    :has_dataset_type :graph ;
    rdfs:comment "Predicting an unobserved link between two entities in a network" ;
    rdfs:seeAlso <https://www.wikidata.org/entity/Q98925312> .
:multiclass_classification a :ML_task ;
    skos:prefLabel "multiclass classification" ;
    skos:broader :classification ;
    :belongs_to :supervised_learning ;
    rdfs:comment "Classifying instances into one of multiple classes" ;
    rdfs:seeAlso <https://www.wikidata.org/entity/Q6934605> .
:named_entity_recognition a :ML_task ;
    skos:prefLabel "named entity recognition" ;
    skos:altLabel "NER" , "entity extraction" , "entity identification" ;
    :belongs_to :supervised_learning ;
    :has_dataset_type :text ;
    rdfs:comment "Extraction of named entity mentions in unstructured text into pre-defined categories" ;
    rdfs:seeAlso <https://www.wikidata.org/entity/Q403574> .
:object_detection a :ML_task ;
    skos:prefLabel "object detection" ;
    skos:altLabel "object tracking" , "image object tracking" , "instance segmentation" ;
    :belongs_to :supervised_learning ;
    :has_dataset_type :image ;
    rdfs:comment "Detecting and localizing an object in an image" ;
    rdfs:seeAlso <https://www.wikidata.org/entity/Q3045304> .
:ranking a :ML_task ;
    skos:prefLabel "ranking" ;
    :belongs_to :supervised_learning ;
    :has_dataset_type :tabular ;
    rdfs:comment "Ordering items in a set by criteria" ;
    rdfs:seeAlso <https://www.wikidata.org/entity/Q526719> .
:recommendation a :ML_task ;
    skos:prefLabel "recommendation" ;
    :belongs_to :supervised_learning , :unsupervised_learning ;
    rdfs:comment "Predicting users' preferences" ;
    rdfs:seeAlso <https://www.wikidata.org/entity/Q554950> .
:regression a :ML_task ;
    skos:prefLabel "regression" ;
    :belongs_to :supervised_learning ;
    rdfs:comment "Predicting continuous numerical values" ;
    rdfs:seeAlso <https://www.wikidata.org/entity/Q208042> .
:sentence_similarity a :ML_task ;
    skos:prefLabel "sentence similarity" ;
    :belongs_to :supervised_learning ;
    :has_dataset_type :text ;
    rdfs:comment "Predicting the semantic similarity between two sentences" .
:sentiment_analysis a :ML_task ;
    skos:prefLabel "sentiment analysis" ;
    :belongs_to :supervised_learning ;
    :has_dataset_type :text ;
    rdfs:comment "Identifying and extracting subjective information in texts, e.g., mood" ;
    rdfs:seeAlso <https://www.wikidata.org/entity/Q2271421> .
:tabular_classification a :ML_task ;
    skos:prefLabel "tabular classification" ;
    skos:broader :classification ;
    :belongs_to :supervised_learning ;
    :has_dataset_type :tabular ;
    rdfs:comment "Predicting categories (classes) for rows of a data table" ;
    :supported_by_oma_ml "true"^^xsd:boolean .
:tabular_regression a :ML_task ;
    skos:prefLabel "tabular regression" ;
    skos:broader :regression ;
    :belongs_to :supervised_learning ;
    :has_dataset_type :tabular ;
    rdfs:comment "Predicting numeric values for rows of a data table" ;
    :supported_by_oma_ml "true"^^xsd:boolean .
:tabular_clustering a :ML_task ;
    skos:prefLabel "tabular clustering" ;
    skos:broader :clustering ;
    :belongs_to :unsupervised_learning ;
    :has_dataset_type :tabular ;
    rdfs:comment "Grouping a set of objects in such a way that objects in the same group (called a cluster) are more similar (in some sense or another) to each other than to those in other groups" ;
    :supported_by_oma_ml "true"^^xsd:boolean .
:text_analytics a :ML_task ;
    skos:prefLabel "text analytics" ;
    :belongs_to :supervised_learning , :unsupervised_learning ;
    :has_dataset_type :text ;
    rdfs:comment "Changing text documents that are unstructured  into structured data" .
:text_classification a :ML_task ;
    skos:prefLabel "text classification" ;
    skos:broader :classification ;
    :belongs_to :supervised_learning ;
    :has_dataset_type :text ;
    rdfs:comment "Predicting categories (classes) for texts" ;
    rdfs:seeAlso <https://www.wikidata.org/entity/Q102190569> ;
    :supported_by_oma_ml "true"^^xsd:boolean .
:text_regression a :ML_task ;
    skos:prefLabel "text regression" ;
    skos:broader :regression ;
    :belongs_to :supervised_learning ;
    :has_dataset_type :text ;
    rdfs:comment "Predicting numeric values for texts" .
:time_series_analysis a :ML_task ;
    skos:prefLabel "time series analysis" ;
    :belongs_to :supervised_learning ;
    :has_dataset_type :tabular ;
    rdfs:comment "Analyzing series of data points in time order" ;
    rdfs:seeAlso <https://www.wikidata.org/entity/Q11850042> .
:time_series_classification a :ML_task ;
    skos:prefLabel "time series classification" ;
    skos:broader :classification ;
    :belongs_to :supervised_learning ;
    :has_dataset_type :time_series_longitudinal ;
    rdfs:comment "Predicting categories (classes) for time series" ;
    :supported_by_oma_ml "true"^^xsd:boolean .
:time_series_forecasting a :ML_task ;
    skos:prefLabel "time series forecasting" ;
    :belongs_to :supervised_learning ;
    :has_dataset_type :time_series ;
    rdfs:comment "Predicting future events from past events" ;
    :supported_by_oma_ml "true"^^xsd:boolean .
:topic_modeling a :ML_task ;
    skos:prefLabel "topic modeling" ;
    skos:altLabel "topic modelling" ;
    :belongs_to :unsupervised_learning ;
    rdfs:comment "Finding abstract topics that occur in several texts and classify documents accordingly" ;
    rdfs:seeAlso <https://www.wikidata.org/entity/Q96468792> .
:translation a :ML_task ;
    skos:prefLabel "translation" ;
    skos:altLabel "machine translation" ;
    :belongs_to :supervised_learning ;
    :has_dataset_type :text ;
    rdfs:comment "Translating a text in one natural language, e.g., English into another, e.g., Spanish" ;
    rdfs:seeAlso <https://www.wikidata.org/entity/Q79798> .
:vertex_classification a :ML_task ;
    skos:prefLabel "vertex classification" ;
    skos:broader :classification ;
    :belongs_to :supervised_learning ;
    :has_dataset_type :graph ;
    rdfs:comment "Mapping a system of vertices, for which it is then classified and counts the types for vertices" .
:video_classification a :ML_task ;
    skos:prefLabel "video classification" ;
    skos:broader :classification ;
    :belongs_to :supervised_learning ;
    :has_dataset_type :video ;
    rdfs:comment "Predicting categories (classes) for videos" .
:video_object_tracking a :ML_task ;
    skos:prefLabel "video object tracking" ;
    :belongs_to :supervised_learning ;
    :has_dataset_type :video ;
    rdfs:comment "Tracking a moving object over a period of time" .
:video_regression a :ML_task ;
    skos:prefLabel "video regression" ;
    skos:broader :regression ;
    :belongs_to :supervised_learning ;
    :has_dataset_type :video ;
    rdfs:comment "Predicting numeric values for videos" .


# ML_approach

:adaboost a :ML_approach ;
    skos:prefLabel "adaboost" ;
    :used_for :classification , :regression ;
    rdfs:comment "AdaBoost, short for Adaptive Boosting, is a statistical classification meta-algorithm" ;
    rdfs:seeAlso <https://www.wikidata.org/entity/Q2823869> .
:affinity_propagation a :ML_approach ;
    skos:prefLabel "affinity propagation" ;
    :used_for :clustering ;
    rdfs:comment "Exemplar clustering Algorithm" ;
    rdfs:seeAlso <https://www.wikidata.org/wiki/Q3407504> .
:agglomerative_clustering a :ML_approach ;
    skos:prefLabel "agglomerative clustering" ;
    skos:broader :hierarchical_clustering ;
    :used_for :clustering ;
    rdfs:comment "A bottom up clustering method where clusters have subclusters, where these subclusters can also have subclusters" .
:arsenal_ensemble a :ML_approach ;
    skos:prefLabel "Arsenal ensemble" ;
    skos:altLabel "Arsenal" ;
    skos:broader :ensemble ;
    :used_for :time_series_classification .
:artificial_neural_network a :ML_approach ;
    skos:prefLabel "artificial neural network" ;
    skos:altLabel "ANN" , "neural network" ;
    :used_for :classification , :regression , :anomaly_detection , :time_series_classification ;
    :possible_if :numerical_features ;
    :performance :long_training_time , :accurate ;
    rdfs:comment "Computational model used in machine learning, based on connected, hierarchical functions" ;
    rdfs:seeAlso <https://www.wikidata.org/entity/Q192776> .
:autoencoder a :ML_approach ;
    skos:prefLabel "autoencoder" ;
    skos:altLabel "AE" ;
    skos:broader :artificial_neural_network ;
    :used_for :anomaly_detection ;
    rdfs:comment "Neural network that learns efficient data encoding in an unsupervised manner" ;
    rdfs:seeAlso <https://www.wikidata.org/entity/Q786435> .
:autoregressive_integrated_moving_average a :ML_approach ;
    skos:prefLabel "autoregressive integrated moving average" ;
    skos:altLabel "ARIMA" ;
    :used_for :time_series_analysis ;
    rdfs:comment "Statistical model used in time series analysis" ;
    rdfs:seeAlso <https://www.wikidata.org/entity/Q2566298> .
:bag_of_sfa_symbols a :ML_approach ;
    skos:prefLabel "Bag-of-SFA-Symbols" ;
    skos:altLabel "BOSS" ;
    skos:broader :ensemble ;
    :used_for :time_series_classification ;
    rdfs:comment "Ensemble of bag of Symbolic Fourier Approximation Symbols" .
:bayesian_linear_regression a :ML_approach ;
    skos:prefLabel "Bayesian linear regression" ;
    skos:broader :linear_regression ;
    :used_for :regression ;
    :possible_if :small_dataset ;
    rdfs:comment "Approach to linear regression in which the statistical analysis is undertaken within the context of Bayesian inference" ;
    rdfs:seeAlso <https://www.wikidata.org/entity/Q4874474> .
:bayesian_neural_network a :ML_approach ;
    skos:prefLabel "Bayesian neural network" ;
    skos:broader :artificial_neural_network ;
    :possible_if :numerical_features ;
    rdfs:comment "Probability model which is factored by applying a single conditional probability distribution for each variable for the given model" .
:bernoulli_naive_bayes a :ML_approach ;
    skos:prefLabel "Bernoulli naive bayes" ;
    :used_for :classification ;
    rdfs:comment "Naive Bayes classifier for multivariate Bernoulli models." .
:balanced_iterative_reducing_and_clustering_using_hierarchies a :ML_approach ;
    skos:prefLabel "balanced iterative reducing and clustering using hierarchies" ;
    skos:altLabel "BIRCH" ;
    skos:broader :hierarchical_clustering ;
    :used_for :clustering ;
    rdfs:comment "An efficient hierarchical clustering method optimized for large datasets, which builds a clustering feature tree incrementally" ;
    rdfs:seeAlso <https://www.wikidata.org/entity/Q4835721> .
:boltzman_machine a :ML_approach ;
    skos:prefLabel "Boltzman machine" ;
    skos:broader :artificial_neural_network ;
    rdfs:comment "A type of stochastic recurrent neural network" .
:boosted_decision_tree a :ML_approach ;
    skos:prefLabel "boosted decision tree" ;
    skos:broader :decision_tree ;
    :performance :large_memory_footprint ;
    rdfs:comment "An ensemble learning method where the current tree's errors will  be corrected by the next tree and the next tree's errors will be corrected by the tree after, and so on" .
:c_means a :ML_approach ;
    skos:prefLabel "c-means" ;
    :used_for :clustering , :anomaly_detection ;
    rdfs:comment "Soft clustering where each data point is assigned a probability score to belong to that cluster" .
:canonical_correlation_analysis a :ML_approach ;
    skos:prefLabel "canonical correlation analysis" ;
    skos:altLabel "CCA" ;
    :used_for :feature_reduction ;
    :possible_if :numerical_features ;
    rdfs:comment "Way of inferring information from cross-covariance matrices" ;
    rdfs:seeAlso <https://www.wikidata.org/entity/Q115542> .
:canonical_interval_forest a :ML_approach ;
    skos:prefLabel "Canonical Interval Forest" ;
    skos:altLabel "CIF" ;
    :used_for :time_series_classification ;
    rdfs:comment "Canonical Interval Forest Classifier" .
:canonical_time_series_characteristics a :ML_approach ;
    skos:prefLabel "Canonical Time-series Characteristics" ;
    skos:altLabel "catch22" ;
    :used_for :time_series_classification ;
    rdfs:comment "Canonical Time-series Characteristics (catch22) classifier" .
:catboost a :ML_approach ;
    skos:prefLabel "catboost" ;
    skos:broader :gradient_boosting_tree ;
    :used_for :classification , :regression ;
    :performance :accurate , :explainable ;
    rdfs:comment "Yandex open source gradient boosting framework on decision trees" ;
    rdfs:seeAlso <https://www.wikidata.org/entity/Q104853624> .
:collaborative_filtering a :ML_approach ;
    skos:prefLabel "collaborative filtering" ;
    :used_for :recommendation ;
    rdfs:comment "Algorithms to filter data from user reviews to make personalized recommendations for users with similar preferences" ;
    rdfs:seeAlso <https://www.wikidata.org/entity/Q94702> .
:conceptual_clustering a :ML_approach ;
    skos:prefLabel "conceptual clustering" ;
    :used_for :clustering ;
    rdfs:comment "Machine learning approach for unsupervised classification" ;
    rdfs:seeAlso <https://www.wikidata.org/entity/Q5158434> .
:conditional_markov_model a :ML_approach ;
    skos:prefLabel "conditional markov model" ;
    skos:broader :markov_model ;
    rdfs:comment "A model that has two phases, structural phase and statistical phase" .
:conditional_random_field a :ML_approach ;
    skos:prefLabel "conditional random field" ;
    skos:altLabel "CRF" ;
    :used_for :time_series_analysis ;
    rdfs:comment "Class of statistical modeling method applied in pattern recognition and machine learning and used for structured prediction" ;
    rdfs:seeAlso <https://www.wikidata.org/entity/Q1124538> .
:contractable_boss a :ML_approach ;
    skos:prefLabel "Contractable BOSS" ;
    skos:altLabel "cBOSS" ;
    skos:broader :ensemble ;
    :used_for :time_series_classification ;
    rdfs:comment "Contractable Bag of Symbolic Fourier Approximation Symbols" .
:convolutional_neural_network a :ML_approach ;
    skos:prefLabel "convolutional neural network" ;
    skos:altLabel "CNN" ;
    skos:broader :artificial_neural_network ;
    :used_for :image_classification , :time_series_classification ;
    rdfs:comment "A class of deep neural networks, most commonly applied to analyzing images" ;
    rdfs:seeAlso <https://www.wikidata.org/entity/Q17084460> .
:decision_tree a :ML_approach ;
    skos:prefLabel "decision tree" ;
    :used_for :classification , :regression ;
    :performance :fast_training , :explainable ;
    rdfs:comment "Decision support tool that uses a tree-like model of decisions and their possible consequences, including chance event outcomes, resource costs, and utility" ;
    rdfs:seeAlso <https://www.wikidata.org/entity/Q831366> .
:deep_convolutional_lstm a :ML_approach ;
    skos:prefLabel "Deep Convolutional LSTM" ;
    skos:altLabel "DeepConvLSTM" ;
    skos:broader :artificial_neural_network ;
    :used_for :time_series_classification .
:density_based_clustering a :ML_approach ;
    skos:prefLabel "density-based clustering" ;
    :used_for :clustering ;
    rdfs:comment "Algorithm that finds non linear shapes structure based on their density" ;
    rdfs:seeAlso <https://www.wikidata.org/entity/Q56388089> .
:density_based_spatial_clustering_of_applications_with_noise a :ML_approach ;
    skos:prefLabel "density-based spatial clustering of applications with noise" ;
    skos:altLabel "DBSCAN" ;
    skos:broader :density_based_clustering ;
    :used_for :clustering ;
    rdfs:comment "Density-based clustering algorithm" ;
    rdfs:seeAlso <https://www.wikidata.org/entity/Q1114630> .
:diverse_representation_canonical_interval_forest a :ML_approach ;
    skos:prefLabel "Diverse Representation Canonical Interval Forest" ;
    skos:altLabel "DrCIF" ;
    :used_for :time_series_classification ;
    rdfs:comment "Diverse Representation Canonical Interval Forest Classifier (DrCIF)." .
:elastic_ensemble a :ML_approach ;
    skos:prefLabel "Elastic Ensemble" ;
    skos:altLabel "EE" ;
    skos:broader :ensemble ;
    :used_for :time_series_classification ;
    :performance :long_training_time ;
    rdfs:comment "Ensemble of elastic nearest neighbor classifiers" .
:ensemble skos:prefLabel "ensemble" ;
    :used_for :tabular_classification , :tabular_regression ;
    rdfs:comment "Combining various machine learning approaches using a voting mechanism" .
:expectation_maximization_clustering a :ML_approach ;
    skos:prefLabel "expectation maximization clustering" ;
    :used_for :clustering ;
    rdfs:comment "Iterative method for finding maximum likelihood estimates in statistical models" ;
    rdfs:seeAlso <https://www.wikidata.org/entity/Q1275153> .
:exponential_smoothing a :ML_approach ;
    skos:prefLabel "exponential smoothing" ;
    rdfs:comment "A rule of thumb technique for smoothing time series data using the exponential window function" .
:extra_tree a :ML_approach ;
    skos:prefLabel "extra tree" ;
    skos:broader :decision_tree ;
    :used_for :classification , :regression ;
    rdfs:comment "Ensemble learning technique which aggregates the results of multiple de-correlated decision trees collected in a forest to output it’s classification result" .
:feed_forward_neural_network a :ML_approach ;
    skos:prefLabel "feed-forward neural network" ;
    skos:altLabel "FFN" ;
    skos:broader :artificial_neural_network ;
    rdfs:comment "Artificial neural network wherein connections between the nodes do not form a cycle" ;
    rdfs:seeAlso <https://www.wikidata.org/entity/Q5441227> .
:fresh_prince a :ML_approach ;
    skos:prefLabel "Fresh PRINCE" ;
    :used_for :time_series_classification ;
    rdfs:comment "Fresh Pipeline with RotatIoN forest Classifier." .
:gated_recurrent_unit a :ML_approach ;
    skos:prefLabel "gated recurrent unit" ;
    skos:altLabel "GRU" ;
    skos:broader :artificial_neural_network ;
    rdfs:comment "Mechanisms in recurrent neural networks" ;
    rdfs:seeAlso <https://www.wikidata.org/entity/Q25325415> .
:gaussian_mixture_model a :ML_approach ;
    skos:prefLabel "Gaussian mixture model" ;
    skos:altLabel "GMM" ;
    :used_for :clustering ;
    rdfs:comment "A model that is a mixture of several Gaussian distributions" .
:gaussian_naives_bayes a :ML_approach ;
    skos:prefLabel "Gaussian naives bayes" ;
    skos:altLabel "GNB" ;
    rdfs:comment "Probabilistic machine learning algorithm used for many classification functions that is based on the Bayes theorem" .
:gaussian_process a :ML_approach ;
    skos:prefLabel "Gaussian process" ;
    skos:altLabel "GP" ;
    :used_for :classification , :regression ;
    :not_recommended_if :many_features ;
    rdfs:comment "Statistical model where observations occur in a continuous domain, e.g. time or space. In a Gaussian process, every point in some continuous input space is associated with a normally distributed random variable" ;
    rdfs:seeAlso <https://www.wikidata.org/entity/Q1496376> .
:generalized_linear_model a :ML_approach ;
    skos:prefLabel "generalized linear model" ;
    skos:altLabel "GLM" ;
    :used_for :classification ;
    rdfs:comment "Flexible generalization of ordinary linear regression" ;
    rdfs:seeAlso <https://www.wikidata.org/entity/Q1501882> .
:generative_adversarial_network a :ML_approach ;
    skos:prefLabel "generative adversarial network" ;
    skos:altLabel "GAN" ;
    skos:broader :artificial_neural_network ;
    rdfs:comment "Deep learning method in which two neural networks compete with each other in a game, learning to generate new data with the same statistics as the training set" ;
    rdfs:seeAlso <https://www.wikidata.org/entity/Q25104379> .
:gradient_boosting_tree a :ML_approach ;
    skos:prefLabel "gradient boosting tree" ;
    skos:broader :boosted_decision_tree ;
    :used_for :classification , :regression , :ranking ;
    :performance :accurate , :explainable ;
    rdfs:comment "Ensemble of weak predictors, which are often decision trees" .
:hidden_markov_model a :ML_approach ;
    skos:prefLabel "hidden markov model" ;
    skos:altLabel "HMM" ;
    skos:broader :markov_model ;
    :used_for :time_series_analysis , :anomaly_detection ;
    rdfs:comment "Statistical Markov model" ;
    rdfs:seeAlso <https://www.wikidata.org/entity/Q176769> .
:hierachical_dbscan a :ML_approach ;
    skos:prefLabel "hierachical dbscan" ;
    skos:altLabel "HDBSCAN" ;
    skos:broader :density_based_spatial_clustering_of_applications_with_noise ;
    :used_for :clustering ;
    rdfs:comment "Data clustering algorithm" ;
    rdfs:seeAlso <https://www.wikidata.org/entity/Q1114630> .
:hierarchical_clustering a :ML_approach ;
    skos:prefLabel "hierarchical clustering" ;
    :used_for :clustering ;
    rdfs:comment "Method of cluster analysis which seeks to build a hierarchy of clusters" ;
    rdfs:seeAlso <https://www.wikidata.org/entity/Q1277447> .
:hierarchical_vote_collective_of_transformation_based_ensembles_v1 a :ML_approach ;
    skos:prefLabel "Hierarchical Vote Collective of Transformation-based Ensembles V1" ;
    skos:altLabel "HIVE-COTE V1" ;
    skos:broader :ensemble ;
    :used_for :time_series_classification ;
    :performance :long_training_time , :accurate ;
    rdfs:comment "Hierarchical Vote Collective of Transformation-based Ensembles (HIVE-COTE) V1" .
:hierarchical_vote_collective_of_transformation_based_ensembles_v2 a :ML_approach ;
    skos:prefLabel "Hierarchical Vote Collective of Transformation-based Ensembles V2" ;
    skos:altLabel "HIVE-COTE V2" ;
    skos:broader :ensemble ;
    :used_for :time_series_classification ;
    :performance :long_training_time , :accurate ;
    rdfs:comment "Hierarchical Vote Collective of Transformation-based Ensembles (HIVE-COTE) V2" .
:inception_fully_convolutional_network a :ML_approach ;
    skos:prefLabel "Inception Fully Convolutional Network" ;
    skos:altLabel "InceptionFCN" ;
    skos:broader :artificial_neural_network ;
    :used_for :time_series_classification .
:inception_time a :ML_approach ;
    skos:prefLabel "Inception Time" ;
    skos:altLabel "InceptionTime" ;
    skos:broader :artificial_neural_network ;
    :used_for :time_series_classification ;
    :performance :scalable ;
    rdfs:comment "Ensemble of deep Convolutional Neural Network (CNN) models, inspired by the Inception-v4 architecture" .
:independent_component_analysis a :ML_approach ;
    skos:prefLabel "independent component analysis" ;
    skos:altLabel "ICA" ;
    :used_for :feature_reduction ;
    :possible_if :numerical_features ;
    rdfs:comment "Method for separating a multivariate signal into additive subcomponents" ;
    rdfs:seeAlso <https://www.wikidata.org/entity/Q1259145> .
:individual_boss a :ML_approach ;
    skos:prefLabel "Individual BOSS" ;
    skos:altLabel "IndividualBOSS" ;
    skos:broader :ensemble ;
    :used_for :time_series_classification ;
    rdfs:comment "Single bag of Symbolic Fourier Approximation Symbols" .
:individual_temporal_dictionary_ensemble a :ML_approach ;
    skos:prefLabel "Individual Temporal Dictionary Ensemble" ;
    skos:altLabel "IndividualTDE" ;
    skos:broader :ensemble ;
    :used_for :time_series_classification ;
    rdfs:comment "Single TDE classifier, an extension of the Bag of SFA Symbols (BOSS) model." .
:k_means a :ML_approach ;
    skos:prefLabel "k-means" ;
    :used_for :clustering ;
    :possible_if :numerical_features ;
    rdfs:comment "Vector quantization method that partitions n observations into k clusters in which each observation belongs to the cluster with the nearest mean, serving as a prototype of the cluster" ;
    rdfs:seeAlso <https://www.wikidata.org/entity/Q310401> .
:k_modes a :ML_approach ;
    skos:prefLabel "k-modes" ;
    skos:broader :k_means ;
    :used_for :clustering ;
    :possible_if :categorical_features , :text_features ;
    rdfs:comment "Using dissimilarities, quantification of the total mismatches between two objects" .
:k_nearest_neighbor a :ML_approach ;
    skos:prefLabel "k-nearest neighbor" ;
    skos:altLabel "kNN" ;
    :used_for :classification , :regression ;
    :performance :fast_training ;
    rdfs:comment "Simple algorithm for classification and regression" ;
    rdfs:seeAlso <https://www.wikidata.org/entity/Q1071612> .
:kernel_ridge_regression a :ML_approach ;
    skos:prefLabel "Kernel ridge regression" ;
    skos:broader :ridge_regression ;
    :used_for :regression .
:kernel_svm a :ML_approach ;
    skos:prefLabel "kernel svm" ;
    skos:broader :support_vector_machine ;
    :performance :accurate ;
    rdfs:comment "Set of mathematical functions that are defined as the kernel" .
:kohonen_network a :ML_approach ;
    skos:prefLabel "Kohonen network" ;
    skos:broader :artificial_neural_network ;
    rdfs:comment "Type of artificial neural network" ;
    rdfs:seeAlso <https://www.wikidata.org/entity/Q1136838> .
:lasso_regression a :ML_approach ;
    skos:prefLabel "Lasso regression" ;
    skos:broader :linear_regression ;
    :used_for :classification , :regression ;
    rdfs:comment "Regularization algorithm that assists in the elimination of irrelevant parameters, thus helping in the concentration of selection and regularizes the models" .
:latent_dirichlet_allocation a :ML_approach ;
    skos:prefLabel "latent dirichlet allocation" ;
    skos:altLabel "LDA" ;
    :used_for :feature_reduction , :topic_modeling ;
    rdfs:comment "generative statistical model that allows sets of observations to be explained by unobserved groups that explain why some parts of the data are similar" ;
    rdfs:seeAlso <https://www.wikidata.org/entity/Q269236> .
:light_gradient_boosting_machine a :ML_approach ;
    skos:prefLabel "light gradient boosting machine" ;
    skos:altLabel "LGBM" ;
    skos:broader :gradient_boosting_tree ;
    :used_for :classification , :regression ;
    :performance :accurate , :explainable ;
    rdfs:comment "Open-source distributed gradient-boosting framework for machine learning" ;
    rdfs:seeAlso <https://www.wikidata.org/entity/Q57267665> .
:linear_discriminant_analysis a :ML_approach ;
    skos:prefLabel "Linear Discriminant Analysis" ;
    :used_for :classification ;
    rdfs:comment "Method for  finding a linear combination of features that characterizes or separates two or more classes of objects" ;
    rdfs:seeAlso <https://www.wikidata.org/entity/Q1228929> .
:linear_regression a :ML_approach ;
    skos:prefLabel "linear regression" ;
    :used_for :regression ;
    :performance :fast_training ;
    rdfs:comment "Statistical approach for modeling the relationship between a scalar dependent variable and one or more explanatory variables" ;
    rdfs:seeAlso <https://www.wikidata.org/entity/Q10861030> .
:linear_svc a :ML_approach ;
    skos:prefLabel "linear SVC" ;
    skos:broader :support_vector_machine ;
    :used_for :classification ;
    rdfs:comment "Similar to SVC with parameter kernel=’linear’, but implemented in terms of liblinear rather than libsvm, so it has more flexibility in the choice of penalties and loss functions and should scale better to large numbers of samples" .
:linear_svm a :ML_approach ;
    skos:prefLabel "linear SVM" ;
    skos:broader :support_vector_machine ;
    :not_recommended_if :large_dataset ;
    :performance :fast_training ;
    rdfs:comment "A linearly scalable routine that creates an SVM model which scales linearly with the size of the training data set" .
:local_linear_embedding a :ML_approach ;
    skos:prefLabel "local linear embedding" ;
    skos:altLabel "LLE" ;
    :used_for :feature_reduction ;
    rdfs:comment "Unsupervised method for non-linear dimensionality reduction that can discover non-linear structures in the data set, and also preserve the distances within local neighborhoods" .
:logistic_regression a :ML_approach ;
    skos:prefLabel "logistic regression" ;
    :used_for :classification , :regression , :ranking ;
    :performance :fast_training ;
    rdfs:comment "Estimating the parameters of a logistic model, i.e., the coefficients in the linear combination" ;
    rdfs:seeAlso <https://www.wikidata.org/entity/Q1132755> .
:long_short_term_memory a :ML_approach ;
    skos:prefLabel "long short term memory" ;
    skos:altLabel "LSTM" ;
    skos:broader :artificial_neural_network ;
    :used_for :time_series_analysis ;
    rdfs:comment "Recurrent neural network architecture" ;
    rdfs:seeAlso <https://www.wikidata.org/entity/Q6673524> .
:markov_model a :ML_approach ;
    skos:prefLabel "Markov model" ;
    skos:altLabel "MM" ;
    rdfs:comment "Probability tool" ;
    rdfs:seeAlso <https://www.wikidata.org/entity/Q6771326> .
:martrix_profile a :ML_approach ;
    skos:prefLabel "Martrix Profile" ;
    skos:altLabel "MP" ;
    :used_for :time_series_classification ;
    rdfs:comment "Martrix Profile (MP) classifier" .
:maximum_entropy_markov_model a :ML_approach ;
    skos:prefLabel "maximum entropy Markov model" ;
    skos:altLabel "MEMM" ;
    skos:broader :markov_model ;
    rdfs:comment "Graphical model for sequence labeling that combines features of hidden Markov models (HMMs) and maximum entropy (MaxEnt) models" ;
    rdfs:seeAlso <https://www.wikidata.org/entity/Q6795829> .
:mean_shift_clustering a :ML_approach ;
    skos:prefLabel "Mean shift Clustering" ;
    :used_for :clustering ;
    rdfs:comment "Mean shift clustering iteratively moves data points uphill in a density landscape to discover clusters." ;
    rdfs:seeAlso <https://www.wikidata.org/wiki/Q6803557> .
:multi_scale_convolutional_neural_networks a :ML_approach ;
    skos:prefLabel "Multi-Scale Convolutional Neural Networks" ;
    skos:altLabel "MCNN" ;
    skos:broader :artificial_neural_network ;
    :used_for :time_series_classification ;
    :performance :scalable ;
    rdfs:comment "A novel end-to-end neural network model, MCNN, incorporates feature extraction and classification in a single framework." .
:multilayer_perceptron a :ML_approach ;
    skos:prefLabel "multilayer perceptron" ;
    skos:altLabel "MLP" ;
    skos:broader :feed_forward_neural_network ;
    rdfs:comment "Type of feedforward neural network" ;
    rdfs:seeAlso <https://www.wikidata.org/entity/Q2991667> .
:multinominal_naive_bayes a :ML_approach ;
    skos:prefLabel "multinominal naive bayes" ;
    :used_for :classification ;
    :possible_if :large_dataset , :text_features ;
    :performance :fast_training ;
    rdfs:comment "Simple probabilistic classifier based on applying Bayes' theorem with strong (naive) independence assumptions between the features" ;
    rdfs:seeAlso <https://www.wikidata.org/entity/Q812530> .
:multivariate_regression a :ML_approach ;
    skos:prefLabel "multivariate regression" ;
    :used_for :regression .
:multivariate_symbolic_extension a :ML_approach ;
    skos:prefLabel "MUltivariate Symbolic Extension" ;
    skos:altLabel "MUSE" ;
    :used_for :time_series_classification .
:ordering_points_to_identify_the_clustering_structure a :ML_approach ;
    skos:prefLabel "ordering points to identify the clustering structure" ;
    skos:altLabel "OPTICS" ;
    :used_for :clustering .
:orthogonal_matching_pursuit a :ML_approach ;
    skos:prefLabel "Orthogonal Matching Pursuit" .
:passive_aggressive a :ML_approach ;
    skos:prefLabel "passive aggressive" ;
    :used_for :classification ;
    rdfs:comment "Family of algorithms for large-scale learning" .
:perceptron a :ML_approach ;
    skos:prefLabel "perceptron" ;
    skos:broader :artificial_neural_network ;
    rdfs:comment "Algorithm for supervised learning of binary classifiers" ;
    rdfs:seeAlso <https://www.wikidata.org/entity/Q690207> .
:poisson_regression a :ML_approach ;
    skos:prefLabel "poisson regression" ;
    skos:broader :linear_regression ;
    :used_for :regression ;
    rdfs:comment "Statistical model for count data" ;
    rdfs:seeAlso <https://www.wikidata.org/entity/Q954529> .
:polynomial_regression a :ML_approach ;
    skos:prefLabel "polynomial regression" ;
    :used_for :regression ;
    rdfs:comment "Regression analysis in which the relationship between the independent variable x and the dependent variable y is modelled as an nth degree polynomial in x" ;
    rdfs:seeAlso <https://www.wikidata.org/entity/Q45343> .
:prophet a :ML_approach ;
    skos:prefLabel "prophet" ;
    :used_for :time_series_analysis .
:proximity_forest a :ML_approach ;
    skos:prefLabel "Proximity Forest" ;
    skos:altLabel "PF" ;
    skos:broader :ensemble ;
    :used_for :time_series_classification ;
    rdfs:comment "Models a decision tree forest which uses distance measures to partition data" .
:decision_stump a :ML_approach ;
    skos:prefLabel "decision stump" ;
    :used_for :time_series_classification ;
    rdfs:comment "Models a decision stump which uses a distance measure to partition data" .
:proximity_tree a :ML_approach ;
    skos:prefLabel "Proximity Tree" ;
    skos:broader :decision_tree ;
    :used_for :time_series_classification ;
    rdfs:comment "A decision tree which uses distance measures to partition data" .
:quadratic_discriminant_analysis a :ML_approach ;
    skos:prefLabel "Quadratic Discriminant Analysis" ;
    :used_for :classification .
:random_forest a :ML_approach ;
    skos:prefLabel "random forest" ;
    skos:broader :decision_tree ;
    :used_for :classification , :regression ;
    :performance :fast_training , :accurate ;
    rdfs:comment "Ensemble learning method for classification, regression and other tasks that operates by constructing a multitude of decision trees at training time" ;
    rdfs:seeAlso <https://www.wikidata.org/entity/Q245748> .
:distributed_random_forest a :ML_approach ;
    skos:prefLabel "distributed random forest" ;
    skos:altLabel "DRF" ;
    skos:broader :random_forest ;
    :used_for :classification , :regression .
:random_interval a :ML_approach ;
    skos:prefLabel "Random Interval" ;
    :used_for :time_series_classification ;
    rdfs:comment "Random Interval Classifier" .
:random_interval_spectral_ensemble a :ML_approach ;
    skos:prefLabel "Random Interval Spectral Ensemble" ;
    skos:altLabel "RISE" ;
    :used_for :time_series_classification .
:random_kitchen_sinks_sampler a :ML_approach ;
    skos:prefLabel "random kitchen sinks sampler" ;
    rdfs:comment "Approximate a RBF kernel feature map using random Fourier features" .
:random_sample_consensus a :ML_approach ;
    skos:prefLabel "RANdom SAmple Consensus" ;
    skos:altLabel "RANSAC" ;
    :used_for :regression ;
    rdfs:seeAlso <https://www.wikidata.org/entity/Q218533> .
:recurrent_nn a :ML_approach ;
    skos:prefLabel "recurrent nn" ;
    skos:altLabel "RNN" ;
    skos:broader :artificial_neural_network ;
    :used_for :time_series_analysis ;
    rdfs:comment "Class of artificial neural network where connections between units form a directed graph along a temporal sequence" ;
    rdfs:seeAlso <https://www.wikidata.org/entity/Q1457734> .
:residual_neural_network a :ML_approach ;
    skos:prefLabel "Residual Neural Network" ;
    skos:altLabel "ResNet" ;
    skos:broader :artificial_neural_network ;
    :used_for :image_classification , :time_series_classification ;
    rdfs:comment "Deep Convolutional and LSTM Recurrent Neural Networks for Multimodal Wearable Activity Recognition" .
:ridge_classifier a :ML_approach ;
    skos:prefLabel "Ridge Classifier" ;
    :used_for :classification .
:ridge_regression a :ML_approach ;
    skos:prefLabel "ridge regression" ;
    skos:broader :linear_regression ;
    :used_for :classification , :regression ;
    rdfs:comment "Regularization technique for ill-posed problems" ;
    rdfs:seeAlso <https://www.wikidata.org/entity/Q2778212> .
:seasonal_autoregressive_integrated_moving_average_exogenous a :ML_approach ;
    skos:prefLabel "seasonal autoregressive integrated moving average exogenous" ;
    skos:altLabel "SARIMAX" ;
    :used_for :time_series_analysis .
:self_organizing_map a :ML_approach ;
    skos:prefLabel "self-organizing map" ;
    skos:altLabel "SOM" ;
    :used_for :clustering , :anomaly_detection , :feature_reduction ;
    rdfs:comment "Type of artificial neural network" ;
    rdfs:seeAlso <https://www.wikidata.org/entity/Q1136838> .
:self_organizing_tree_algorithm a :ML_approach ;
    skos:prefLabel "self-organizing tree algorithm" ;
    skos:altLabel "SOTA" ;
    :used_for :clustering , :anomaly_detection .
:shapelet_transform_classifier a :ML_approach ;
    skos:prefLabel "Shapelet Transform Classifier" ;
    :used_for :time_series_classification ;
    :performance :long_training_time .
:signature_classifier a :ML_approach ;
    skos:prefLabel "Signature Classifier" ;
    :used_for :time_series_classification ;
    rdfs:comment "Classification module using signature-based features" .
:singular_value_decomposition a :ML_approach ;
    skos:prefLabel "singular value decomposition" ;
    skos:altLabel "SVD" ;
    :used_for :feature_reduction , :recommendation ;
    :possible_if :numerical_features ;
    rdfs:comment "Factorization of a real or complex matrix" ;
    rdfs:seeAlso <https://www.wikidata.org/entity/Q420904> .
:spectral_clustering a :ML_approach ;
    skos:prefLabel "spectral clustering" ;
    :used_for :clustering ;
    rdfs:comment "Performing dimensionality reduction before clustering in fewer dimensions by making use of the spectrum (eigenvalues) of the similarity matrix of the data" ;
    rdfs:seeAlso <https://www.wikidata.org/entity/Q2976589> .
:stacking_ensemble a :ML_approach ;
    skos:prefLabel "stacking ensemble" ;
    :used_for :classification .
:stochastic_gradient_descent a :ML_approach ;
    skos:prefLabel "stochastic gradient descent" ;
    skos:altLabel "SGD" ;
    :used_for :classification , :regression ;
    rdfs:comment "optimization algorithm" ;
    rdfs:seeAlso <https://www.wikidata.org/entity/Q7617819> .
:summary_statistic a :ML_approach ;
    skos:prefLabel "Summary statistic" ;
    :used_for :time_series_classification ;
    rdfs:comment "Summary statistic classifier" .
:supervised_time_series_forest a :ML_approach ;
    skos:prefLabel "Supervised Time Series Forest" ;
    skos:altLabel "STSF" ;
    :used_for :time_series_classification ;
    :performance :fast_training , :explainable , :scalable .
:support_vector_machine a :ML_approach ;
    skos:prefLabel "support vector machine" ;
    skos:altLabel "SVM" ;
    :used_for :classification , :regression , :anomaly_detection ;
    :not_recommended_if :many_features ;
    rdfs:comment "Set of methods for supervised statistical learning" ;
    rdfs:seeAlso <https://www.wikidata.org/entity/Q282453> .
:support_vector_regression a :ML_approach ;
    skos:prefLabel "support vector regression" ;
    skos:broader :linear_regression ;
    :used_for :regression ;
    rdfs:comment "SVM for regression tasks" ;
    rdfs:seeAlso <https://www.wikidata.org/entity/Q57534282> .
:temporal_dictionary_ensemble a :ML_approach ;
    skos:prefLabel "Temporal Dictionary Ensemble" ;
    skos:altLabel "TDE" ;
    skos:broader :ensemble ;
    :used_for :time_series_classification .
:temporal_fusion_transformer a :ML_approach ;
    skos:prefLabel "temporal fusion transformer" ;
    skos:broader :transformer ;
    :used_for :time_series_forecasting .
:theta_method a :ML_approach ;
    skos:prefLabel "Theta method" ;
    :used_for :time_series_forecasting .
:time_series_combination_of_heterogeneous_and_integrated_embedding_forest a :ML_approach ;
    skos:prefLabel "Time Series Combination of Heterogeneous and Integrated Embedding Forest" ;
    skos:altLabel "TS-CHIEF" ;
    :used_for :time_series_classification ;
    :performance :long_training_time .
:time_series_forest a :ML_approach ;
    skos:prefLabel "Time series forest" ;
    skos:altLabel "TSF" ;
    :used_for :time_series_classification ;
    :performance :fast_training , :explainable , :scalable ;
    rdfs:comment "Time series forest (TSF) classifier" .
:transformer a :ML_approach ;
    skos:prefLabel "transformer" ;
    skos:broader :artificial_neural_network ;
    rdfs:comment "Deep learning model adopting self-attention" ;
    rdfs:seeAlso <https://www.wikidata.org/entity/Q85810444> .
:variational_bayesian_gaussian_mixture_model a :ML_approach ;
    skos:prefLabel "variational Bayesian Gaussian mixture model" ;
    skos:altLabel "VB-GMM" ;
    skos:broader :gaussian_mixture_model ;
    :used_for :clustering .
:word_extraction_for_time_series_classification a :ML_approach ;
    skos:prefLabel "Word Extraction for Time Series Classification" ;
    skos:altLabel "WEASEL" ;
    :used_for :time_series_classification .
:word2vector a :ML_approach ;
    skos:prefLabel "word2vector" ;
    skos:altLabel "word2vec" ;
    :used_for :text_analytics ;
    rdfs:comment "Group of related models that are used to produce word embeddings" ;
    rdfs:seeAlso <https://www.wikidata.org/entity/Q22673982> .
:xgboost a :ML_approach ;
    skos:prefLabel "xgboost" ;
    skos:altLabel "XGB" ;
    skos:broader :gradient_boosting_tree ;
    :used_for :classification , :regression ;
    :performance :accurate , :explainable ;
    rdfs:comment "Scalable machine learning system for tree boosting" ;
    rdfs:seeAlso <https://www.wikidata.org/entity/Q23793561> .


# Preprocessing_approach

:kernel_approximation a :Preprocessing_approach ;
    skos:prefLabel "kernel approximation" ;
    :used_for :classification , :regression .
:principal_component_analysis a :Preprocessing_approach ;
    skos:prefLabel "principal component analysis" ;
    skos:altLabel "PCA" ;
    :used_for :feature_reduction , :anomaly_detection ;
    :possible_if :numerical_features ;
    :performance :fast_training ;
    rdfs:comment "Conversion of a set of observations of possibly correlated variables into a set of values of linearly uncorrelated variables called principal components" ;
    rdfs:seeAlso <https://www.wikidata.org/entity/Q2873> .
:kernel_principal_component_analysis a :Preprocessing_approach ;
    skos:prefLabel "kernel principal component analysis" ;
    skos:altLabel "kernel PCA" ;
    skos:broader :principal_component_analysis ;
    :used_for :feature_reduction , :anomaly_detection ;
    :possible_if :numerical_features ;
    :performance :fast_training ;
    rdfs:comment "Multivariate analysis technique with kernel method" ;
    rdfs:seeAlso <https://www.wikidata.org/entity/Q17093020> .
:nystroem_kernel_approximation a :Preprocessing_approach ;
    skos:prefLabel "Nystroem kernel approximation" ;
    skos:broader :kernel_approximation .
:radial_basis_function_kernel a :Preprocessing_approach ;
    skos:prefLabel "radial basis function kernel" ;
    skos:altLabel "RBF kernel" ;
    skos:broader :kernel_approximation ;
    rdfs:comment "Popular kernel function used in SVM classification" ;
    rdfs:seeAlso <https://www.wikidata.org/entity/Q7280263> .
:rocket a :Preprocessing_approach ;
    skos:prefLabel "ROCKET" .
:minirocket a :Preprocessing_approach ;
    skos:prefLabel "MiniROCKET" .


# Metric

:accuracy a :Metric ;
    skos:prefLabel "accuracy" ;
    :used_for :classification ;
    :recommended_if :balanced_dataset ;
    :not_recommended_if :unbalanced_dataset ;
    rdfs:comment "Simple prediction performance measure for classification tasks" ;
    rdfs:seeAlso <https://www.wikidata.org/entity/Q272035> .
:adjusted_rand_score a :Metric ;
    skos:prefLabel "Adjusted Rand Score" ;
    skos:altLabel "ARI" , "Adjusted Rand Index" ;
    :used_for :classification ;
    rdfs:comment "measure of the similarity between two data clusterings" .
:area_under_precision_recall_curve a :Metric ;
    skos:prefLabel "area under precision recall curve" ;
    skos:altLabel "AUCPR" , "AUPRC" , "AUC-PR" ;
    :used_for :classification ;
    rdfs:comment "AUC-PR stands for area under the (precision-recall) curve. Generally, the higher the AUC-PR score, the better a classifier performs for the given task. One way to calculate AUC-PR is to find the AP, or average precision." .
:area_under_roc_curve a :Metric ;
    skos:prefLabel "area under roc curve" ;
    skos:altLabel "AUC" ;
    :used_for :classification ;
    rdfs:comment "Simple Generalisation of the Area Under the ROC Curve for Multiple Class Classification Problems" ;
    rdfs:seeAlso <https://www.wikidata.org/entity/Q55878266> .
:area_under_roc_curve_macro a :Metric ;
    skos:prefLabel "area under roc curve macro" ;
    skos:altLabel "AUC macro" ;
    :used_for :classification ;
    rdfs:comment "AUC score for multiclass classification using macro averaging" .
:area_under_roc_curve_micro a :Metric ;
    skos:prefLabel "area under roc curve micro" ;
    skos:altLabel "AUC micro" ;
    :used_for :classification ;
    rdfs:comment "AUC score for multiclass classification using micro averaging" .
:area_under_roc_curve_weighted a :Metric ;
    skos:prefLabel "area under roc curve weighted" ;
    skos:altLabel "AUC weighted" ;
    :used_for :classification ;
    rdfs:comment "AUC score for multiclass classification using weighted averaging" .
:average_precision a :Metric ;
    skos:prefLabel "average precision" ;
    skos:altLabel "AP" ;
    :used_for :classification .
:balanced_accuracy a :Metric ;
    skos:prefLabel "balanced accuracy" ;
    :used_for :classification .
:binary_accuracy a :Metric ;
    skos:prefLabel "binary accuracy" ;
    :used_for :classification ;
    rdfs:comment "Calculates how often predictions match binary labels" .
:binary_cross_entropy a :Metric ;
    skos:prefLabel "binary cross entropy" ;
    :used_for :classification .
:binary_intersection_over_union a :Metric ;
    skos:prefLabel "binary intersection over union" ;
    skos:altLabel "binary IoU" ;
    :used_for :image_segmentation ;
    rdfs:comment "Computes the Intersection-Over-Union metric for class 0 and / or 1" .
:brier a :Metric ;
    skos:prefLabel "brier" ;
    :used_for :classification .
:categorical_accuracy a :Metric ;
    skos:prefLabel "categorical accuracy" ;
    :used_for :classification ;
    rdfs:comment "Calculates how often predictions match one-hot labels" .
:categorical_cross_entropy a :Metric ;
    skos:prefLabel "categorical cross entropy" ;
    :used_for :classification .
:categorical_hinge a :Metric ;
    skos:prefLabel "categorical hinge" ;
    :used_for :classification .
:coefficient_of_determination a :Metric ;
    skos:prefLabel "coefficient of determination" ;
    skos:altLabel "R2" ;
    :used_for :regression ;
    rdfs:comment "Indicator for how well data points fit a line or curve" ;
    rdfs:seeAlso <https://www.wikidata.org/entity/Q192830> .
:cohens_kappa a :Metric ;
    skos:prefLabel "cohens kappa" ;
    rdfs:comment "Statistic measuring inter-rater agreement for categorical items kappa" ;
    rdfs:seeAlso <https://www.wikidata.org/entity/Q1107106> .
:cosine_similarity a :Metric ;
    skos:prefLabel "cosine similarity" ;
    :used_for :regression .
:coverage a :Metric ;
    skos:prefLabel "Coverage" ;
    :used_for :time_series_forecasting ;
    rdfs:comment "Percentage of actual values that are within the prediction intervall" .
:critical_success_index a :Metric ;
    skos:prefLabel "critical success index" ;
    skos:altLabel "CSI" , "Threat score" , "TS" .
:d2_absolute_error a :Metric ;
    skos:prefLabel "d2 absolute error" ;
    :used_for :regression .
:d2_pinball_score a :Metric ;
    skos:prefLabel "d2 pinball score" ;
    :used_for :regression .
:d2_tweedie_score a :Metric ;
    skos:prefLabel "d2 tweedie score" ;
    :used_for :regression .
:explained_variance a :Metric ;
    skos:prefLabel "explained variance" ;
    skos:altLabel "Max Error" ;
    :used_for :regression ;
    rdfs:comment "Explained variance score for regression" .
:f_measure a :Metric ;
    skos:prefLabel "F-measure" ;
    skos:altLabel "F" , "F1" , "F1-score" ;
    :used_for :classification ;
    :recommended_if :unbalanced_dataset ;
    rdfs:comment "Measure of a test's accuracy" ;
    rdfs:seeAlso <https://www.wikidata.org/entity/Q6975395> .
:f_measure_macro a :Metric ;
    skos:prefLabel "F-measure macro" ;
    skos:altLabel "F1 macro" ;
    :used_for :classification .
:f_measure_micro a :Metric ;
    skos:prefLabel "F-measure micro" ;
    skos:altLabel "F1 micro" ;
    :used_for :classification .
:f_measure_samples a :Metric ;
    skos:prefLabel "F-measure samples" ;
    :used_for :classification .
:f_measure_weighted a :Metric ;
    skos:prefLabel "F-measure weighted" ;
    skos:altLabel "F1 weighted" ;
    :used_for :classification .
:false_discovery_rate a :Metric ;
    skos:prefLabel "false discovery rate" ;
    skos:altLabel "FDR" ;
    rdfs:comment "Statistical method for handling multiple comparisons" ;
    rdfs:seeAlso <https://www.wikidata.org/entity/Q5432696> .
:false_negative_rate a :Metric ;
    skos:prefLabel "false negative rate" ;
    skos:altLabel "FNR" , "miss rate" .
:false_negatives a :Metric ;
    skos:prefLabel "false negatives" ;
    :used_for :classification .
:false_omission_rate a :Metric ;
    skos:prefLabel "false omission rate" ;
    skos:altLabel "FOR" .
:false_positive_rate a :Metric ;
    skos:prefLabel "false positive rate" ;
    skos:altLabel "FPR" , "fall-out" ;
    rdfs:comment "Probability of falsely rejecting the null hypothesis for a particular test" ;
    rdfs:seeAlso <https://www.wikidata.org/entity/Q5432725> .
:false_positives a :Metric ;
    skos:prefLabel "false positives" ;
    :used_for :classification .
:fowlkes_mallows_index a :Metric ;
    skos:prefLabel "fowlkes mallows index" ;
    skos:altLabel "FM" ;
    rdfs:comment "External evaluation method used to determine the similarity between two clusterings" ;
    rdfs:seeAlso <https://www.wikidata.org/entity/Q5476477> .
:gini a :Metric ;
    skos:prefLabel "gini" ;
    skos:altLabel "Gini" ;
    :used_for :classification ;
    rdfs:comment "Index to measure inequality" .
:hinge a :Metric ;
    skos:prefLabel "hinge" ;
    :used_for :classification .
:informedness a :Metric ;
    skos:prefLabel "informedness" ;
    skos:altLabel "bookmaker informedness" , "BM" .
:intersection_over_union a :Metric ;
    skos:prefLabel "intersection over union" ;
    skos:altLabel "IoU" ;
    :used_for :image_segmentation .
:jaccard a :Metric ;
    skos:prefLabel "Jaccard" ;
    skos:altLabel "Jaccard Index" , "Jaccard distance" ;
    :used_for :classification ;
    rdfs:comment "Measure of similarity and diversity between sets" ;
    rdfs:seeAlso <https://www.wikidata.org/entity/Q865360> .
:jaccard_macro a :Metric ;
    skos:prefLabel "Jaccard macro" ;
    :used_for :classification .
:jaccard_micro a :Metric ;
    skos:prefLabel "Jaccard micro" ;
    :used_for :classification .
:jaccard_samples a :Metric ;
    skos:prefLabel "Jaccard samples" ;
    :used_for :classification .
:jaccard_weighted a :Metric ;
    skos:prefLabel "Jaccard weighted" ;
    :used_for :classification .
:kullback_leibler_divergence a :Metric ;
    skos:prefLabel "kullback-leibler divergence" ;
    skos:altLabel "KL divergence" .
:log_cosh_error a :Metric ;
    skos:prefLabel "log cosh error" ;
    :used_for :regression .
:log_loss a :Metric ;
    skos:prefLabel "log loss" ;
    skos:altLabel "Log loss" ;
    :used_for :classification ;
    rdfs:comment "Average cross-entropy between the distribution of the true labels and the predictions" ;
    rdfs:seeAlso <https://www.wikidata.org/entity/Q22667762> .
:markedness a :Metric ;
    skos:prefLabel "markedness" ;
    skos:altLabel "MK" , "deltaP" ;
    rdfs:comment "State of standing out as unusual or difficult in comparison to a more common or regular form" ;
    rdfs:seeAlso <https://www.wikidata.org/entity/Q1897166> .
:matthews_correlation_coefficient a :Metric ;
    skos:prefLabel "matthews correlation coefficient" ;
    skos:altLabel "MCC" ;
    rdfs:comment "Measure of the quality of binary (two-class) classifications" ;
    rdfs:seeAlso <https://www.wikidata.org/entity/Q6791500> .
:max_error a :Metric ;
    skos:prefLabel "max error" ;
    skos:altLabel "Max Error" ;
    :used_for :regression ;
    rdfs:comment "Maximum residual error for regression" .
:mean a :Metric ;
    skos:prefLabel "mean" .
:mean_absolute_error a :Metric ;
    skos:prefLabel "mean absolute error" ;
    skos:altLabel "MAE" ;
    :used_for :regression , :time_series_forecasting ;
    rdfs:comment "Measure of difference between two continuous variables" ;
    rdfs:seeAlso <https://www.wikidata.org/entity/Q6803609> .
:mean_absolute_percentage_error a :Metric ;
    skos:prefLabel "mean absolute percentage error" ;
    skos:altLabel "MAPE" ;
    :used_for :regression , :time_series_forecasting ;
    rdfs:comment "Measure of prediction accuracy of a forecast" ;
    rdfs:seeAlso <https://www.wikidata.org/entity/Q6803607> .
:mean_absolute_scaled_error a :Metric ;
    skos:prefLabel "mean absolute scaled error" ;
    skos:altLabel "MASE" ;
    :used_for :time_series_forecasting ;
    rdfs:comment "Measure of forecasting quality" ;
    rdfs:seeAlso <https://www.wikidata.org/entity/Q6803610> .
:mean_gamma_deviance a :Metric ;
    skos:prefLabel "mean gamma deviance" ;
    :used_for :regression .
:mean_intersection_over_union a :Metric ;
    skos:prefLabel "mean intersection-over-union" ;
    skos:altLabel "mean intersection-over-union" ;
    :used_for :image_segmentation .
:mean_metric_wrapper a :Metric ;
    skos:prefLabel "mean metric wrapper" .
:mean_per_class_error a :Metric ;
    skos:prefLabel "mean per class error" ;
    :used_for :classification ;
    rdfs:comment "Average of the error rate for each class" .
:mean_poisson_deviance a :Metric ;
    skos:prefLabel "mean poisson deviance" ;
    :used_for :regression .
:mean_relative_error a :Metric ;
    skos:prefLabel "mean relative error" ;
    :used_for :regression .
:mean_residual_deviance a :Metric ;
    skos:prefLabel "mean residual deviance" ;
    :used_for :regression .
:mean_squared_error a :Metric ;
    skos:prefLabel "mean squared error" ;
    skos:altLabel "MSE" ;
    :used_for :classification , :regression ;
    rdfs:comment "Average of the squares of the errors between estimated and actual values" ;
    rdfs:seeAlso <https://www.wikidata.org/entity/Q1940696> .
:mean_squared_log_error a :Metric ;
    skos:prefLabel "mean squared log error" ;
    :used_for :regression .
:mean_tensor a :Metric ;
    skos:prefLabel "mean tensor" .
:median_absolute_error a :Metric ;
    skos:prefLabel "median absolute error" ;
    skos:altLabel "MAE" ;
    :used_for :regression , :time_series_forecasting .
:median_absolute_error a :Metric ;
    skos:prefLabel "median absolute error" ;
    skos:altLabel "Median AE" ;
    :used_for :regression .
:median_absolute_percentage_error a :Metric ;
    skos:prefLabel "median absolute percentage error" ;
    skos:altLabel "MAPE" ;
    :used_for :regression , :time_series_forecasting .
:median_absolute_scaled_error a :Metric ;
    skos:prefLabel "median absolute scaled error" ;
    skos:altLabel "MASE" ;
    :used_for :time_series_forecasting .
:median_squared_error a :Metric ;
    skos:prefLabel "median squared error" ;
    skos:altLabel "MSE" ;
    :used_for :regression , :time_series_forecasting .
:neg_log_loss a :Metric ;
    skos:prefLabel "neg log loss" ;
    skos:altLabel "Neg Log loss" ;
    :used_for :classification ;
    rdfs:comment "Average cross-entropy between the distribution of the true labels and the predictions" ;
    rdfs:seeAlso <https://www.wikidata.org/entity/Q22667762> .
:negative_predictive_value a :Metric ;
    skos:prefLabel "negative predictive value" ;
    skos:altLabel "NPV" ;
    rdfs:comment "Proportion of negative results in tests that are true negative" ;
    rdfs:seeAlso <https://www.wikidata.org/entity/Q2776546> .
:normalized_discounted_cumulative_gain a :Metric ;
    skos:prefLabel "normalized discounted cumulative gain" ;
    skos:altLabel "NDCG" ;
    :used_for :ranking .
:one_hot_intersection_over_union a :Metric ;
    skos:prefLabel "one hot intersection over union" ;
    :used_for :image_segmentation .
:one_hot_mean_intersection_over_union a :Metric ;
    skos:prefLabel "one hot mean intersection over union" ;
    skos:altLabel "one hot mean IoU" ;
    :used_for :image_segmentation .
:overall_accuracy a :Metric ;
    skos:prefLabel "overall accuracy" ;
    :used_for :classification .
:overall_f1 a :Metric ;
    skos:prefLabel "overall f1" ;
    :used_for :classification .
:overall_precision a :Metric ;
    skos:prefLabel "overall precision" ;
    :used_for :classification .
:overall_recall a :Metric ;
    skos:prefLabel "overall recall" ;
    :used_for :classification .
:pac_score a :Metric ;
    skos:prefLabel "pac score" ;
    skos:altLabel "PAC-Bayesian AUC classification and scoring" ;
    :used_for :classification .
:pearson_correlation_coefficient a :Metric ;
    skos:prefLabel "pearson correlation coefficient" ;
    skos:altLabel "pearsonr" ;
    :used_for :regression ;
    rdfs:comment "Type of coefficient" ;
    rdfs:seeAlso <https://www.wikidata.org/entity/Q1136628> .
:poisson a :Metric ;
    skos:prefLabel "poisson" .
:precision a :Metric ;
    skos:prefLabel "precision" ;
    skos:altLabel "positive predictive value" , "PPV" ;
    :used_for :classification ;
    rdfs:comment "Reason for preferred rank based on level of detail, time precision (e.g. day instead of year)" ;
    rdfs:seeAlso <https://www.wikidata.org/entity/Q71536040> .
:precision_at_recall a :Metric ;
    skos:prefLabel "precision at recall" ;
    :used_for :classification ;
    rdfs:comment "Computes best precision where recall is >= specified value." .
:precision_macro a :Metric ;
    skos:prefLabel "precision macro" ;
    :used_for :classification .
:precision_micro a :Metric ;
    skos:prefLabel "precision micro" ;
    :used_for :classification .
:precision_samples a :Metric ;
    skos:prefLabel "precision samples" ;
    :used_for :classification .
:precision_weighted a :Metric ;
    skos:prefLabel "precision weighted" ;
    :used_for :classification .
:prevalence_threshold a :Metric ;
    skos:prefLabel "prevalence threshold" ;
    skos:altLabel "PT" .
:r2 a :Metric ;
    skos:prefLabel "r2" ;
    skos:altLabel "R2 scrore" ;
    :used_for :regression .
:recall a :Metric ;
    skos:prefLabel "recall" ;
    skos:altLabel "sensitivity" , "hit rate" , "true positive rate" , "TPR" ;
    :used_for :classification ;
    rdfs:comment "Retrieval of events or information from the past" ;
    rdfs:seeAlso <https://www.wikidata.org/entity/Q18733> .
:recall_at_precision a :Metric ;
    skos:prefLabel "recall at precision" ;
    :used_for :classification .
:recall_macro a :Metric ;
    skos:prefLabel "recall macro" ;
    :used_for :classification .
:recall_micro a :Metric ;
    skos:prefLabel "recall micro" ;
    :used_for :classification .
:recall_samples a :Metric ;
    skos:prefLabel "recall samples" ;
    :used_for :classification .
:recall_weighted a :Metric ;
    skos:prefLabel "recall weighted" ;
    :used_for :classification .
:receiver_operating_characteristic_curve a :Metric ;
    skos:prefLabel "receiver operating characteristic curve" ;
    skos:altLabel "ROC AUC" ;
    :used_for :classification .
:receiver_operating_characteristic_curve_weighted a :Metric ;
    skos:prefLabel "receiver operating characteristic curve weighted" ;
    skos:altLabel "ROC AUC weighted" ;
    :used_for :classification .
:receiver_operating_characteristic_curve_samples a :Metric ;
    skos:prefLabel "receiver operating characteristic curve samples" ;
    skos:altLabel "ROC AUC samples" ;
    :used_for :classification .
:receiver_operating_characteristic_curve_one_vs_one a :Metric ;
    skos:prefLabel "receiver operating characteristic curve one vs one" ;
    skos:altLabel "ROC AUC OVO" ;
    :used_for :classification .
:receiver_operating_characteristic_curve_one_vs_one_macro a :Metric ;
    skos:prefLabel "receiver operating characteristic curve one vs one macro" ;
    skos:altLabel "ROC AUC OVO macro" ;
    :used_for :classification .
:receiver_operating_characteristic_curve_one_vs_one_weighted a :Metric ;
    skos:prefLabel "receiver operating characteristic curve one vs one weighted" ;
    skos:altLabel "ROC AUC OVO weighted" ;
    :used_for :classification .
:receiver_operating_characteristic_curve_one_vs_rest a :Metric ;
    skos:prefLabel "receiver operating characteristic curve one vs rest" ;
    skos:altLabel "ROC AUC OVR" ;
    :used_for :classification .
:receiver_operating_characteristic_curve_one_vs_rest_micro a :Metric ;
    skos:prefLabel "receiver operating characteristic curve one vs rest micro" ;
    skos:altLabel "ROC AUC OVR micro" ;
    :used_for :classification .
:receiver_operating_characteristic_curve_one_vs_rest_macro a :Metric ;
    skos:prefLabel "receiver operating characteristic curve one vs rest macro" ;
    skos:altLabel "ROC AUC OVR macro" ;
    :used_for :classification .
:receiver_operating_characteristic_curve_one_vs_rest_weighted a :Metric ;
    skos:prefLabel "receiver operating characteristic curve one vs rest weighted" ;
    skos:altLabel "ROC AUC OVR weighted" ;
    :used_for :classification .
:root_mean_squared_error a :Metric ;
    skos:prefLabel "root mean squared error" ;
    skos:altLabel "RMSE" ;
    :used_for :regression .
:root_mean_squared_log_error a :Metric ;
    skos:prefLabel "root mean squared log error" ;
    skos:altLabel "RMSLE" ;
    :used_for :regression .
:root_mean_squared_scaled_error a :Metric ;
    skos:prefLabel "root mean squared scaled error" ;
    skos:altLabel "RMSSE" ;
    :used_for :time_series_forecasting .
:sensitifity_at_specificity a :Metric ;
    skos:prefLabel "sensitifity at specificity" ;
    :used_for :classification .
:sparse_categorical_accuracy a :Metric ;
    skos:prefLabel "sparse categorical accuracy" ;
    :used_for :classification ;
    rdfs:comment "Calculates how often predictions match integer labels" .
:sparse_categorical_crossentropy a :Metric ;
    skos:prefLabel "sparse categorical crossentropy" ;
    :used_for :classification .
:sparse_top_k_categorical_accuracy a :Metric ;
    skos:prefLabel "sparse top k categorical accuracy" ;
    :used_for :classification ;
    rdfs:comment "Computes how often integer targets are in the top K predictions" .
:spearman_rank_correlation_coefficient a :Metric ;
    skos:prefLabel "Spearman rank correlation coefficient" ;
    skos:altLabel "spearmanr" ;
    :used_for :regression ;
    rdfs:comment "Nonparametric measure of rank correlation" ;
    rdfs:seeAlso <https://www.wikidata.org/entity/Q1126730> .
:specificity a :Metric ;
    skos:prefLabel "specificity" ;
    skos:altLabel "selectivity" , "true negative rate" , "TNR" .
:specificity_at_sensitivity a :Metric ;
    skos:prefLabel "specificity at sensitivity" ;
    :used_for :classification .
:squared_hinge a :Metric ;
    skos:prefLabel "squared hinge" ;
    :used_for :classification .
:sum a :Metric ;
    skos:prefLabel "sum" .
:symmetric_mean_absolute_percentage_error a :Metric ;
    skos:prefLabel "symmetric mean absolute percentage error" ;
    skos:altLabel "SMAPE" ;
    :used_for :time_series_forecasting .
:top_k_categorical_accuracy a :Metric ;
    skos:prefLabel "top k categorical accuracy" ;
    :used_for :classification ;
    rdfs:comment "Computes how often targets are in the top K predictions" .
:true_negatives a :Metric ;
    skos:prefLabel "true negatives" ;
    skos:altLabel "TN" ;
    :used_for :classification .
:true_positives a :Metric ;
    skos:prefLabel "true positives" ;
    skos:altLabel "TP" ;
    :used_for :classification .


# ML_library

:catboost_lib a :ML_library ;
    skos:prefLabel "CatBoost" ;
    rdfs:comment "Yandex open source gradient boosting framework on decision trees" ;
    rdfs:seeAlso <https://www.wikidata.org/entity/Q55656976> .
:fastai_lib a :ML_library ;
    skos:prefLabel "Fastai" ;
    rdfs:comment "Free open-source library for deep learning sitting atop PyTorch" ;
    rdfs:seeAlso <https://www.wikidata.org/entity/Q96377821> .
:gluonts_lib a :ML_library ;
    skos:prefLabel "GluonTS" ;
    rdfs:comment "GluonTS is a Python package for probabilistic time series modeling, focusing on deep learning based models, based on PyTorch and MXNet." ;
    rdfs:seeAlso <https://ts.gluon.ai> .
:greykite_lib a :ML_library ;
    skos:prefLabel "GreyKite" ;
    rdfs:comment "A flexible, intuitive and fast forecasting library" ;
    rdfs:seeAlso <https://github.com/linkedin/greykite> .
:h2o_lib a :ML_library ;
    skos:prefLabel "H2O" ;
    rdfs:comment "Machine learning library in Python" ;
    rdfs:seeAlso <https://www.wikidata.org/entity/Q16972732> .
:ibm_snap_ml_lib a :ML_library ;
    skos:prefLabel "IBM Snap ML" ;
    rdfs:comment "Snap ML is a library for training generalized linear models" ;
    rdfs:seeAlso <https://ibm.github.io/ai-on-z-101/snapml> .
:kats_lib a :ML_library ;
    skos:prefLabel "Kats" ;
    rdfs:comment "A kit to analyze time series data, a lightweight, extendable framework to perform time series analysis, from understanding the key statistics and characteristics, detecting change points and anomalies, to forecasting future trends." ;
    rdfs:seeAlso <https://github.com/facebookresearch/Kats> .
:keras_lib a :ML_library ;
    skos:prefLabel "Keras" ;
    skos:broader :tensorflow_lib ;
    rdfs:comment "Neural network library" ;
    rdfs:seeAlso <https://www.wikidata.org/entity/Q28470421> .
:lightgbm_lib a :ML_library ;
    skos:prefLabel "LightGBM" ;
    rdfs:comment "Free and open-source distributed gradient-boosting framework for machine learning" ;
    rdfs:seeAlso <https://www.wikidata.org/entity/Q57267665> .
:mllib_lib a :ML_library ;
    skos:prefLabel "MLlib" ;
    rdfs:comment "MLlib is Apache Spark's scalable machine learning library" ;
    rdfs:seeAlso <https://spark.apache.org/mllib> .
:mxnet_lib a :ML_library ;
    skos:prefLabel "MXNET" ;
    rdfs:comment "Multi-language machine learning library" ;
    rdfs:seeAlso <https://www.wikidata.org/entity/Q22348165> .
:pmdarima_lib a :ML_library ;
    skos:prefLabel "pmdarima" ;
    rdfs:comment "Pmdarima is a statistical library for time series analysis capabilities" ;
    rdfs:seeAlso <https://pypi.org/project/pmdarima> .
:prophet_lib a :ML_library ;
    skos:prefLabel "Prophet" ;
    rdfs:comment "Prophet is a library for forecasting time series data" ;
    rdfs:seeAlso <https://facebook.github.io/prophet> .
:pyflux_lib a :ML_library ;
    skos:prefLabel "PyFlux" ;
    rdfs:comment "PyFlux is a library for time series analysis and prediction" ;
    rdfs:seeAlso <https://github.com/RJT1990/pyflux> .
:pytorch_forecasting_lib a :ML_library ;
    skos:prefLabel "Pytorch-Forecasting" ;
    rdfs:comment "PyTorch Forecasting aims to ease state-of-the-art timeseries forecasting with neural networks for both real-world cases and research" ;
    rdfs:seeAlso <https://github.com/jdb78/pytorch-forecasting> .
:pytorch_lib a :ML_library ;
    skos:prefLabel "Pytorch" ;
    rdfs:comment "Open source machine learning library for Python, based on Torch" ;
    rdfs:seeAlso <https://www.wikidata.org/entity/Q47509047> .
:pywavelets_lib a :ML_library ;
    skos:prefLabel "PyWavelets" ;
    rdfs:comment "PyWavelets is open source wavelet transform software for Python. It combines a simple high level interface with low level C and Cython performance." ;
    rdfs:seeAlso <https://github.com/PyWavelets/pywt> .
:scikit_learn_lib a :ML_library ;
    skos:prefLabel "Scikit-learn" ;
    skos:altLabel "sklearn" ;
    rdfs:comment "Machine learning library for the Python programming language" ;
    rdfs:seeAlso <https://www.wikidata.org/entity/Q1026367> .
:sktime_lib a :ML_library ;
    skos:prefLabel "sktime" ;
    rdfs:comment "Modular open-source framework for a wide range of time series machine learning tasks. It offers scikit-learn compatible interfaces and model composition tools, with the goal to make the ecosystem more usable and interoperable as a whole." ;
    rdfs:seeAlso <https://github.com/sktime/sktime> .
:statsmodel_lib a :ML_library ;
    skos:prefLabel "Statsmodel" ;
    rdfs:comment "Statsmodels is a Python package that allows users to explore data, estimate statistical models, and perform statistical tests" ;
    rdfs:seeAlso <https://www.wikidata.org/entity/Q25304899> .
:tensorflow_lib a :ML_library ;
    skos:prefLabel "TensorFlow" ;
    rdfs:comment "Free and open-source software library for machine learning and artificial intelligence which can be used across a range of tasks but has a particular focus on training and inference of deep neural networks" ;
    rdfs:seeAlso <https://www.wikidata.org/entity/Q21447895> .
:tsfresh_lib a :ML_library ;
    skos:prefLabel "tsfresh" ;
    rdfs:comment "Python library for time series" ;
    rdfs:seeAlso <https://www.wikidata.org/entity/Q107384267> .
:tslearn_lib a :ML_library ;
    skos:prefLabel "tslearn" ;
    rdfs:comment "Python package that provides machine learning tools for the analysis of time series. The package builds on scikit-learn, numpy and scipy libraries." ;
    rdfs:seeAlso <https://github.com/tslearn-team/tslearn> .
:weka_lib a :ML_library ;
    skos:prefLabel "Weka" ;
    rdfs:comment "Suite of machine learning software written in Java" ;
    rdfs:seeAlso <https://www.wikidata.org/entity/Q115494> .
:xgboost_lib a :ML_library ;
    skos:prefLabel "XGBoost" ;
    rdfs:comment "Scalable machine learning system for tree boosting" ;
    rdfs:seeAlso <https://www.wikidata.org/entity/Q23793561> .


# AutoML_solution

:adanet a :AutoML_solution ;
    skos:prefLabel "Adanet" ;
    :used_for :tensorflow_lib ;
    :can_perform :tabular_classification , :tabular_regression ;
    rdfs:comment "Lightweight TensorFlow-based framework for automatically learning high-quality models with minimal expert intervention" ;
    rdfs:seeAlso <https://github.com/tensorflow/adanet> .
:alphad3m a :AutoML_solution ;
    skos:prefLabel "Alphad3m" ;
    :used_for :scikit_learn_lib , :pywavelets_lib , :pytorch_lib ;
    :can_perform :tabular_classification , :tabular_regression , :clustering , :time_series_forecasting , :time_series_classification , :text_classification , :text_regression , :image_classification , :object_detection , :video_classification , :audio_classification , :audio_regression , :graph_matching , :vertex_classification , :link_prediction , :community_detection ;
    rdfs:comment "AutoML system that automatically searches for models and derives end-to-end pipelines that read, pre-process the data, and train the model" ;
    rdfs:seeAlso <https://pypi.org/project/alphad3m> .
:analytics_zoo_chronos a :AutoML_solution ;
    skos:prefLabel "Analytics Zoo Chronos" ;
    :used_for :prophet_lib , :tensorflow_lib , :pytorch_lib , :pmdarima_lib ;
    :can_perform :time_series_forecasting ;
    rdfs:comment "Open source Big Data AI platform including the following features for scaling end-to-end AI to distributed Big Data" ;
    rdfs:seeAlso <https://github.com/intel-analytics/analytics-zoo> .
:atm a :AutoML_solution ;
    skos:prefLabel "ATM" ;
    :used_for :scikit_learn_lib ;
    :can_perform :tabular_classification , :tabular_regression ;
    rdfs:comment "AutoML system designed with ease of use in mind" ;
    rdfs:seeAlso <https://github.com/HDI-Project/ATM> .
:auto_timeseries a :AutoML_solution ;
    skos:prefLabel "Auto_TimeSeries" ;
    :used_for :scikit_learn_lib , :pmdarima_lib , :prophet_lib , :pyflux_lib , :statsmodel_lib , :xgboost_lib ;
    :can_perform :time_series_forecasting ;
    rdfs:comment "Complex model building utility for time series data. It will automatically select the best model which gives best score specified." ;
    rdfs:seeAlso <https://github.com/AutoViML/Auto_TS> .
:auto_weka a :AutoML_solution ;
    skos:prefLabel "Auto-Weka" ;
    :used_for :weka_lib ;
    :can_perform :tabular_classification , :tabular_regression , :clustering , :time_series_forecasting ;
    rdfs:comment "AutoML library for WEKA" ;
    rdfs:seeAlso <https://github.com/automl/autoweka> .
:autocve a :AutoML_solution ;
    skos:prefLabel "AutoCVE" ;
    :used_for :xgboost_lib , :scikit_learn_lib ;
    :can_perform :tabular_classification ;
    rdfs:comment "AutoML library" ;
    rdfs:seeAlso <https://github.com/celiolarcher/AUTOCVE> .
:autogluon a :AutoML_solution ;
    skos:prefLabel "Autogluon" ;
    :used_for :scikit_learn_lib , :catboost_lib , :lightgbm_lib , :xgboost_lib , :pytorch_lib , :mxnet_lib ;
    :can_perform :tabular_classification , :tabular_regression , :text_classification , :text_regression , :sentiment_analysis , :sentence_similarity , :image_classification , :object_detection , :video_classification , :video_object_tracking , :action_recognition , :time_series_forecasting , :named_entity_recognition ;
    rdfs:comment "AutoGluon automates machine learning tasks on image, text, time series, and tabular data." ;
    rdfs:seeAlso <https://auto.gluon.ai> ;
    :supported_by_oma_ml "true"^^xsd:boolean .
:autokeras a :AutoML_solution ;
    skos:prefLabel "Autokeras" ;
    :used_for :keras_lib ;
    :can_perform :tabular_classification , :tabular_regression , :time_series_forecasting , :text_classification , :text_regression , :image_classification , :image_regression ;
    rdfs:comment "An AutoML system based on Keras." ;
    rdfs:seeAlso <https://autokeras.com> ;
    :supported_by_oma_ml "true"^^xsd:boolean .
:autopytorch a :AutoML_solution ;
    skos:prefLabel "Autopytorch" ;
    :used_for :pytorch_lib , :pytorch_forecasting_lib ;
    :can_perform :tabular_classification , :tabular_regression , :image_classification , :time_series_forecasting ;
    rdfs:comment "AutoML framework focussing on neural architecture search" ;
    rdfs:seeAlso <https://github.com/automl/Auto-PyTorch> .
:autosklearn a :AutoML_solution ;
    skos:prefLabel "Autosklearn" ;
    :used_for :scikit_learn_lib ;
    :can_perform :tabular_classification , :tabular_regression ;
    rdfs:comment "AutoML library for Scikit-learn" ;
    rdfs:seeAlso <https://automl.github.io/auto-sklearn> .
:autots a :AutoML_solution ;
    skos:prefLabel "AutoTS" ;
    :used_for :prophet_lib , :pytorch_lib , :gluonts_lib , :pmdarima_lib , :tensorflow_lib ;
    :can_perform :time_series_forecasting ;
    rdfs:comment "Time series package for Python designed for rapidly deploying high-accuracy forecasts at scale" ;
    rdfs:seeAlso <https://pypi.org/project/autots> .
:aws_sagemaker_autopilot a :AutoML_solution ;
    skos:prefLabel "AWS Sagemaker Autopilot" ;
    :used_for :scikit_learn_lib , :tsfresh_lib , :gluonts_lib , :xgboost_lib , :fastai_lib ;
    :can_perform :tabular_classification , :tabular_regression , :time_series_classification ;
    rdfs:comment "AutoML solution for AWS Sagemaker" ;
    rdfs:seeAlso <https://aws.amazon.com/de/sagemaker/autopilot> .
:azure_automl a :AutoML_solution ;
    skos:prefLabel "Azure AutoML" ;
    :can_perform :tabular_classification , :tabular_regression , :time_series_forecasting , :text_classification , :image_classification , :object_detection ;
    rdfs:comment "AutoML solution for MS Azure" ;
    rdfs:seeAlso <https://azure.microsoft.com/en-us/products/machine-learning/automatedml> .
:databricks a :AutoML_solution ;
    skos:prefLabel "Databricks" ;
    :used_for :pmdarima_lib , :prophet_lib , :tensorflow_lib , :xgboost_lib ;
    :can_perform :time_series_forecasting ;
    rdfs:comment "Commercial AutoML solution" ;
    rdfs:seeAlso <https://www.databricks.com/de/product/automl> .
:datarobot a :AutoML_solution ;
    skos:prefLabel "DataRobot" ;
    :used_for :pmdarima_lib , :prophet_lib , :tensorflow_lib , :xgboost_lib ;
    :can_perform :time_series_forecasting , :time_series_classification ;
    rdfs:comment "Commercial AutoML solution" ;
    rdfs:seeAlso <https://aws-quickstart.github.io/quickstart-data-robot-automl-platform> .
:evalml a :AutoML_solution ;
    skos:prefLabel "EvalML" ;
    :used_for :scikit_learn_lib , :catboost_lib , :lightgbm_lib , :xgboost_lib ;
    :can_perform :tabular_classification , :tabular_regression , :time_series_forecasting , :time_series_classification , :text_classification , :text_regression ;
    rdfs:comment "EvalML is an AutoML library which builds, optimizes, and evaluates machine learning pipelines using domain-specific objective functions." ;
    rdfs:seeAlso <https://github.com/alteryx/evalml> ;
    :supported_by_oma_ml "true"^^xsd:boolean .
:fedot a :AutoML_solution ;
    skos:prefLabel "FEDOT" ;
    :used_for :scikit_learn_lib , :statsmodel_lib ;
    :can_perform :time_series_forecasting ;
    rdfs:comment "FEDOT is an open-source framework for automated modeling and machine learning (AutoML) problems." ;
    rdfs:seeAlso <https://github.com/aimclub/FEDOT> .
:flaml a :AutoML_solution ;
    skos:prefLabel "FLAML" ;
    :used_for :scikit_learn_lib , :catboost_lib , :lightgbm_lib , :xgboost_lib , :prophet_lib ;
    :can_perform :tabular_classification , :tabular_regression , :ranking , :time_series_forecasting , :text_classification ;
    rdfs:comment "FLAML is a lightweight Python library for efficient automation of machine learning, including selection of models, hyperparameters, and other tunable choices of an application" ;
    rdfs:seeAlso <https://github.com/microsoft/FLAML> ;
    :supported_by_oma_ml "true"^^xsd:boolean .
:gama a :AutoML_solution ;
    skos:prefLabel "GAMA" ;
    :used_for :scikit_learn_lib ;
    :can_perform :tabular_classification , :tabular_regression ;
    rdfs:comment "General Automated Machine learning Assistant: An automated machine learning tool based on genetic programming." ;
    rdfs:seeAlso <https://github.com/openml-labs/gama> ;
    :supported_by_oma_ml "true"^^xsd:boolean .
:google_automl a :AutoML_solution ;
    skos:prefLabel "Google AutoML" ;
    :used_for :tensorflow_lib ;
    :can_perform :tabular_classification , :tabular_regression , :time_series_forecasting ;
    rdfs:comment "A suite of machine learning products that enables developers with limited machine learning expertise to train ML models specific to business needs" ;
    rdfs:seeAlso <https://pypi.org/project/google-cloud-automl> .
:h2o_automl a :AutoML_solution ;
    skos:prefLabel "H2O Automl" ;
    :used_for :h2o_lib , :xgboost_lib ;
    :can_perform :tabular_classification , :tabular_regression ;
    rdfs:comment "H2O's AutoML automates the process of training and tuning a large selection of models, allowing the user to focus on other aspects of the data science and machine learning pipeline such as data pre-processing, feature engineering and model deployment." ;
    rdfs:seeAlso <https://github.com/h2oai> ;
    :supported_by_oma_ml "true"^^xsd:boolean .
:ibm_autoai a :AutoML_solution ;
    skos:prefLabel "IBM AutoAI" ;
    :used_for :ibm_snap_ml_lib , :scikit_learn_lib , :tensorflow_lib , :xgboost_lib ;
    :can_perform :time_series_forecasting ;
    rdfs:comment "Commercial AutoML solution by IBM" ;
    rdfs:seeAlso <https://www.ibm.com/docs/en/cloud-paks/cp-data/4.0?topic=models-autoai> .
:mcfly a :AutoML_solution ;
    skos:prefLabel "Mcfly" ;
    :used_for :tensorflow_lib ;
    :can_perform :time_series_classification ;
    rdfs:comment "AutoML library for time series" ;
    rdfs:seeAlso <https://github.com/NLeSC/mcfly> .
:merlion a :AutoML_solution ;
    skos:prefLabel "Merlion" ;
    :used_for :lightgbm_lib , :prophet_lib , :scikit_learn_lib , :statsmodel_lib , :greykite_lib , :kats_lib ;
    :can_perform :time_series_forecasting ;
    rdfs:comment "A Machine Learning Library for Time Series" ;
    rdfs:seeAlso <https://github.com/salesforce/Merlion> .
:mlbox a :AutoML_solution ;
    skos:prefLabel "MLBOX" ;
    :used_for :keras_lib , :scikit_learn_lib ;
    :can_perform :tabular_classification , :tabular_regression ;
    rdfs:comment "Automated Machine Learning library in Python" ;
    rdfs:seeAlso <https://github.com/AxeldeRomblay/MLBox> .
:mljar a :AutoML_solution ;
    skos:prefLabel "MLJAR" ;
    :used_for :scikit_learn_lib , :catboost_lib , :lightgbm_lib , :xgboost_lib ;
    :can_perform :tabular_classification , :tabular_regression ;
    rdfs:comment "Automated Machine Learning Python package that works with tabular data." ;
    rdfs:seeAlso <https://supervised.mljar.com> ;
    :supported_by_oma_ml "true"^^xsd:boolean .
:pycaret a :AutoML_solution ;
    skos:prefLabel "Pycaret" ;
    :used_for :scikit_learn_lib , :catboost_lib , :lightgbm_lib , :xgboost_lib ;
    :can_perform :tabular_classification , :tabular_regression , :tabular_clustering , :anomaly_detection , :time_series_forecasting ;
    rdfs:comment "Open-source, low-code machine learning library in Python" ;
    rdfs:seeAlso <https://github.com/pycaret/pycaret> ;
    :supported_by_oma_ml "true"^^xsd:boolean .
:rapidminer a :AutoML_solution ;
    skos:prefLabel "Rapidminer" ;
    :used_for :weka_lib , :h2o_lib ;
    :can_perform :tabular_classification , :tabular_regression , :clustering , :anomaly_detection , :time_series_forecasting ;
    rdfs:comment "Commercial data science platform with AutoModel feature" ;
    rdfs:seeAlso <https://rapidminer.com> .
:remi_ai a :AutoML_solution ;
    skos:prefLabel "Remi AI" ;
    :can_perform :time_series_forecasting ;
    rdfs:comment "Commercial data science platform with AutoML feature" ;
    rdfs:seeAlso <https://www.remi.ai> .
:tpot a :AutoML_solution ;
    skos:prefLabel "TPOT" ;
    :used_for :scikit_learn_lib , :pytorch_lib ;
    :can_perform :tabular_classification , :tabular_regression , :image_classification ;
    rdfs:comment "AutoML library for Scikit-learn" ;
    rdfs:seeAlso <http://automl.info/tpot> ;
    :supported_by_oma_ml "true"^^xsd:boolean .
:transmogrifai a :AutoML_solution ;
    skos:prefLabel "TransmogrifAI" ;
    :used_for :mllib_lib ;
    :can_perform :tabular_classification , :tabular_regression ;
    rdfs:comment "End-to-end AutoML library for structured data written in Scala that runs on top of Apache Spark" ;
    rdfs:seeAlso <https://transmogrif.ai> .
:lama a :AutoML_solution ;
    skos:prefLabel "LAMA" ;
    :used_for :pytorch_lib , :lightgbm_lib , :scikit_learn_lib , :catboost_lib ;
    :can_perform :tabular_classification , :tabular_regression , :binary_classification ;
    rdfs:comment "LightAutoML - automatic model creation framework" ;
    rdfs:seeAlso <https://github.com/sb-ai-lab/LightAutoML> ;
    :supported_by_oma_ml "true"^^xsd:boolean .


# Configuration_item

:tabular_classification_in_autokeras a :Configuration_item ;
    skos:prefLabel "tabular classification in AutoKeras" ;
    :category :task_configuration ;
    :automl_solution :autokeras ;
    :ml_task :tabular_classification ;
    :parameter_value :metric_autokeras_tabular_classification , :loss_function_autokeras_tabular_classification , :max_trials_autokeras_tabular_classification , :tuner_autokeras_tabular_classification , :max_model_size_autokeras_tabular_classification ;
    rdfs:comment "Task configuration for tabular classification in AutoKeras" ;
    rdfs:seeAlso <https://autokeras.com> .
:tabular_regression_in_autokeras a :Configuration_item ;
    skos:prefLabel "tabular regression in AutoKeras" ;
    :category :task_configuration ;
    :automl_solution :autokeras ;
    :ml_task :tabular_regression ;
    :parameter_value :metric_autokeras_tabular_regression , :loss_function_autokeras_tabular_regression , :max_trials_autokeras_tabular_regression , :tuner_autokeras_tabular_regression , :max_model_size_autokeras_tabular_regression ;
    rdfs:comment "Task configuration for tabular regression in AutoKeras" ;
    rdfs:seeAlso <https://autokeras.com> .
:image_classification_in_autokeras a :Configuration_item ;
    skos:prefLabel "image classification in AutoKeras" ;
    :category :task_configuration ;
    :automl_solution :autokeras ;
    :ml_task :image_classification ;
    :parameter_value :metric_autokeras_image_classification , :loss_function_autokeras_image_classification , :max_trials_autokeras_image_classification , :tuner_autokeras_image_classification , :max_model_size_autokeras_image_classification ;
    rdfs:comment "Task configuration for image classification in AutoKeras" ;
    rdfs:seeAlso <https://autokeras.com> .
:image_regression_in_autokeras a :Configuration_item ;
    skos:prefLabel "image regression in AutoKeras" ;
    :category :task_configuration ;
    :automl_solution :autokeras ;
    :ml_task :image_regression ;
    :parameter_value :metric_autokeras_image_regression , :loss_function_autokeras_image_regression , :max_trials_autokeras_image_regression , :tuner_autokeras_image_regression , :max_model_size_autokeras_image_regression ;
    rdfs:comment "Task configuration for image regression in AutoKeras" ;
    rdfs:seeAlso <https://autokeras.com> .
:text_classification_in_autokeras a :Configuration_item ;
    skos:prefLabel "text classification in AutoKeras" ;
    :category :task_configuration ;
    :automl_solution :autokeras ;
    :ml_task :text_classification ;
    :parameter_value :metric_autokeras_text_classification , :loss_function_autokeras_text_classification , :max_trials_autokeras_text_classification , :tuner_autokeras_text_classification , :max_model_size_autokeras_text_classification ;
    rdfs:comment "Task configuration for text classification in AutoKeras" ;
    rdfs:seeAlso <https://autokeras.com> .
:text_regression_in_autokeras a :Configuration_item ;
    skos:prefLabel "text regression in AutoKeras" ;
    :category :task_configuration ;
    :automl_solution :autokeras ;
    :ml_task :text_regression ;
    :parameter_value :metric_autokeras_text_regression , :loss_function_autokeras_text_regression , :max_trials_autokeras_text_regression , :tuner_autokeras_text_regression , :max_model_size_autokeras_text_regression ;
    rdfs:comment "Task configuration for text regression in AutoKeras" ;
    rdfs:seeAlso <https://autokeras.com> .
:time_series_forecasting_in_autokeras a :Configuration_item ;
    skos:prefLabel "time series forecasting in AutoKeras" ;
    :category :task_configuration ;
    :automl_solution :autokeras ;
    :ml_task :time_series_forecasting ;
    :parameter_value :metric_autokeras_time_series_forecasting , :loss_function_autokeras_time_series_forecasting , :max_trials_autokeras_time_series_forecasting , :tuner_autokeras_time_series_forecasting , :max_model_size_autokeras_time_series_forecasting , :lookback_autokeras_time_series_forecasting , :gap_autokeras_time_series_forecasting , :forecasting_horizon_autokeras_time_series_forcasting ;
    rdfs:comment "Task configuration for time series forecasting in AutoKeras" ;
    rdfs:seeAlso <https://autokeras.com> .
:tabular_classification_in_autosklearn a :Configuration_item ;
    skos:prefLabel "tabular classification in Autosklearn" ;
    :category :task_configuration ;
    :automl_solution :autosklearn ;
    :ml_task :tabular_classification ;
    :parameter_value :time_limit_autosklearn_tabular_classification , :time_limit_per_run_autosklearn_tabular_classification , :ensemble_size_autosklearn_tabular_classification , :ensemble_nbest_autosklearn_tabular_classification , :metric_autosklearn_tabular_classification , :use_approach_autosklearn_tabular_classification , :include_preprocessor_autosklearn_tabular_classification ;
    rdfs:comment "Task configuration for tabular classification in Autosklearn" ;
    rdfs:seeAlso <https://automl.github.io/auto-sklearn/master/api.html#classification> .
:tabular_regression_in_autosklearn a :Configuration_item ;
    skos:prefLabel "tabular regression in Autosklearn" ;
    :category :task_configuration ;
    :automl_solution :autosklearn ;
    :ml_task :tabular_regression ;
    :parameter_value :time_limit_autosklearn_tabular_regression , :time_limit_per_run_autosklearn_tabular_regression , :ensemble_size_autosklearn_tabular_regression , :ensemble_nbest_autosklearn_tabular_regression , :metric_autosklearn_tabular_regression , :use_approach_autosklearn_tabular_regression , :include_preprocessor_autosklearn_tabular_regression ;
    rdfs:comment "Task configuration for tabular regression in Autosklearn" ;
    rdfs:seeAlso <https://automl.github.io/auto-sklearn/master/api.html#regression> .
:tabular_classification_in_flaml a :Configuration_item ;
    skos:prefLabel "tabular classification in FLAML" ;
    :category :task_configuration ;
    :automl_solution :flaml ;
    :ml_task :tabular_classification ;
    :parameter_value :use_approach_flaml_tabular_classification , :metric_flaml_tabular_classification , :ensemble_flaml_tabular_classification , :eval_method_flaml , :validation_split_flaml , :cross_validation_fold_flaml , :split_type_flaml_classification , :hyperparameter_optimization_method_flaml ;
    rdfs:comment "Task configuration for tabular classification in FLAML" ;
    rdfs:seeAlso <https://microsoft.github.io/FLAML/docs/reference/automl/automl> .
:tabular_regression_in_flaml a :Configuration_item ;
    skos:prefLabel "tabular regression in FLAML" ;
    :category :task_configuration ;
    :automl_solution :flaml ;
    :ml_task :tabular_regression ;
    :parameter_value :use_approach_flaml_tabular_regression , :metric_flaml_tabular_regression , :ensemble_flaml_tabular_regression , :eval_method_flaml , :validation_split_flaml , :cross_validation_fold_flaml , :split_type_flaml_regression , :hyperparameter_optimization_method_flaml ;
    rdfs:comment "Task configuration for tabular regression in FLAML" ;
    rdfs:seeAlso <https://microsoft.github.io/FLAML/docs/reference/automl/automl> .
:time_series_forecasting_in_flaml a :Configuration_item ;
    skos:prefLabel "time series forecasting in FLAML" ;
    :category :task_configuration ;
    :automl_solution :flaml ;
    :ml_task :time_series_forecasting ;
    :parameter_value :use_approach_flaml_time_series_analysis , :metric_flaml_time_series_analysis , :ensemble_flaml_time_series_forecasting , :eval_method_flaml , :forecasting_horizon_flaml_time_series_forcasting , :validation_split_flaml , :cross_validation_fold_flaml , :split_type_flaml_time_series_forecasting , :hyperparameter_optimization_method_flaml ;
    rdfs:comment "Task configuration for time series forecasting in FLAML" ;
    rdfs:seeAlso <https://microsoft.github.io/FLAML/docs/reference/automl/automl> .
:text_classification_in_flaml a :Configuration_item ;
    skos:prefLabel "text classification in FLAML" ;
    :category :task_configuration ;
    :automl_solution :flaml ;
    :ml_task :text_classification ;
    :parameter_value :use_approach_flaml_text_classification , :metric_flaml_text_classification , :ensemble_flaml_text_classification , :eval_method_flaml , :validation_split_flaml , :cross_validation_fold_flaml , :split_type_flaml_classification , :hyperparameter_optimization_method_flaml ;
    rdfs:comment "Task configuration for text classification in FLAML" ;
    rdfs:seeAlso <https://microsoft.github.io/FLAML/docs/reference/automl/automl> .
:ranking_in_flaml a :Configuration_item ;
    skos:prefLabel "ranking in FLAML" ;
    :category :task_configuration ;
    :automl_solution :flaml ;
    :ml_task :ranking ;
    :parameter_value :use_approach_flaml_ranking , :metric_flaml_ranking , :ensemble_flaml_ranking , :eval_method_flaml , :validation_split_flaml , :cross_validation_fold_flaml , :split_type_flaml_ranking , :hyperparameter_optimization_method_flaml ;
    rdfs:comment "Task configuration for ranking in FLAML" ;
    rdfs:seeAlso <https://microsoft.github.io/FLAML/docs/reference/automl/automl> .
:text_regression_in_flaml a :Configuration_item ;
    skos:prefLabel "text regression in FLAML" ;
    :category :task_configuration ;
    :automl_solution :flaml ;
    :ml_task :text_regression ;
    :parameter_value :use_approach_flaml_text_regression , :metric_flaml_text_regression , :ensemble_flaml_text_regression , :eval_method_flaml , :validation_split_flaml , :cross_validation_fold_flaml , :split_type_flaml_regression , :hyperparameter_optimization_method_flaml ;
    rdfs:comment "Task configuration for text regression in FLAML" ;
    rdfs:seeAlso <https://microsoft.github.io/FLAML/docs/reference/automl/automl> .
:tabular_classification_in_evalml a :Configuration_item ;
    skos:prefLabel "tabular classification in EvalML" ;
    :category :task_configuration ;
    :automl_solution :evalml ;
    :ml_task :tabular_classification ;
    :parameter_value :use_approach_evalml_tabular_classification , :metric_evalml_tabular_classification , :tuner_class_evalml , :optimize_thresholds_evalml , :ensembling_evalml , :max_batches_evalml , :allow_long_running_models_evalml , :pipelines_per_batch_evalml , :exclude_featurizers_evalml ;
    rdfs:comment "Task configuration for tabular classification in EvalML" ;
    rdfs:seeAlso <https://evalml.alteryx.com/en/stable/api_index.html> .
:tabular_regression_in_evalml a :Configuration_item ;
    skos:prefLabel "tabular regression in EvalML" ;
    :category :task_configuration ;
    :automl_solution :evalml ;
    :ml_task :tabular_regression ;
    :parameter_value :use_approach_evalml_tabular_regression , :metric_evalml_tabular_regression , :tuner_class_evalml , :optimize_thresholds_evalml , :ensembling_evalml , :max_batches_evalml , :allow_long_running_models_evalml , :pipelines_per_batch_evalml , :exclude_featurizers_evalml ;
    rdfs:comment "Task configuration for tabular regression in EvalML" ;
    rdfs:seeAlso <https://evalml.alteryx.com/en/stable/api_index.html> .
:time_series_regression_in_evalml a :Configuration_item ;
    skos:prefLabel "time series regression in EvalML" ;
    :category :task_configuration ;
    :automl_solution :evalml ;
    :ml_task :time_series_forecasting ;
    :parameter_value :use_approach_evalml_time_series_regression , :metric_evalml_time_series_regression , :tuner_class_evalml , :forecasting_horizon_evalml_time_series_forcasting , :lookback_evalml_time_series_forecasting , :gap_evalml_time_series_forecasting , :optimize_thresholds_evalml , :ensembling_evalml , :max_batches_evalml , :allow_long_running_models_evalml , :pipelines_per_batch_evalml , :exclude_featurizers_evalml ;
    rdfs:comment "Task configuration for time series regression in EvalML" ;
    rdfs:seeAlso <https://evalml.alteryx.com/en/stable/api_index.html> .
:time_series_classification_in_evalml a :Configuration_item ;
    skos:prefLabel "time series classification in EvalML" ;
    :category :task_configuration ;
    :automl_solution :evalml ;
    :ml_task :time_series_classification ;
    :parameter_value :use_approach_evalml_time_series_classification , :tuner_class_evalml , :optimize_thresholds_evalml , :ensembling_evalml , :max_batches_evalml , :allow_long_running_models_evalml , :pipelines_per_batch_evalml , :exclude_featurizers_evalml ;
    rdfs:comment "Task configuration for time series classification in EvalML" ;
    rdfs:seeAlso <https://evalml.alteryx.com/en/stable/api_index.html> .
:text_classification_in_evalml a :Configuration_item ;
    skos:prefLabel "text classification in EvalML" ;
    :category :task_configuration ;
    :automl_solution :evalml ;
    :ml_task :text_classification ;
    :parameter_value :use_approach_evalml_text_classification , :metric_evalml_text_classification , :tuner_class_evalml , :optimize_thresholds_evalml , :ensembling_evalml , :max_batches_evalml , :allow_long_running_models_evalml , :pipelines_per_batch_evalml , :exclude_featurizers_evalml ;
    rdfs:comment "Task configuration for text classification in EvalML" ;
    rdfs:seeAlso <https://evalml.alteryx.com/en/stable/api_index.html> .
:text_regression_in_evalml a :Configuration_item ;
    skos:prefLabel "text regression in EvalML" ;
    :category :task_configuration ;
    :automl_solution :evalml ;
    :ml_task :text_regression ;
    :parameter_value :use_approach_evalml_text_regression , :metric_evalml_text_regression , :tuner_class_evalml , :optimize_thresholds_evalml , :ensembling_evalml , :max_batches_evalml , :allow_long_running_models_evalml , :pipelines_per_batch_evalml , :exclude_featurizers_evalml ;
    rdfs:comment "Task configuration for text regression in EvalML" ;
    rdfs:seeAlso <https://evalml.alteryx.com/en/stable/api_index.html> .
:tabular_classification_pycaret a :Configuration_item ;
    skos:prefLabel "tabular classification PyCaret" ;
    :category :task_configuration ;
    :automl_solution :pycaret ;
    :ml_task :tabular_classification ;
    :parameter_value :metric_pycaret_tabular_classification , :cross_validation_fold_pycaret ;
    rdfs:comment "Task configuration for tabular classification PyCaret" ;
    rdfs:seeAlso <https://pycaret.readthedocs.io> .
:tabular_regression_pycaret a :Configuration_item ;
    skos:prefLabel "tabular regression PyCaret" ;
    :category :task_configuration ;
    :automl_solution :pycaret ;
    :ml_task :tabular_regression ;
    :parameter_value :metric_pycaret_tabular_regression , :cross_validation_fold_pycaret ;
    rdfs:comment "Task configuration for tabular regression PyCaret" ;
    rdfs:seeAlso <https://pycaret.readthedocs.io> .
:time_series_forecasting__pycaret a :Configuration_item ;
    skos:prefLabel "time series forecasting  PyCaret" ;
    :category :task_configuration ;
    :automl_solution :pycaret ;
    :ml_task :time_series_forecasting ;
    :parameter_value :metric_pycaret_time_series_forecasting , :forecasting_horizon_pycaret_time_series_forcasting , :cross_validation_fold_pycaret ;
    rdfs:comment "Task configuration for time series forecasting  PyCaret" ;
    rdfs:seeAlso <https://pycaret.readthedocs.io> .
:clustering_pycaret a :Configuration_item ;
    skos:prefLabel "clustering PyCaret" ;
    :category :task_configuration ;
    :automl_solution :pycaret ;
    :ml_task :tabular_clustering ;
    :parameter_value :include_approach_pycaret_clustering ;
    rdfs:comment "Task configuration for clustering" ;
    rdfs:seeAlso <https://pycaret.readthedocs.io> .
:tabular_classification_in_autogluon a :Configuration_item ;
    skos:prefLabel "tabular classification in AutoGluon" ;
    :category :task_configuration ;
    :automl_solution :autogluon ;
    :ml_task :tabular_classification ;
    :parameter_value :use_approach_autogluon_classification , :metric_autogluon_tabular_classification ;
    rdfs:comment "Task configuration for tabular classification in AutoGluon" ;
    rdfs:seeAlso <https://auto.gluon.ai> .
:tabular_regression_in_autogluon a :Configuration_item ;
    skos:prefLabel "tabular regression in AutoGluon" ;
    :category :task_configuration ;
    :automl_solution :autogluon ;
    :ml_task :tabular_regression ;
    :parameter_value :use_approach_autogluon_regression , :metric_autogluon_tabular_regression ;
    rdfs:comment "Task configuration for tabular regression in AutoGluon" ;
    rdfs:seeAlso <https://auto.gluon.ai> .
:time_series_forecasting_in_autogluon a :Configuration_item ;
    skos:prefLabel "time series forecasting in AutoGluon" ;
    :category :task_configuration ;
    :automl_solution :autogluon ;
    :ml_task :time_series_forecasting ;
    :parameter_value :metric_autogluon_time_series_forecasting , :forecasting_horizon_autogluon_time_series_forcasting ;
    rdfs:comment "Task configuration for time series forecasting in AutoGluon" ;
    rdfs:seeAlso <https://auto.gluon.ai> .
:image_classification_in_autogluon a :Configuration_item ;
    skos:prefLabel "image classification in AutoGluon" ;
    :category :task_configuration ;
    :automl_solution :autogluon ;
    :ml_task :image_classification ;
    :parameter_value :use_approach_autogluon_image_classification , :metric_autogluon_image_classification ;
    rdfs:comment "Task configuration for image classification in AutoGluon" ;
    rdfs:seeAlso <https://auto.gluon.ai> .
:object_detection_in_autogluon a :Configuration_item ;
    skos:prefLabel "object detection in AutoGluon" ;
    :category :task_configuration ;
    :automl_solution :autogluon ;
    :ml_task :object_detection ;
    :parameter_value :use_approach_autogluon_object_detection ;
    rdfs:comment "Task configuration for object detection in AutoGluon" ;
    rdfs:seeAlso <https://auto.gluon.ai> .
:text_classification_in_autogluon a :Configuration_item ;
    skos:prefLabel "text classification in AutoGluon" ;
    :category :task_configuration ;
    :automl_solution :autogluon ;
    :ml_task :text_classification ;
    :parameter_value :use_approach_autogluon_text_classification , :metric_autogluon_text_classification ;
    rdfs:comment "Task configuration for text classification in AutoGluon" ;
    rdfs:seeAlso <https://auto.gluon.ai> .
:named_entity_recognition_in_autogluon a :Configuration_item ;
    skos:prefLabel "named entity recognition in AutoGluon" ;
    :category :task_configuration ;
    :automl_solution :autogluon ;
    :ml_task :named_entity_recognition ;
    :parameter_value :use_approach_autogluon_named_entity_recognition , :metric_autogluon_named_entity_recognition ;
    rdfs:comment "Task configuration for named entity recognition in AutoGluon" ;
    rdfs:seeAlso <https://auto.gluon.ai> .
:text_regression_in_autogluon a :Configuration_item ;
    skos:prefLabel "text regression in AutoGluon" ;
    :category :task_configuration ;
    :automl_solution :autogluon ;
    :ml_task :text_regression ;
    :parameter_value :use_approach_autogluon_text_regression , :metric_autogluon_text_regression ;
    rdfs:comment "Task configuration for text regression in AutoGluon" ;
    rdfs:seeAlso <https://auto.gluon.ai> .
:time_series_classification_in_mcfly a :Configuration_item ;
    skos:prefLabel "time series classification in mcfly" ;
    :category :task_configuration ;
    :automl_solution :mcfly ;
    :ml_task :time_series_classification ;
    :parameter_value :use_approach_mcfly_time_series_classification , :metric_mcfly_time_series_classification , :epochs_mcfly ;
    rdfs:comment "Task configuration for time series classification in mcfly" ;
    rdfs:seeAlso <https://mcfly.readthedocs.io/en/latest/reference.html> .
:tabular_classification_in_auto_pytorch a :Configuration_item ;
    skos:prefLabel "tabular classification in Auto-PyTorch" ;
    :category :task_configuration ;
    :automl_solution :autopytorch ;
    :ml_task :tabular_classification ;
    :parameter_value :use_approach_auto_pytorch_classification , :metric_autopytorch_tabular_classification ;
    rdfs:comment "Task configuration for tabular classification in Auto-PyTorch" ;
    rdfs:seeAlso <https://automl.github.io/Auto-PyTorch/development/api.html> .
:tabular_regression_in_auto_pytorch a :Configuration_item ;
    skos:prefLabel "tabular regression in Auto-PyTorch" ;
    :category :task_configuration ;
    :automl_solution :autopytorch ;
    :ml_task :tabular_regression ;
    :parameter_value :use_approach_auto_pytorch_regression , :metric_autopytorch_tabular_regression ;
    rdfs:comment "Task configuration for tabular regression in Auto-PyTorch" ;
    rdfs:seeAlso <https://automl.github.io/Auto-PyTorch/development/api.html> .
:time_series_forecasting_in_auto_pytorch a :Configuration_item ;
    skos:prefLabel "time series forecasting in Auto-PyTorch" ;
    :category :task_configuration ;
    :automl_solution :autopytorch ;
    :ml_task :time_series_forecasting ;
    :parameter_value :metric_autopytorch_time_series_forecasting , :forecasting_horizon_autopytorch_time_series_forcasting ;
    rdfs:comment "Task configuration for time series forecasting in Auto-PyTorch" ;
    rdfs:seeAlso <https://automl.github.io/Auto-PyTorch/development/api.html> .
:tabular_classification_mljar a :Configuration_item ;
    skos:prefLabel "tabular classification MLJAR" ;
    :category :task_configuration ;
    :automl_solution :mljar ;
    :ml_task :tabular_classification ;
    :parameter_value :metric_mljar_tabular_classification ;
    rdfs:comment "Task configuration for tabular classification MLJAR" ;
    rdfs:seeAlso <https://supervised.mljar.com/api> .
:tabular_regression_mljar a :Configuration_item ;
    skos:prefLabel "tabular regression MLJAR" ;
    :category :task_configuration ;
    :automl_solution :mljar ;
    :ml_task :tabular_regression ;
    :parameter_value :metric_mljar_tabular_regression ;
    rdfs:comment "Task configuration for tabular regression MLJAR" ;
    rdfs:seeAlso <https://supervised.mljar.com/api> .
:tabular_classification_tpot a :Configuration_item ;
    skos:prefLabel "tabular classification TPOT" ;
    :category :task_configuration ;
    :automl_solution :tpot ;
    :ml_task :tabular_classification ;
    :parameter_value :metric_tpot_tabular_classification ;
    rdfs:comment "Task configuration for tabular classification TPOT" ;
    rdfs:seeAlso <http://epistasislab.github.io/tpot/api> .
:tabular_regression_tpot a :Configuration_item ;
    skos:prefLabel "tabular regression TPOT" ;
    :category :task_configuration ;
    :automl_solution :tpot ;
    :ml_task :tabular_regression ;
    :parameter_value :metric_tpot_tabular_regression ;
    rdfs:comment "Task configuration for tabular regression TPOT" ;
    rdfs:seeAlso <http://epistasislab.github.io/tpot/api> .
:image_classification_tpot a :Configuration_item ;
    skos:prefLabel "image classification TPOT" ;
    :category :task_configuration ;
    :automl_solution :tpot ;
    :ml_task :image_classification ;
    :parameter_value :metric_tpot_image_classification ;
    rdfs:comment "Task configuration for image classification TPOT" ;
    rdfs:seeAlso <http://epistasislab.github.io/tpot/api> .
:tabular_classification_in_autocve a :Configuration_item ;
    skos:prefLabel "tabular classification in AutoCVE" ;
    :category :task_configuration ;
    :automl_solution :autocve ;
    :ml_task :tabular_classification ;
    :parameter_value :use_approach_autocve_classification , :metric_autocve_classification ;
    rdfs:comment "Task configuration for tabular classification in AutoCVE" ;
    rdfs:seeAlso <https://github.com/celiolarcher/AUTOCVE> .
:tabular_classification_in_gama a :Configuration_item ;
    skos:prefLabel "tabular classification in GAMA" ;
    :category :task_configuration ;
    :automl_solution :gama ;
    :ml_task :tabular_classification ;
    :parameter_value :tuner_class_gama , :metric_gama_tabular_classification ;
    rdfs:comment "Task configuration for tabular classification in GAMA" ;
    rdfs:seeAlso <https://openml-labs.github.io/gama/master/api/index.html> .
:tabular_regression_in_gama a :Configuration_item ;
    skos:prefLabel "tabular regression in GAMA" ;
    :category :task_configuration ;
    :automl_solution :gama ;
    :ml_task :tabular_regression ;
    :parameter_value :tuner_class_gama , :metric_gama_tabular_regression ;
    rdfs:comment "Task configuration for tabular regression in GAMA" ;
    rdfs:seeAlso <https://openml-labs.github.io/gama/master/api/index.html> .
:tabular_classification_in_lama a :Configuration_item ;
    skos:prefLabel "tabular classification in LAMA" ;
    :category :task_configuration ;
    :automl_solution :lama ;
    :ml_task :tabular_classification ;
    :parameter_value :loss_function_lama_tabular_classification , :metric_lama_tabular_classification ;
    rdfs:comment "Task configuration for tabular classification in LAMA" ;
    rdfs:seeAlso <https://openml-labs.github.io/gama/master/api/index.html> .
:binary_classification_in_lama a :Configuration_item ;
    skos:prefLabel "binary classification in LAMA" ;
    :category :task_configuration ;
    :automl_solution :lama ;
    :ml_task :binary_classification ;
    :parameter_value :loss_function_lama_binary_classification , :metric_lama_binary_classification ;
    rdfs:comment "Task configuration for binary classification in LAMA" ;
    rdfs:seeAlso <https://openml-labs.github.io/gama/master/api/index.html> .
:tabular_regression_in_lama a :Configuration_item ;
    skos:prefLabel "tabular regression in LAMA" ;
    :category :task_configuration ;
    :automl_solution :lama ;
    :ml_task :tabular_regression ;
    :parameter_value :loss_function_lama_tabular_regression , :metric_lama_tabular_regression ;
    rdfs:comment "Task configuration for tabular regression in LAMA" ;
    rdfs:seeAlso <https://openml-labs.github.io/gama/master/api/index.html> .
:tabular_classification_in_h2o_automl a :Configuration_item ;
    skos:prefLabel "tabular classification in H2O AutoML" ;
    :category :task_configuration ;
    :automl_solution :h2o_automl ;
    :ml_task :tabular_classification ;
    :parameter_value :metric_h2o_automl_tabular_classification , :include_approach_h2o_automl , :max_models_h2o_automl , :sort_metric_h2o_automl ;
    rdfs:comment "Task configuration for tabular classification in H2O AutoML" .
:tabular_regression_in_h2o_automl a :Configuration_item ;
    skos:prefLabel "tabular regression in H2O AutoML" ;
    :category :task_configuration ;
    :automl_solution :h2o_automl ;
    :ml_task :tabular_regression ;
    :parameter_value :metric_h2o_automl_tabular_regression , :include_approach_h2o_automl , :max_models_h2o_automl , :sort_metric_h2o_automl ;
    rdfs:comment "Task configuration for tabular regression in H2O AutoML" .
:ensemble a :Configuration_item ;
    skos:prefLabel "ensemble" ;
    :category :parameter ;
    :has_datatype :boolean .
:ensemble_flaml_tabular_classification a :Configuration_item ;
    skos:prefLabel "ensemble flaml tabular classification" ;
    :category :parameter ;
    skos:broader :ensemble ;
    :has_datatype :boolean .
:ensemble_flaml_tabular_regression a :Configuration_item ;
    skos:prefLabel "ensemble flaml tabular regression" ;
    :category :parameter ;
    skos:broader :ensemble ;
    :has_datatype :boolean .
:ensemble_flaml_time_series_forecasting a :Configuration_item ;
    skos:prefLabel "ensemble flaml time series forecasting" ;
    :category :parameter ;
    skos:broader :ensemble ;
    :has_datatype :boolean .
:ensemble_flaml_text_classification a :Configuration_item ;
    skos:prefLabel "ensemble flaml text classification" ;
    :category :parameter ;
    skos:broader :ensemble ;
    :has_datatype :boolean .
:ensemble_flaml_text_regression a :Configuration_item ;
    skos:prefLabel "ensemble flaml text regression" ;
    :category :parameter ;
    skos:broader :ensemble ;
    :has_datatype :boolean .
:ensemble_flaml_ranking a :Configuration_item ;
    skos:prefLabel "ensemble flaml ranking" ;
    :category :parameter ;
    skos:broader :ensemble ;
    :has_datatype :boolean .
:ensemble_nbest a :Configuration_item ;
    skos:prefLabel "ensemble_nbest" ;
    :category :parameter ;
    :has_datatype :integer ;
    rdfs:comment "Restricting the number of ensemble models" .
:ensemble_nbest_autosklearn_tabular_classification a :Configuration_item ;
    skos:prefLabel "ensemble nbest autosklearn tabular classification" ;
    :category :parameter ;
    skos:broader :ensemble_nbest ;
    :has_datatype :integer ;
    rdfs:comment "Restricting the number of ensemble models" ;
    rdfs:seeAlso <https://automl.github.io/auto-sklearn/master/api.html#> .
:ensemble_nbest_autosklearn_tabular_regression a :Configuration_item ;
    skos:prefLabel "ensemble nbest autosklearn tabular regression" ;
    :category :parameter ;
    skos:broader :ensemble_nbest ;
    :has_datatype :integer ;
    rdfs:comment "Restricting the number of ensemble models" ;
    rdfs:seeAlso <https://automl.github.io/auto-sklearn/master/api.html#> .
:ensemble_size a :Configuration_item ;
    skos:prefLabel "ensemble size" ;
    :category :parameter ;
    :has_datatype :integer ;
    rdfs:comment "Restricting the size of ensemble models" .
:ensemble_size_autosklearn_tabular_classification a :Configuration_item ;
    skos:prefLabel "ensemble size autosklearn tabular classification" ;
    :category :parameter ;
    skos:broader :ensemble_size ;
    :has_datatype :integer ;
    rdfs:comment "Restricting the size of ensemble models" ;
    rdfs:seeAlso <https://automl.github.io/auto-sklearn/master/api.html#> .
:ensemble_size_autosklearn_tabular_regression a :Configuration_item ;
    skos:prefLabel "ensemble size autosklearn tabular regression" ;
    :category :parameter ;
    skos:broader :ensemble_size ;
    :has_datatype :integer ;
    rdfs:comment "Restricting the size of ensemble models" ;
    rdfs:seeAlso <https://automl.github.io/auto-sklearn/master/api.html#> .
:use_approach a :Configuration_item ;
    skos:prefLabel "use approach" ;
    :category :parameter ;
    rdfs:comment "Selecting ML approaches to be used for AutoML" .
:use_approach_autosklearn_tabular_classification a :Configuration_item ;
    skos:prefLabel "use approach Autosklearn tabular classification" ;
    :category :parameter ;
    skos:broader :use_approach ;
    :has_datatype :list ;
    :parameter_value :adaboost , :decision_tree , :extra_tree , :gradient_boosting_tree , :k_nearest_neighbor , :linear_svm , :multilayer_perceptron , :random_forest , :gaussian_naives_bayes ;
    rdfs:comment "Selecting ML approaches to be used for AutoML" ;
    rdfs:seeAlso <https://automl.github.io/auto-sklearn/master/api.html#classification> .
:use_approach_autosklearn_tabular_regression a :Configuration_item ;
    skos:prefLabel "use approach Autosklearn tabular regression" ;
    :category :parameter ;
    skos:broader :use_approach ;
    :has_datatype :list ;
    :parameter_value :adaboost , :bayesian_linear_regression , :decision_tree , :extra_tree , :gaussian_process , :gradient_boosting_tree , :k_nearest_neighbor , :linear_svm , :multilayer_perceptron , :random_forest ;
    rdfs:comment "Selecting ML approaches to be used for AutoML" ;
    rdfs:seeAlso <https://automl.github.io/auto-sklearn/master/api.html#regression> .
:use_approach_flaml_tabular_classification a :Configuration_item ;
    skos:prefLabel "use approach FLAML tabular classification" ;
    :category :parameter ;
    skos:broader :use_approach ;
    :has_datatype :list ;
    :parameter_value :light_gradient_boosting_machine , :xgboost , :random_forest , :extra_tree , :logistic_regression , :catboost , :k_nearest_neighbor ;
    rdfs:comment "Selecting ML approaches to be used for AutoML" ;
    rdfs:seeAlso <https://microsoft.github.io/FLAML/docs/reference/automl/automl> .
:use_approach_flaml_tabular_regression a :Configuration_item ;
    skos:prefLabel "use approach FLAML tabular regression" ;
    :category :parameter ;
    skos:broader :use_approach ;
    :has_datatype :list ;
    :parameter_value :light_gradient_boosting_machine , :xgboost , :random_forest , :extra_tree , :logistic_regression , :catboost , :k_nearest_neighbor ;
    rdfs:comment "Selecting ML approaches to be used for AutoML" ;
    rdfs:seeAlso <https://microsoft.github.io/FLAML/docs/reference/automl/automl> .
:use_approach_flaml_time_series_analysis a :Configuration_item ;
    skos:prefLabel "use approach FLAML time series analysis" ;
    :category :parameter ;
    skos:broader :use_approach ;
    :has_datatype :list ;
    :parameter_value :light_gradient_boosting_machine , :xgboost , :random_forest , :extra_tree , :prophet , :autoregressive_integrated_moving_average , :seasonal_autoregressive_integrated_moving_average_exogenous ;
    rdfs:comment "Selecting ML approaches to be used for AutoML" ;
    rdfs:seeAlso <https://microsoft.github.io/FLAML/docs/reference/automl/automl> .
:use_approach_flaml_ranking a :Configuration_item ;
    skos:prefLabel "use approach FLAML ranking" ;
    :category :parameter ;
    skos:broader :use_approach ;
    :parameter_value :light_gradient_boosting_machine , :xgboost ;
    rdfs:comment "Selecting ML approaches to be used for AutoML" ;
    rdfs:seeAlso <https://microsoft.github.io/FLAML/docs/reference/automl/automl> .
:use_approach_flaml_text_classification a :Configuration_item ;
    skos:prefLabel "use approach FLAML text classification" ;
    :category :parameter ;
    skos:broader :use_approach ;
    :has_datatype :list ;
    :parameter_value :transformer ;
    rdfs:comment "Selecting ML approaches to be used for AutoML" ;
    rdfs:seeAlso <https://microsoft.github.io/FLAML/docs/reference/automl/automl> .
:use_approach_flaml_text_regression a :Configuration_item ;
    skos:prefLabel "use approach FLAML text regression" ;
    :category :parameter ;
    skos:broader :use_approach ;
    :has_datatype :list ;
    :parameter_value :transformer ;
    rdfs:comment "Selecting ML approaches to be used for AutoML" ;
    rdfs:seeAlso <https://microsoft.github.io/FLAML/docs/reference/automl/automl> .
:use_approach_evalml_tabular_classification a :Configuration_item ;
    skos:prefLabel "use approach EvalML tabular classification" ;
    :category :parameter ;
    skos:broader :use_approach ;
    :has_datatype :list ;
    :parameter_value :catboost , :decision_tree , :extra_tree , :light_gradient_boosting_machine , :linear_regression , :random_forest , :xgboost ;
    rdfs:comment "Selecting ML approaches to be used for AutoML" ;
    rdfs:seeAlso <https://evalml.alteryx.com/en/stable/api_index.html> .
:use_approach_evalml_tabular_regression a :Configuration_item ;
    skos:prefLabel "use approach EvalML tabular regression" ;
    :category :parameter ;
    skos:broader :use_approach ;
    :has_datatype :list ;
    :parameter_value :catboost , :decision_tree , :extra_tree , :light_gradient_boosting_machine , :linear_regression , :random_forest , :xgboost ;
    rdfs:comment "Selecting ML approaches to be used for AutoML" ;
    rdfs:seeAlso <https://evalml.alteryx.com/en/stable/api_index.html> .
:use_approach_evalml_text_classification a :Configuration_item ;
    skos:prefLabel "use approach EvalML text classification" ;
    :category :parameter ;
    skos:broader :use_approach ;
    :has_datatype :list ;
    :parameter_value :catboost , :decision_tree , :extra_tree , :light_gradient_boosting_machine , :linear_regression , :random_forest , :xgboost ;
    rdfs:comment "Selecting ML approaches to be used for AutoML" ;
    rdfs:seeAlso <https://evalml.alteryx.com/en/stable/api_index.html> .
:use_approach_evalml_text_regression a :Configuration_item ;
    skos:prefLabel "use approach EvalML text regression" ;
    :category :parameter ;
    skos:broader :use_approach ;
    :has_datatype :list ;
    :parameter_value :catboost , :decision_tree , :extra_tree , :light_gradient_boosting_machine , :linear_regression , :random_forest , :xgboost ;
    rdfs:comment "Selecting ML approaches to be used for AutoML" ;
    rdfs:seeAlso <https://evalml.alteryx.com/en/stable/api_index.html> .
:use_approach_evalml_time_series_regression a :Configuration_item ;
    skos:prefLabel "use approach EvalML time series regression" ;
    :category :parameter ;
    skos:broader :use_approach ;
    :has_datatype :list ;
    :parameter_value :autoregressive_integrated_moving_average , :catboost , :decision_tree , :exponential_smoothing , :extra_tree , :k_nearest_neighbor , :linear_regression , :random_forest , :xgboost ;
    rdfs:comment "Selecting ML approaches to be used for AutoML" ;
    rdfs:seeAlso <https://evalml.alteryx.com/en/stable/api_index.html> .
:use_approach_evalml_time_series_classification a :Configuration_item ;
    skos:prefLabel "use approach EvalML time series classification" ;
    :category :parameter ;
    skos:broader :use_approach ;
    :has_datatype :list ;
    :parameter_value :catboost , :decision_tree , :extra_tree , :k_nearest_neighbor , :linear_regression , :random_forest , :xgboost ;
    rdfs:comment "Selecting ML approaches to be used for AutoML" ;
    rdfs:seeAlso <https://evalml.alteryx.com/en/stable/api_index.html> .
:use_approach_auto_pytorch_classification a :Configuration_item ;
    skos:prefLabel "use approach Auto-Pytorch classification" ;
    :category :parameter ;
    skos:broader :use_approach ;
    :has_datatype :list ;
    :parameter_value :multilayer_perceptron ;
    rdfs:comment "Selecting ML approaches to be used for AutoML" ;
    rdfs:seeAlso <https://automl.github.io/Auto-PyTorch/development/api.html> .
:use_approach_auto_pytorch_regression a :Configuration_item ;
    skos:prefLabel "use approach Auto-Pytorch regression" ;
    :category :parameter ;
    skos:broader :use_approach ;
    :has_datatype :list ;
    :parameter_value :multilayer_perceptron ;
    rdfs:comment "Selecting ML approaches to be used for AutoML" ;
    rdfs:seeAlso <https://automl.github.io/Auto-PyTorch/development/api.html> .
:use_approach_autocve_classification a :Configuration_item ;
    skos:prefLabel "use approach AutoCVE classification" ;
    :category :parameter ;
    skos:broader :use_approach ;
    :has_datatype :list ;
    :parameter_value :gradient_boosting_tree , :gaussian_naives_bayes , :decision_tree , :extra_tree , :random_forest , :k_nearest_neighbor , :linear_svm , :logistic_regression , :stochastic_gradient_descent , :multilayer_perceptron ;
    rdfs:comment "Selecting ML approaches to be used for AutoML" ;
    rdfs:seeAlso <https://github.com/celiolarcher/AUTOCVE> .
:use_approach_autogluon_classification a :Configuration_item ;
    skos:prefLabel "use approach AutoGluon classification" ;
    :category :parameter ;
    skos:broader :use_approach ;
    :has_datatype :list ;
    :parameter_value :gradient_boosting_tree , :multilayer_perceptron , :k_nearest_neighbor , :random_forest , :extra_tree , :logistic_regression ;
    rdfs:comment "Selecting ML approaches to be used for AutoML" ;
    rdfs:seeAlso <https://auto.gluon.ai> .
:use_approach_autogluon_regression a :Configuration_item ;
    skos:prefLabel "use approach AutoGluon regression" ;
    :category :parameter ;
    skos:broader :use_approach ;
    :has_datatype :list ;
    :parameter_value :gradient_boosting_tree , :multilayer_perceptron , :k_nearest_neighbor , :ridge_regression , :random_forest , :extra_tree ;
    rdfs:comment "Selecting ML approaches to be used for AutoML" ;
    rdfs:seeAlso <https://auto.gluon.ai> .
:use_approach_autogluon_image_classification a :Configuration_item ;
    skos:prefLabel "use approach AutoGluon image classification" ;
    :category :parameter ;
    skos:broader :use_approach ;
    :has_datatype :list ;
    :parameter_value :multilayer_perceptron ;
    rdfs:comment "Selecting ML approaches to be used for AutoML" ;
    rdfs:seeAlso <https://auto.gluon.ai> .
:use_approach_autogluon_object_detection a :Configuration_item ;
    skos:prefLabel "use approach AutoGluon object detection" ;
    :category :parameter ;
    skos:broader :use_approach ;
    :has_datatype :list ;
    :parameter_value :multilayer_perceptron ;
    rdfs:comment "Selecting ML approaches to be used for AutoML" ;
    rdfs:seeAlso <https://auto.gluon.ai> .
:use_approach_autogluon_text_classification a :Configuration_item ;
    skos:prefLabel "use approach AutoGluon text classification" ;
    :category :parameter ;
    skos:broader :use_approach ;
    :has_datatype :list ;
    :parameter_value :multilayer_perceptron ;
    rdfs:comment "Selecting ML approaches to be used for AutoML" ;
    rdfs:seeAlso <https://auto.gluon.ai> .
:use_approach_autogluon_named_entity_recognition a :Configuration_item ;
    skos:prefLabel "use approach AutoGluon named entity recognition" ;
    :category :parameter ;
    skos:broader :use_approach ;
    :has_datatype :list ;
    :parameter_value :multilayer_perceptron ;
    rdfs:comment "Selecting ML approaches to be used for AutoML" ;
    rdfs:seeAlso <https://auto.gluon.ai> .
:use_approach_autogluon_text_regression a :Configuration_item ;
    skos:prefLabel "use approach AutoGluon text regression" ;
    :category :parameter ;
    skos:broader :use_approach ;
    :has_datatype :list ;
    :parameter_value :multilayer_perceptron ;
    rdfs:comment "Selecting ML approaches to be used for AutoML" ;
    rdfs:seeAlso <https://auto.gluon.ai> .
:use_approach_mcfly_time_series_classification a :Configuration_item ;
    skos:prefLabel "use approach mcfly time series classification" ;
    :category :parameter ;
    skos:broader :use_approach ;
    :has_datatype :list ;
    :parameter_value :inception_time , :residual_neural_network , :deep_convolutional_lstm , :convolutional_neural_network ;
    rdfs:comment "Selecting ML approaches to be used for AutoML" ;
    rdfs:seeAlso <https://mcfly.readthedocs.io/en/latest/reference.html> .
:include_preprocessor a :Configuration_item ;
    skos:prefLabel "include preprocessor" ;
    :category :parameter ;
    rdfs:comment "Selecting preprocessing approaches" .
:include_preprocessor_autosklearn_tabular_classification a :Configuration_item ;
    skos:prefLabel "include preprocessor Autosklearn tabular classification" ;
    :category :parameter ;
    skos:broader :include_preprocessor ;
    :has_datatype :list ;
    :parameter_value :kernel_principal_component_analysis , :radial_basis_function_kernel , :nystroem_kernel_approximation ;
    rdfs:comment "Selecting preprocessing approaches" ;
    rdfs:seeAlso <https://automl.github.io/auto-sklearn/master/api.html#> .
:include_preprocessor_autosklearn_tabular_regression a :Configuration_item ;
    skos:prefLabel "include preprocessor Autosklearn tabular regression" ;
    :category :parameter ;
    skos:broader :include_preprocessor ;
    :has_datatype :list ;
    :parameter_value :kernel_principal_component_analysis , :radial_basis_function_kernel , :nystroem_kernel_approximation ;
    rdfs:comment "Selecting preprocessing approaches" ;
    rdfs:seeAlso <https://automl.github.io/auto-sklearn/master/api.html#> .
:configuration_via_metalearning a :Configuration_item ;
    skos:prefLabel "configuration via metalearning" ;
    :category :parameter ;
    :has_datatype :integer ;
    rdfs:comment "Configuring meta learning, e.g., learning from hyperparameter settings that worked well in previous trainings" .
:configuration_via_metalearning_autosklearn a :Configuration_item ;
    skos:prefLabel "configuration via metalearning autosklearn" ;
    :category :parameter ;
    skos:broader :configuration_via_metalearning ;
    :has_datatype :integer ;
    rdfs:comment "Configuring meta learning, e.g., learning from hyperparameter settings that worked well in previous trainings" ;
    rdfs:seeAlso <https://automl.github.io/auto-sklearn/master/api.html#> .
:metric a :Configuration_item ;
    skos:prefLabel "metric" ;
    :category :parameter ;
    rdfs:comment "Selecting the prediction performance metric for which AutoML is optimized" .
:metric_autokeras_tabular_classification a :Configuration_item ;
    skos:prefLabel "metric autokeras tabular classification" ;
    :category :parameter ;
    skos:broader :metric ;
    :has_datatype :single_value ;
    :parameter_value :accuracy , :binary_accuracy , :categorical_accuracy , :sparse_categorical_accuracy , :top_k_categorical_accuracy , :sparse_top_k_categorical_accuracy , :binary_cross_entropy , :categorical_cross_entropy , :poisson , :area_under_roc_curve , :precision , :recall , :true_positives , :true_negatives , :false_positives , :false_negatives , :hinge , :squared_hinge , :categorical_hinge ;
    rdfs:comment "Selecting the prediction performance metric for which AutoML is optimized" ;
    rdfs:seeAlso <https://autokeras.com> .
:metric_autokeras_tabular_regression a :Configuration_item ;
    skos:prefLabel "metric autokeras tabular regression" ;
    :category :parameter ;
    skos:broader :metric ;
    :has_datatype :single_value ;
    :parameter_value :mean_squared_error , :root_mean_squared_error , :mean_absolute_error , :mean_absolute_percentage_error , :mean_squared_log_error , :cosine_similarity , :log_cosh_error ;
    rdfs:comment "Selecting the prediction performance metric for which AutoML is optimized" ;
    rdfs:seeAlso <https://autokeras.com> .
:metric_autokeras_image_classification a :Configuration_item ;
    skos:prefLabel "metric AutoKeras image classification" ;
    :category :parameter ;
    skos:broader :metric ;
    :has_datatype :single_value ;
    :parameter_value :accuracy , :binary_accuracy , :categorical_accuracy , :sparse_categorical_accuracy , :top_k_categorical_accuracy , :sparse_top_k_categorical_accuracy , :binary_cross_entropy , :categorical_cross_entropy , :poisson , :area_under_roc_curve , :precision , :recall , :true_positives , :true_negatives , :false_positives , :false_negatives , :hinge , :squared_hinge , :categorical_hinge ;
    rdfs:comment "Selecting the prediction performance metric for which AutoML is optimized" ;
    rdfs:seeAlso <https://autokeras.com> .
:metric_autokeras_image_regression a :Configuration_item ;
    skos:prefLabel "metric AutoKeras image regression" ;
    :category :parameter ;
    skos:broader :metric ;
    :has_datatype :single_value ;
    :parameter_value :mean_squared_error , :root_mean_squared_error , :mean_absolute_error , :mean_absolute_percentage_error , :mean_squared_log_error , :cosine_similarity , :log_cosh_error ;
    rdfs:comment "Selecting the prediction performance metric for which AutoML is optimized" ;
    rdfs:seeAlso <https://autokeras.com> .
:metric_autokeras_text_classification a :Configuration_item ;
    skos:prefLabel "metric AutoKeras text classification" ;
    :category :parameter ;
    skos:broader :metric ;
    :has_datatype :single_value ;
    :parameter_value :accuracy , :binary_accuracy , :categorical_accuracy , :sparse_categorical_accuracy , :top_k_categorical_accuracy , :sparse_top_k_categorical_accuracy , :binary_cross_entropy , :categorical_cross_entropy , :poisson , :area_under_roc_curve , :precision , :recall , :true_positives , :true_negatives , :false_positives , :false_negatives , :hinge , :squared_hinge , :categorical_hinge ;
    rdfs:comment "Selecting the prediction performance metric for which AutoML is optimized" ;
    rdfs:seeAlso <https://autokeras.com> .
:metric_autokeras_text_regression a :Configuration_item ;
    skos:prefLabel "metric AutoKeras text regression" ;
    :category :parameter ;
    skos:broader :metric ;
    :has_datatype :single_value ;
    :parameter_value :mean_squared_error , :root_mean_squared_error , :mean_absolute_error , :mean_absolute_percentage_error , :mean_squared_log_error , :cosine_similarity , :log_cosh_error ;
    rdfs:comment "Selecting the prediction performance metric for which AutoML is optimized" ;
    rdfs:seeAlso <https://autokeras.com> .
:metric_autokeras_time_series_forecasting a :Configuration_item ;
    skos:prefLabel "metric AutoKeras time series forecasting" ;
    :category :parameter ;
    skos:broader :metric ;
    :has_datatype :single_value ;
    :parameter_value :mean_squared_error , :root_mean_squared_error , :mean_absolute_error , :mean_absolute_percentage_error , :mean_squared_log_error , :cosine_similarity , :log_cosh_error ;
    rdfs:comment "Selecting the prediction performance metric for which AutoML is optimized" ;
    rdfs:seeAlso <https://autokeras.com> .
:metric_autosklearn_tabular_classification a :Configuration_item ;
    skos:prefLabel "metric Autosklearn tabular classification" ;
    :category :parameter ;
    skos:broader :metric ;
    :has_datatype :single_value ;
    :parameter_value :accuracy , :balanced_accuracy , :f_measure , :f_measure_macro , :f_measure_micro , :f_measure_samples , :f_measure_weighted , :receiver_operating_characteristic_curve , :precision , :precision_macro , :precision_micro , :precision_samples , :precision_weighted , :average_precision , :recall , :recall_macro , :recall_micro , :recall_samples , :recall_weighted , :log_loss ;
    rdfs:comment "Selecting the prediction performance metric for which AutoML is optimized" ;
    rdfs:seeAlso <https://automl.github.io/auto-sklearn/master/api.html#classification> .
:metric_autosklearn_tabular_regression a :Configuration_item ;
    skos:prefLabel "metric Autosklearn tabular regression" ;
    :category :parameter ;
    skos:broader :metric ;
    :has_datatype :single_value ;
    :parameter_value :r2 , :mean_squared_error , :mean_absolute_error , :median_absolute_error ;
    rdfs:comment "Selecting the prediction performance metric for which AutoML is optimized" ;
    rdfs:seeAlso <https://automl.github.io/auto-sklearn/master/api.html#regression> .
:metric_flaml_tabular_classification a :Configuration_item ;
    skos:prefLabel "metric FLAML tabular classification" ;
    :category :parameter ;
    skos:broader :metric ;
    :has_datatype :single_value ;
    :parameter_value :accuracy , :receiver_operating_characteristic_curve , :receiver_operating_characteristic_curve_one_vs_rest , :log_loss , :receiver_operating_characteristic_curve_one_vs_one , :average_precision , :f_measure , :f_measure_micro , :f_measure_macro , :area_under_roc_curve_weighted , :receiver_operating_characteristic_curve_one_vs_rest_weighted , :receiver_operating_characteristic_curve_one_vs_one_weighted ;
    rdfs:comment "Selecting the prediction performance metric for which AutoML is optimized" ;
    rdfs:seeAlso <https://microsoft.github.io/FLAML/docs/reference/automl/automl> .
:metric_flaml_tabular_regression a :Configuration_item ;
    skos:prefLabel "metric FLAML tabular regression" ;
    :category :parameter ;
    skos:broader :metric ;
    :has_datatype :single_value ;
    :parameter_value :mean_squared_error , :root_mean_squared_error , :mean_absolute_error , :receiver_operating_characteristic_curve_one_vs_rest , :receiver_operating_characteristic_curve_one_vs_one , :receiver_operating_characteristic_curve , :mean_absolute_percentage_error , :r2 , :area_under_roc_curve_weighted , :receiver_operating_characteristic_curve_one_vs_rest_weighted , :receiver_operating_characteristic_curve_one_vs_one_weighted ;
    rdfs:comment "Selecting the prediction performance metric for which AutoML is optimized" ;
    rdfs:seeAlso <https://microsoft.github.io/FLAML/docs/reference/automl/automl> .
:metric_flaml_text_classification a :Configuration_item ;
    skos:prefLabel "metric FLAML text classification" ;
    :category :parameter ;
    skos:broader :metric ;
    :has_datatype :single_value ;
    :parameter_value :accuracy , :receiver_operating_characteristic_curve , :receiver_operating_characteristic_curve_one_vs_rest , :log_loss , :receiver_operating_characteristic_curve_one_vs_one , :average_precision , :f_measure , :f_measure_micro , :f_measure_macro , :area_under_roc_curve_weighted , :receiver_operating_characteristic_curve_one_vs_rest_weighted , :receiver_operating_characteristic_curve_one_vs_one_weighted ;
    rdfs:comment "Selecting the prediction performance metric for which AutoML is optimized" ;
    rdfs:seeAlso <https://microsoft.github.io/FLAML/docs/reference/automl/automl> .
:metric_flaml_text_regression a :Configuration_item ;
    skos:prefLabel "metric FLAML text regression" ;
    :category :parameter ;
    skos:broader :metric ;
    :has_datatype :single_value ;
    :parameter_value :mean_squared_error , :root_mean_squared_error , :mean_absolute_error , :receiver_operating_characteristic_curve_one_vs_rest , :receiver_operating_characteristic_curve_one_vs_one , :receiver_operating_characteristic_curve , :mean_absolute_percentage_error , :r2 , :area_under_roc_curve_weighted , :receiver_operating_characteristic_curve_one_vs_rest_weighted , :receiver_operating_characteristic_curve_one_vs_one_weighted ;
    rdfs:comment "Selecting the prediction performance metric for which AutoML is optimized" ;
    rdfs:seeAlso <https://microsoft.github.io/FLAML/docs/reference/automl/automl> .
:metric_flaml_ranking a :Configuration_item ;
    skos:prefLabel "metric FLAML ranking" ;
    :category :parameter ;
    skos:broader :metric ;
    :has_datatype :single_value ;
    :parameter_value :normalized_discounted_cumulative_gain ;
    rdfs:comment "Selecting the prediction performance metric for which AutoML is optimized" ;
    rdfs:seeAlso <https://microsoft.github.io/FLAML/docs/reference/automl/automl> .
:metric_flaml_time_series_analysis a :Configuration_item ;
    skos:prefLabel "metric FLAML time series analysis" ;
    :category :parameter ;
    skos:broader :metric ;
    :has_datatype :single_value ;
    :parameter_value :mean_absolute_percentage_error ;
    rdfs:comment "Selecting the prediction performance metric for which AutoML is optimized" ;
    rdfs:seeAlso <https://microsoft.github.io/FLAML/docs/reference/automl/automl> .
:metric_evalml_tabular_classification a :Configuration_item ;
    skos:prefLabel "metric EvalML tabular classification" ;
    :category :parameter ;
    skos:broader :metric ;
    :has_datatype :single_value ;
    :parameter_value :accuracy , :balanced_accuracy , :f_measure , :f_measure_micro , :f_measure_macro , :f_measure_weighted , :precision , :precision_macro , :precision_micro , :precision_weighted , :recall , :recall_micro , :recall_macro , :recall_weighted , :area_under_roc_curve , :area_under_roc_curve_micro , :area_under_roc_curve_macro , :area_under_roc_curve_weighted , :gini , :log_loss , :matthews_correlation_coefficient ;
    rdfs:comment "Selecting the prediction performance metric for which AutoML is optimized" ;
    rdfs:seeAlso <https://evalml.alteryx.com/en/stable/api_index.html> .
:metric_evalml_tabular_regression a :Configuration_item ;
    skos:prefLabel "metric EvalML tabular regression" ;
    :category :parameter ;
    skos:broader :metric ;
    :has_datatype :single_value ;
    :parameter_value :root_mean_squared_error , :mean_squared_log_error , :root_mean_squared_log_error , :r2 , :mean_absolute_error , :mean_squared_error , :median_absolute_error , :max_error , :explained_variance ;
    rdfs:comment "Selecting the prediction performance metric for which AutoML is optimized" ;
    rdfs:seeAlso <https://evalml.alteryx.com/en/stable/api_index.html> .
:metric_evalml_text_classification a :Configuration_item ;
    skos:prefLabel "metric EvalML text classification" ;
    :category :parameter ;
    skos:broader :metric ;
    :has_datatype :single_value ;
    :parameter_value :accuracy , :balanced_accuracy , :f_measure , :f_measure_micro , :f_measure_macro , :f_measure_weighted , :precision , :precision_macro , :precision_micro , :precision_weighted , :recall , :recall_micro , :recall_macro , :recall_weighted , :area_under_roc_curve , :area_under_roc_curve_micro , :area_under_roc_curve_macro , :area_under_roc_curve_weighted , :gini , :log_loss , :matthews_correlation_coefficient ;
    rdfs:comment "Selecting the prediction performance metric for which AutoML is optimized" ;
    rdfs:seeAlso <https://evalml.alteryx.com/en/stable/api_index.html> .
:metric_evalml_text_regression a :Configuration_item ;
    skos:prefLabel "metric EvalML text regression" ;
    :category :parameter ;
    skos:broader :metric ;
    :has_datatype :single_value ;
    :parameter_value :root_mean_squared_error , :mean_squared_log_error , :root_mean_squared_log_error , :r2 , :mean_absolute_error , :mean_squared_error , :median_absolute_error , :max_error , :explained_variance ;
    rdfs:comment "Selecting the prediction performance metric for which AutoML is optimized" ;
    rdfs:seeAlso <https://evalml.alteryx.com/en/stable/api_index.html> .
:metric_evalml_time_series_regression a :Configuration_item ;
    skos:prefLabel "metric EvalML time series regression" ;
    :category :parameter ;
    skos:broader :metric ;
    :has_datatype :single_value ;
    :parameter_value :mean_absolute_percentage_error ;
    rdfs:comment "Selecting the prediction performance metric for which AutoML is optimized" ;
    rdfs:seeAlso <https://evalml.alteryx.com/en/stable/api_index.html> .
:metric_autogluon_tabular_regression a :Configuration_item ;
    skos:prefLabel "metric AutoGluon tabular regression" ;
    :category :parameter ;
    skos:broader :metric ;
    :has_datatype :single_value ;
    :parameter_value :root_mean_squared_error , :mean_squared_error , :mean_absolute_error , :median_absolute_error , :mean_absolute_percentage_error , :r2 ;
    rdfs:comment "Selecting the prediction performance metric for which AutoML is optimized" ;
    rdfs:seeAlso <https://auto.gluon.ai> .
:metric_autogluon_tabular_classification a :Configuration_item ;
    skos:prefLabel "metric AutoGluon tabular classification" ;
    :category :parameter ;
    skos:broader :metric ;
    :has_datatype :single_value ;
    :parameter_value :accuracy , :balanced_accuracy , :f_measure , :f_measure_macro , :f_measure_micro , :f_measure_weighted , :receiver_operating_characteristic_curve , :receiver_operating_characteristic_curve_one_vs_one , :average_precision , :precision , :precision_macro , :precision_micro , :precision_weighted , :recall , :recall_macro , :recall_micro , :recall_weighted , :log_loss , :pac_score ;
    rdfs:comment "Selecting the prediction performance metric for which AutoML is optimized" ;
    rdfs:seeAlso <https://auto.gluon.ai> .
:metric_autogluon_text_classification a :Configuration_item ;
    skos:prefLabel "metric AutoGluon text classification" ;
    :category :parameter ;
    skos:broader :metric ;
    :has_datatype :single_value ;
    :parameter_value :accuracy , :balanced_accuracy , :f_measure , :f_measure_macro , :f_measure_micro , :f_measure_weighted , :receiver_operating_characteristic_curve , :receiver_operating_characteristic_curve_one_vs_one , :average_precision , :precision , :precision_macro , :precision_micro , :precision_weighted , :recall , :recall_macro , :recall_micro , :recall_weighted , :log_loss , :pac_score ;
    rdfs:comment "Selecting the prediction performance metric for which AutoML is optimized" ;
    rdfs:seeAlso <https://auto.gluon.ai> .
:metric_autogluon_named_entity_recognition a :Configuration_item ;
    skos:prefLabel "metric AutoGluon named entity recognition" ;
    :category :parameter ;
    skos:broader :metric ;
    :has_datatype :single_value ;
    :parameter_value :overall_recall , :overall_precision , :overall_f1 , :overall_accuracy ;
    rdfs:comment "Selecting the prediction performance metric for which AutoML is optimized" ;
    rdfs:seeAlso <https://auto.gluon.ai> .
:metric_autogluon_text_regression a :Configuration_item ;
    skos:prefLabel "metric AutoGluon text regression" ;
    :category :parameter ;
    skos:broader :metric ;
    :has_datatype :single_value ;
    :parameter_value :root_mean_squared_error , :mean_squared_error , :mean_absolute_error , :median_absolute_error , :r2 , :spearman_rank_correlation_coefficient , :pearson_correlation_coefficient ;
    rdfs:comment "Selecting the prediction performance metric for which AutoML is optimized" ;
    rdfs:seeAlso <https://auto.gluon.ai> .
:metric_autogluon_image_classification a :Configuration_item ;
    skos:prefLabel "metric AutoGluon image classification" ;
    :category :parameter ;
    skos:broader :metric ;
    :has_datatype :single_value ;
    :parameter_value :accuracy ;
    rdfs:comment "Selecting the prediction performance metric for which AutoML is optimized" ;
    rdfs:seeAlso <https://auto.gluon.ai> .
:metric_autogluon_time_series_forecasting a :Configuration_item ;
    skos:prefLabel "metric AutoGluon time series forecasting" ;
    :category :parameter ;
    skos:broader :metric ;
    :has_datatype :single_value ;
    :parameter_value :mean_absolute_percentage_error , :symmetric_mean_absolute_percentage_error , :mean_absolute_scaled_error , :mean_squared_error , :root_mean_squared_error ;
    rdfs:comment "Selecting the prediction performance metric for which AutoML is optimized" ;
    rdfs:seeAlso <https://auto.gluon.ai> .
:metric_autopytorch_tabular_classification a :Configuration_item ;
    skos:prefLabel "metric AutoPytorch tabular classification" ;
    :category :parameter ;
    skos:broader :metric ;
    :has_datatype :single_value ;
    :parameter_value :accuracy , :balanced_accuracy , :f_measure , :receiver_operating_characteristic_curve , :average_precision , :precision , :recall , :log_loss ;
    rdfs:comment "Selecting the prediction performance metric for which AutoML is optimized" .
:metric_autopytorch_time_series_forecasting a :Configuration_item ;
    skos:prefLabel "metric AutoPytorch time series forecasting" ;
    :category :parameter ;
    skos:broader :metric ;
    :has_datatype :single_value ;
    :parameter_value :mean_absolute_scaled_error , :median_absolute_scaled_error , :mean_absolute_error , :median_absolute_error , :mean_absolute_percentage_error , :median_absolute_percentage_error , :mean_squared_error , :median_squared_error ;
    rdfs:comment "Selecting the prediction performance metric for which AutoML is optimized" .
:metric_autopytorch_tabular_regression a :Configuration_item ;
    skos:prefLabel "metric AutoPytorch tabular regression" ;
    :category :parameter ;
    skos:broader :metric ;
    :has_datatype :single_value ;
    :parameter_value :mean_absolute_error , :mean_squared_error , :root_mean_squared_error , :mean_squared_log_error , :median_absolute_error , :r2 ;
    rdfs:comment "Selecting the prediction performance metric for which AutoML is optimized" .
:metric_autocve_classification a :Configuration_item ;
    skos:prefLabel "metric AutoCVE classification" ;
    :category :parameter ;
    skos:broader :metric ;
    :has_datatype :single_value ;
    :parameter_value :accuracy ;
    rdfs:comment "Selecting the prediction performance metric for which AutoML is optimized" ;
    rdfs:seeAlso <https://github.com/celiolarcher/AUTOCVE> .
:metric_mcfly_time_series_classification a :Configuration_item ;
    skos:prefLabel "metric mcfly time series classification" ;
    :category :parameter ;
    skos:broader :metric ;
    :has_datatype :list ;
    :parameter_value :accuracy , :balanced_accuracy , :f_measure , :f_measure_macro , :f_measure_micro , :f_measure_weighted , :f_measure_samples , :receiver_operating_characteristic_curve , :average_precision , :log_loss , :precision , :precision_macro , :precision_micro , :precision_weighted , :precision_samples , :recall , :recall_macro , :recall_micro , :recall_weighted , :recall_samples ;
    rdfs:comment "Selecting the prediction performance metric for which AutoML is optimized" ;
    rdfs:seeAlso <https://mcfly.readthedocs.io/en/latest/reference.html> .
:metric_mljar_tabular_classification a :Configuration_item ;
    skos:prefLabel "metric MLJAR tabular classification" ;
    :category :parameter ;
    skos:broader :metric ;
    :has_datatype :single_value ;
    :parameter_value :log_loss , :area_under_roc_curve , :f_measure , :accuracy , :precision , :recall , :matthews_correlation_coefficient ;
    rdfs:comment "Selecting the prediction performance metric for which AutoML is optimized" ;
    rdfs:seeAlso <https://supervised.mljar.com/api> .
:metric_mljar_tabular_regression a :Configuration_item ;
    skos:prefLabel "metric MLJAR tabular regression" ;
    :category :parameter ;
    skos:broader :metric ;
    :has_datatype :single_value ;
    :parameter_value :mean_absolute_error , :mean_squared_error , :root_mean_squared_error , :r2 , :mean_absolute_percentage_error ;
    rdfs:comment "Selecting the prediction performance metric for which AutoML is optimized" ;
    rdfs:seeAlso <https://supervised.mljar.com/api> .
:metric_pycaret_tabular_classification a :Configuration_item ;
    skos:prefLabel "metric PyCaret tabular classification" ;
    :category :parameter ;
    skos:broader :metric ;
    :has_datatype :single_value ;
    :parameter_value :accuracy , :area_under_roc_curve , :recall , :precision , :f_measure , :cohens_kappa , :matthews_correlation_coefficient ;
    rdfs:comment "Selecting the prediction performance metric for which AutoML is optimized" ;
    rdfs:seeAlso <https://pycaret.readthedocs.io> .
:metric_pycaret_tabular_regression a :Configuration_item ;
    skos:prefLabel "metric PyCaret tabular regression" ;
    :category :parameter ;
    skos:broader :metric ;
    :has_datatype :single_value ;
    :parameter_value :mean_absolute_error , :mean_squared_error , :root_mean_squared_error , :r2 , :root_mean_squared_log_error , :mean_absolute_percentage_error ;
    rdfs:comment "Selecting the prediction performance metric for which AutoML is optimized" ;
    rdfs:seeAlso <https://pycaret.readthedocs.io> .
:metric_pycaret_time_series_forecasting a :Configuration_item ;
    skos:prefLabel "metric PyCaret time series forecasting" ;
    :category :parameter ;
    skos:broader :metric ;
    :has_datatype :single_value ;
    :parameter_value :mean_absolute_scaled_error , :root_mean_squared_scaled_error , :symmetric_mean_absolute_percentage_error , :coverage , :mean_absolute_error , :root_mean_squared_error , :mean_absolute_percentage_error , :r2 ;
    rdfs:comment "Selecting the prediction performance metric for which AutoML is optimized" ;
    rdfs:seeAlso <https://pycaret.readthedocs.io> .
:metric_tpot_tabular_classification a :Configuration_item ;
    skos:prefLabel "metric TPOT tabular classification" ;
    :category :parameter ;
    skos:broader :metric ;
    :has_datatype :single_value ;
    :parameter_value :accuracy , :average_precision , :adjusted_rand_score , :balanced_accuracy , :f_measure , :f_measure_macro , :f_measure_micro , :f_measure_samples , :f_measure_weighted , :log_loss , :precision , :precision_macro , :precision_micro , :precision_samples , :precision_weighted , :recall , :recall_macro , :recall_micro , :recall_samples , :recall_weighted , :jaccard , :jaccard_macro , :jaccard_micro , :jaccard_samples , :jaccard_weighted , :receiver_operating_characteristic_curve , :receiver_operating_characteristic_curve_one_vs_rest , :receiver_operating_characteristic_curve_one_vs_one , :receiver_operating_characteristic_curve_one_vs_rest_weighted , :receiver_operating_characteristic_curve_one_vs_one_weighted ;
    rdfs:comment "Selecting the prediction performance metric for which AutoML is optimized" ;
    rdfs:seeAlso <http://epistasislab.github.io/tpot/api> .
:metric_tpot_tabular_regression a :Configuration_item ;
    skos:prefLabel "metric TPOT tabular regression" ;
    :category :parameter ;
    skos:broader :metric ;
    :has_datatype :single_value ;
    :parameter_value :median_absolute_error , :mean_absolute_error , :mean_squared_error , :r2 ;
    rdfs:comment "Selecting the prediction performance metric for which AutoML is optimized" ;
    rdfs:seeAlso <http://epistasislab.github.io/tpot/api> .
:metric_tpot_image_classification a :Configuration_item ;
    skos:prefLabel "metric TPOT image classification" ;
    :category :parameter ;
    skos:broader :metric ;
    :has_datatype :single_value ;
    :parameter_value :accuracy , :average_precision , :adjusted_rand_score , :balanced_accuracy , :f_measure , :f_measure_macro , :f_measure_micro , :f_measure_samples , :f_measure_weighted , :log_loss , :precision , :precision_macro , :precision_micro , :precision_samples , :precision_weighted , :recall , :recall_macro , :recall_micro , :recall_samples , :recall_weighted , :jaccard , :jaccard_macro , :jaccard_micro , :jaccard_samples , :jaccard_weighted , :receiver_operating_characteristic_curve , :receiver_operating_characteristic_curve_one_vs_rest , :receiver_operating_characteristic_curve_one_vs_one , :receiver_operating_characteristic_curve_one_vs_rest_weighted , :receiver_operating_characteristic_curve_one_vs_one_weighted ;
    rdfs:comment "Selecting the prediction performance metric for which AutoML is optimized" ;
    rdfs:seeAlso <http://epistasislab.github.io/tpot/api> .
:metric_gama_tabular_classification a :Configuration_item ;
    skos:prefLabel "metric GAMA tabular classification" ;
    :category :parameter ;
    skos:broader :metric ;
    :has_datatype :list ;
    :parameter_value :accuracy , :average_precision , :receiver_operating_characteristic_curve , :neg_log_loss , :f_measure_macro , :f_measure_micro , :f_measure_samples , :f_measure_weighted , :precision_macro , :precision_micro , :precision_samples , :precision_weighted , :recall_macro , :recall_micro , :recall_samples , :recall_weighted ;
    rdfs:comment "Selecting the prediction performance metric for which AutoML is optimized" ;
    rdfs:seeAlso <https://openml-labs.github.io/gama/master/api/index.html> .
:metric_gama_tabular_regression a :Configuration_item ;
    skos:prefLabel "metric GAMA tabular regression" ;
    :category :parameter ;
    skos:broader :metric ;
    :has_datatype :list ;
    :parameter_value :explained_variance , :r2 , :mean_absolute_error , :median_absolute_error , :mean_squared_error , :mean_squared_log_error ;
    rdfs:comment "Selecting the prediction performance metric for which AutoML is optimized" ;
    rdfs:seeAlso <https://openml-labs.github.io/gama/master/api/index.html> .
:metric_lama_tabular_classification a :Configuration_item ;
    skos:prefLabel "metric LAMA tabular classification" ;
    :category :parameter ;
    skos:broader :metric ;
    :has_datatype :single_value ;
    :parameter_value :area_under_roc_curve , :categorical_cross_entropy ;
    rdfs:comment "Selecting the prediction performance metric for which AutoML is optimized" ;
    rdfs:seeAlso <https://lightautoml.readthedocs.io/en/latest/pages/modules/generated/lightautoml.tasks.base.Task.html#lightautoml.tasks.base.Task> .
:metric_lama_binary_classification a :Configuration_item ;
    skos:prefLabel "metric LAMA binary classification" ;
    :category :parameter ;
    skos:broader :metric ;
    :has_datatype :single_value ;
    :parameter_value :area_under_roc_curve , :accuracy , :log_loss ;
    rdfs:comment "Selecting the prediction performance metric for which AutoML is optimized" ;
    rdfs:seeAlso <https://lightautoml.readthedocs.io/en/latest/pages/modules/generated/lightautoml.tasks.base.Task.html#lightautoml.tasks.base.Task> .
:metric_lama_tabular_regression a :Configuration_item ;
    skos:prefLabel "metric LAMA tabular regression" ;
    :category :parameter ;
    skos:broader :metric ;
    :has_datatype :single_value ;
    :parameter_value :mean_squared_error , :mean_absolute_error , :mean_absolute_percentage_error , :root_mean_squared_log_error ;
    rdfs:comment "Selecting the prediction performance metric for which AutoML is optimized" ;
    rdfs:seeAlso <https://lightautoml.readthedocs.io/en/latest/pages/modules/generated/lightautoml.tasks.base.Task.html#lightautoml.tasks.base.Task> .
:metric_h2o_automl_tabular_classification a :Configuration_item ;
    skos:prefLabel "metric h2o AutoML tabular classification" ;
    :category :parameter ;
    skos:broader :metric ;
    :has_datatype :single_value ;
    :parameter_value :accuracy , :area_under_roc_curve , :area_under_precision_recall_curve , :log_loss , :mean_squared_error , :mean_per_class_error .
:metric_h2o_automl_tabular_regression a :Configuration_item ;
    skos:prefLabel "metric h2o AutoML tabular regression" ;
    :category :parameter ;
    skos:broader :metric ;
    :has_datatype :single_value ;
    :parameter_value :mean_absolute_error , :mean_residual_deviance , :mean_squared_error , :root_mean_squared_error , :root_mean_squared_log_error .
:time_limit a :Configuration_item ;
    skos:prefLabel "time limit" ;
    :category :parameter ;
    :has_datatype :integer ;
    rdfs:comment "Specifying the maximum runtime of AutoML" .
:time_limit_autosklearn_tabular_classification a :Configuration_item ;
    skos:prefLabel "time limit autosklearn tabular classification" ;
    :category :parameter ;
    skos:broader :time_limit ;
    :has_datatype :integer ;
    rdfs:comment "Specifying the maximum runtime of AutoML" ;
    rdfs:seeAlso <https://automl.github.io/auto-sklearn/master/api.html#> .
:time_limit_autosklearn_tabular_regression a :Configuration_item ;
    skos:prefLabel "time limit autosklearn tabular regression" ;
    :category :parameter ;
    skos:broader :time_limit ;
    :has_datatype :integer ;
    rdfs:comment "Specifying the maximum runtime of AutoML" ;
    rdfs:seeAlso <https://automl.github.io/auto-sklearn/master/api.html#> .
:time_limit_per_run a :Configuration_item ;
    skos:prefLabel "time limit per run" ;
    :category :parameter ;
    :has_datatype :integer ;
    rdfs:comment "Specifying the maximum runtime per AutoML run" .
:time_limit_per_run_autosklearn_tabular_classification a :Configuration_item ;
    skos:prefLabel "time limit per run autosklearn tabular classification" ;
    :category :parameter ;
    skos:broader :time_limit_per_run ;
    :has_datatype :integer ;
    rdfs:comment "Specifying the maximum runtime per AutoML run" ;
    rdfs:seeAlso <https://automl.github.io/auto-sklearn/master/api.html#> .
:time_limit_per_run_autosklearn_tabular_regression a :Configuration_item ;
    skos:prefLabel "time limit per run autosklearn tabular regression" ;
    :category :parameter ;
    skos:broader :time_limit_per_run ;
    :has_datatype :integer ;
    rdfs:comment "Specifying the maximum runtime per AutoML run" ;
    rdfs:seeAlso <https://automl.github.io/auto-sklearn/master/api.html#> .
:max_model_size a :Configuration_item ;
    skos:prefLabel "max_model_size" ;
    :category :parameter ;
    :has_datatype :integer ;
    rdfs:comment "Specifying the maximum size of a neural network model" .
:max_model_size_autokeras_tabular_classification a :Configuration_item ;
    skos:prefLabel "max model size autokeras tabular classification" ;
    :category :parameter ;
    skos:broader :max_model_size ;
    :has_datatype :integer ;
    rdfs:comment "Specifying the maximum size of a neural network model" ;
    rdfs:seeAlso <https://autokeras.com> .
:max_model_size_autokeras_tabular_regression a :Configuration_item ;
    skos:prefLabel "max model size autokeras tabular regression" ;
    :category :parameter ;
    skos:broader :max_model_size ;
    :has_datatype :integer ;
    rdfs:comment "Specifying the maximum size of a neural network model" ;
    rdfs:seeAlso <https://autokeras.com> .
:max_model_size_autokeras_image_classification a :Configuration_item ;
    skos:prefLabel "max model size autokeras image classification" ;
    :category :parameter ;
    skos:broader :max_model_size ;
    :has_datatype :integer ;
    rdfs:comment "Specifying the maximum size of a neural network model" ;
    rdfs:seeAlso <https://autokeras.com> .
:max_model_size_autokeras_image_regression a :Configuration_item ;
    skos:prefLabel "max model size autokeras image regression" ;
    :category :parameter ;
    skos:broader :max_model_size ;
    :has_datatype :integer ;
    rdfs:comment "Specifying the maximum size of a neural network model" ;
    rdfs:seeAlso <https://autokeras.com> .
:max_model_size_autokeras_text_classification a :Configuration_item ;
    skos:prefLabel "max model size autokeras text classification" ;
    :category :parameter ;
    skos:broader :max_model_size ;
    :has_datatype :integer ;
    rdfs:comment "Specifying the maximum size of a neural network model" ;
    rdfs:seeAlso <https://autokeras.com> .
:max_model_size_autokeras_text_regression a :Configuration_item ;
    skos:prefLabel "max model size autokeras text regression" ;
    :category :parameter ;
    skos:broader :max_model_size ;
    :has_datatype :integer ;
    rdfs:comment "Specifying the maximum size of a neural network model" ;
    rdfs:seeAlso <https://autokeras.com> .
:max_model_size_autokeras_time_series_forecasting a :Configuration_item ;
    skos:prefLabel "max model size autokeras time series forecasting" ;
    :category :parameter ;
    skos:broader :max_model_size ;
    :has_datatype :integer ;
    rdfs:comment "Specifying the maximum size of a neural network model" ;
    rdfs:seeAlso <https://autokeras.com> .
:include_approach a :Configuration_item ;
    skos:prefLabel "include approach" ;
    :category :parameter ;
    :has_datatype :list .
:include_approach_autosklearn a :Configuration_item ;
    skos:prefLabel "include approach autosklearn" ;
    :category :parameter ;
    skos:broader :include_approach ;
    :has_datatype :list ;
    rdfs:seeAlso <https://automl.github.io/auto-sklearn/master/api.html#> .
:include_approach_h2o_automl a :Configuration_item ;
    skos:prefLabel "include approach h2o automl" ;
    :category :parameter ;
    skos:broader :include_approach ;
    :has_datatype :list ;
    :parameter_value :distributed_random_forest , :artificial_neural_network , :gradient_boosting_tree , :stacking_ensemble .
:include_approach_pycaret_clustering a :Configuration_item ;
    skos:prefLabel "include approach pycaret Clustering" ;
    :category :parameter ;
    skos:broader :include_approach ;
    :has_datatype :list ;
    :parameter_value :affinity_propagation , :agglomerative_clustering , :balanced_iterative_reducing_and_clustering_using_hierarchies , :density_based_spatial_clustering_of_applications_with_noise , :k_means , :k_modes , :mean_shift_clustering , :ordering_points_to_identify_the_clustering_structure , :spectral_clustering ;
    rdfs:seeAlso <https://pycaret.readthedocs.io/en/latest/api/clustering.html#pycaret.clustering.create_model> .
:epochs a :Configuration_item ;
    skos:prefLabel "epochs" ;
    :category :parameter ;
    :has_datatype :integer ;
    rdfs:comment "Specifying the number of epochs for training neural networks, i.e., how often the entire dataset will be used for training" .
:epochs_mcfly a :Configuration_item ;
    skos:prefLabel "epochs mcfly" ;
    :category :parameter ;
    skos:broader :epochs ;
    :has_datatype :integer ;
    rdfs:comment "Specifying the number of epochs for training neural networks, i.e., how often the entire dataset will be used for training" .
:max_trials a :Configuration_item ;
    skos:prefLabel "max_trials" ;
    :category :parameter ;
    :has_datatype :integer ;
    rdfs:comment "Specifying the maximum number of different Models to try" .
:max_trials_autokeras_tabular_classification a :Configuration_item ;
    skos:prefLabel "max trials autokeras tabular classification" ;
    :category :parameter ;
    skos:broader :max_trials ;
    :has_datatype :integer ;
    rdfs:comment "Specifying the maximum number of different Models to try" ;
    rdfs:seeAlso <https://autokeras.com> .
:max_trials_autokeras_tabular_regression a :Configuration_item ;
    skos:prefLabel "max trials autokeras tabular regression" ;
    :category :parameter ;
    skos:broader :max_trials ;
    :has_datatype :integer ;
    rdfs:comment "Specifying the maximum number of different Models to try" ;
    rdfs:seeAlso <https://autokeras.com> .
:max_trials_autokeras_image_classification a :Configuration_item ;
    skos:prefLabel "max trials autokeras image classification" ;
    :category :parameter ;
    skos:broader :max_trials ;
    :has_datatype :integer ;
    rdfs:comment "Specifying the maximum number of different Models to try" ;
    rdfs:seeAlso <https://autokeras.com> .
:max_trials_autokeras_image_regression a :Configuration_item ;
    skos:prefLabel "max trials autokeras image regression" ;
    :category :parameter ;
    skos:broader :max_trials ;
    :has_datatype :integer ;
    rdfs:comment "Specifying the maximum number of different Models to try" ;
    rdfs:seeAlso <https://autokeras.com> .
:max_trials_autokeras_text_classification a :Configuration_item ;
    skos:prefLabel "max trials autokeras text classification" ;
    :category :parameter ;
    skos:broader :max_trials ;
    :has_datatype :integer ;
    rdfs:comment "Specifying the maximum number of different Models to try" ;
    rdfs:seeAlso <https://autokeras.com> .
:max_trials_autokeras_text_regression a :Configuration_item ;
    skos:prefLabel "max trials autokeras text regression" ;
    :category :parameter ;
    skos:broader :max_trials ;
    :has_datatype :integer ;
    rdfs:comment "Specifying the maximum number of different Models to try" ;
    rdfs:seeAlso <https://autokeras.com> .
:max_trials_autokeras_time_series_forecasting a :Configuration_item ;
    skos:prefLabel "max trials autokeras time series forecasting" ;
    :category :parameter ;
    skos:broader :max_trials ;
    :has_datatype :integer ;
    rdfs:comment "Specifying the maximum number of different Models to try" ;
    rdfs:seeAlso <https://autokeras.com> .
:tuner a :Configuration_item ;
    skos:prefLabel "tuner" ;
    :category :parameter ;
    :has_datatype :single_value ;
    rdfs:comment "Selecting the tuner approach for training" ;
    rdfs:seeAlso <https://autokeras.com> .
:tuner_autokeras_tabular_regression a :Configuration_item ;
    skos:prefLabel "tuner autokeras tabular regression" ;
    :category :parameter ;
    skos:broader :tuner ;
    :has_datatype :single_value ;
    :parameter_value :greedy , :bayesian , :random , :hyperband ;
    rdfs:comment "Selecting the tuner approach for training" ;
    rdfs:seeAlso <https://autokeras.com> .
:tuner_autokeras_tabular_classification a :Configuration_item ;
    skos:prefLabel "tuner autokeras tabular classification" ;
    :category :parameter ;
    skos:broader :tuner ;
    :has_datatype :single_value ;
    :parameter_value :greedy , :bayesian , :random , :hyperband ;
    rdfs:comment "Selecting the tuner approach for training" ;
    rdfs:seeAlso <https://autokeras.com> .
:tuner_autokeras_image_regression a :Configuration_item ;
    skos:prefLabel "tuner autokeras image regression" ;
    :category :parameter ;
    skos:broader :tuner ;
    :has_datatype :single_value ;
    :parameter_value :greedy , :bayesian , :random , :hyperband ;
    rdfs:comment "Selecting the tuner approach for training" ;
    rdfs:seeAlso <https://autokeras.com> .
:tuner_autokeras_image_classification a :Configuration_item ;
    skos:prefLabel "tuner autokeras image classification" ;
    :category :parameter ;
    skos:broader :tuner ;
    :has_datatype :single_value ;
    :parameter_value :greedy , :bayesian , :random , :hyperband ;
    rdfs:comment "Selecting the tuner approach for training" ;
    rdfs:seeAlso <https://autokeras.com> .
:tuner_autokeras_text_regression a :Configuration_item ;
    skos:prefLabel "tuner autokeras text regression" ;
    :category :parameter ;
    skos:broader :tuner ;
    :has_datatype :single_value ;
    :parameter_value :greedy , :bayesian , :random , :hyperband ;
    rdfs:comment "Selecting the tuner approach for training" ;
    rdfs:seeAlso <https://autokeras.com> .
:tuner_autokeras_text_classification a :Configuration_item ;
    skos:prefLabel "tuner autokeras text classification" ;
    :category :parameter ;
    skos:broader :tuner ;
    :has_datatype :single_value ;
    :parameter_value :greedy , :bayesian , :random , :hyperband ;
    rdfs:comment "Selecting the tuner approach for training" ;
    rdfs:seeAlso <https://autokeras.com> .
:tuner_autokeras_time_series_forecasting a :Configuration_item ;
    skos:prefLabel "tuner autokeras time series forecasting" ;
    :category :parameter ;
    skos:broader :tuner ;
    :has_datatype :single_value ;
    :parameter_value :greedy , :bayesian , :random , :hyperband ;
    rdfs:comment "Selecting the tuner approach for training" ;
    rdfs:seeAlso <https://autokeras.com> .
:tuner_class_evalml a :Configuration_item ;
    skos:prefLabel "tuner class evalml" ;
    :category :parameter ;
    skos:broader :tuner ;
    :has_datatype :single_value ;
    :parameter_value :random , :grid_search , :skopt ;
    rdfs:comment "Selecting the tuner approach for training" ;
    rdfs:seeAlso <https://evalml.alteryx.com/en/stable/api_index.html> .
:tuner_class_gama a :Configuration_item ;
    skos:prefLabel "tuner class GAMA" ;
    :category :task_configuration ;
    skos:broader :tuner ;
    :has_datatype :single_value ;
    :parameter_value :random , :async_ea , :async_successive_halving ;
    rdfs:comment "Selecting the tuner approach for training" ;
    rdfs:seeAlso <https://openml-labs.github.io/gama/master/api/index.html> .
:loss_function a :Configuration_item ;
    skos:prefLabel "loss function" ;
    :category :parameter ;
    :has_datatype :single_value ;
    rdfs:comment "Selecting the loss function according to which training is optimized" ;
    rdfs:seeAlso <https://autokeras.com> .
:loss_function_autokeras_tabular_classification a :Configuration_item ;
    skos:prefLabel "loss function autokeras tabular classification" ;
    :category :parameter ;
    skos:broader :loss_function ;
    :has_datatype :single_value ;
    :parameter_value :binary_cross_entropy , :categorical_cross_entropy ;
    rdfs:comment "Selecting the loss function according to which training is optimized" ;
    rdfs:seeAlso <https://autokeras.com> .
:loss_function_autokeras_tabular_regression a :Configuration_item ;
    skos:prefLabel "loss function autokeras tabular regression" ;
    :category :parameter ;
    skos:broader :loss_function ;
    :has_datatype :single_value ;
    :parameter_value :mean_squared_error ;
    rdfs:comment "Selecting the loss function according to which training is optimized" ;
    rdfs:seeAlso <https://autokeras.com> .
:loss_function_autokeras_image_classification a :Configuration_item ;
    skos:prefLabel "loss function autokeras image classification" ;
    :category :parameter ;
    skos:broader :loss_function ;
    :has_datatype :single_value ;
    :parameter_value :binary_cross_entropy , :categorical_cross_entropy ;
    rdfs:comment "Selecting the loss function according to which training is optimized" ;
    rdfs:seeAlso <https://autokeras.com> .
:loss_function_autokeras_image_regression a :Configuration_item ;
    skos:prefLabel "loss function autokeras image regression" ;
    :category :parameter ;
    skos:broader :loss_function ;
    :has_datatype :single_value ;
    :parameter_value :mean_squared_error ;
    rdfs:comment "Selecting the loss function according to which training is optimized" ;
    rdfs:seeAlso <https://autokeras.com> .
:loss_function_autokeras_text_classification a :Configuration_item ;
    skos:prefLabel "loss function autokeras text classification" ;
    :category :parameter ;
    skos:broader :loss_function ;
    :has_datatype :single_value ;
    :parameter_value :binary_cross_entropy , :categorical_cross_entropy ;
    rdfs:comment "Selecting the loss function according to which training is optimized" ;
    rdfs:seeAlso <https://autokeras.com> .
:loss_function_autokeras_text_regression a :Configuration_item ;
    skos:prefLabel "loss function autokeras text regression" ;
    :category :parameter ;
    skos:broader :loss_function ;
    :has_datatype :single_value ;
    :parameter_value :mean_squared_error ;
    rdfs:comment "Selecting the loss function according to which training is optimized" ;
    rdfs:seeAlso <https://autokeras.com> .
:loss_function_autokeras_time_series_forecasting a :Configuration_item ;
    skos:prefLabel "loss function autokeras time series forecasting" ;
    :category :parameter ;
    skos:broader :loss_function ;
    :has_datatype :single_value ;
    :parameter_value :mean_squared_error ;
    rdfs:comment "Selecting the loss function according to which training is optimized" ;
    rdfs:seeAlso <https://autokeras.com> .
:loss_function_mcfly_time_series_classification a :Configuration_item ;
    skos:prefLabel "loss function mcfly time series classification" ;
    :category :parameter ;
    skos:broader :loss_function ;
    :has_datatype :single_value ;
    :parameter_value :categorical_cross_entropy ;
    rdfs:comment "Selecting the loss function according to which training is optimized" ;
    rdfs:seeAlso <https://mcfly.readthedocs.io/en/latest/reference.html> .
:loss_function_lama_tabular_classification a :Configuration_item ;
    skos:prefLabel "loss function lama tabular classification" ;
    :category :parameter ;
    skos:broader :loss_function ;
    :has_datatype :single_value ;
    :parameter_value :categorical_cross_entropy , :f_measure ;
    rdfs:comment "Selecting the loss function according to which training is optimized" ;
    rdfs:seeAlso <https://lightautoml.readthedocs.io/en/latest/pages/modules/generated/lightautoml.tasks.base.Task.html#lightautoml.tasks.base.Task> .
:loss_function_lama_tabular_regression a :Configuration_item ;
    skos:prefLabel "loss function lama tabular regression" ;
    :category :parameter ;
    skos:broader :loss_function ;
    :has_datatype :single_value ;
    :parameter_value :mean_squared_error , :mean_absolute_error , :mean_absolute_percentage_error , :root_mean_squared_log_error ;
    rdfs:comment "Selecting the loss function according to which training is optimized" ;
    rdfs:seeAlso <https://lightautoml.readthedocs.io/en/latest/pages/modules/generated/lightautoml.tasks.base.Task.html#lightautoml.tasks.base.Task> .
:loss_function_lama_binary_classification a :Configuration_item ;
    skos:prefLabel "loss function lama binary classification" ;
    :category :parameter ;
    skos:broader :loss_function ;
    :has_datatype :single_value ;
    :parameter_value :log_loss ;
    rdfs:comment "Selecting the loss function according to which training is optimized" ;
    rdfs:seeAlso <https://lightautoml.readthedocs.io/en/latest/pages/modules/generated/lightautoml.tasks.base.Task.html#lightautoml.tasks.base.Task> .
:forecasting_horizon a :Configuration_item ;
    skos:prefLabel "forecasting horizon" ;
    :category :parameter ;
    :has_datatype :integer ;
    :required "true"^^xsd:boolean ;
    rdfs:comment "Specifying the period for which forecasts are generated for a time series" .
:forecasting_horizon_autokeras_time_series_forcasting a :Configuration_item ;
    skos:prefLabel "forecasting horizon autokeras time series forcasting" ;
    :category :parameter ;
    skos:broader :forecasting_horizon ;
    :has_datatype :integer ;
    rdfs:comment "Specifying the period for which forecasts are generated for a time series" ;
    rdfs:seeAlso <https://autokeras.com> .
:forecasting_horizon_autogluon_time_series_forcasting a :Configuration_item ;
    skos:prefLabel "forecasting horizon autogluon time series forcasting" ;
    :category :parameter ;
    skos:broader :forecasting_horizon ;
    :has_datatype :integer ;
    rdfs:comment "Specifying the period for which forecasts are generated for a time series" ;
    rdfs:seeAlso <https://auto.gluon.ai> .
:forecasting_horizon_evalml_time_series_forcasting a :Configuration_item ;
    skos:prefLabel "forecasting horizon evalml time series forcasting" ;
    :category :parameter ;
    skos:broader :forecasting_horizon ;
    :has_datatype :integer ;
    rdfs:comment "Specifying the period for which forecasts are generated for a time series" ;
    rdfs:seeAlso <https://evalml.alteryx.com/en/stable/api_index.html> .
:forecasting_horizon_flaml_time_series_forcasting a :Configuration_item ;
    skos:prefLabel "forecasting horizon flaml time series forcasting" ;
    :category :parameter ;
    skos:broader :forecasting_horizon ;
    :has_datatype :integer ;
    rdfs:comment "Specifying the period for which forecasts are generated for a time series" ;
    rdfs:seeAlso <https://microsoft.github.io/FLAML/docs/reference/automl/automl> .
:forecasting_horizon_pycaret_time_series_forcasting a :Configuration_item ;
    skos:prefLabel "forecasting horizon pycaret time series forcasting" ;
    :category :parameter ;
    skos:broader :forecasting_horizon ;
    :has_datatype :integer ;
    rdfs:comment "Specifying the period for which forecasts are generated for a time series" ;
    rdfs:seeAlso <https://pycaret.readthedocs.io> .
:forecasting_horizon_autopytorch_time_series_forcasting a :Configuration_item ;
    skos:prefLabel "forecasting horizon autopytorch time series forcasting" ;
    :category :parameter ;
    skos:broader :forecasting_horizon ;
    :has_datatype :integer ;
    rdfs:comment "Specifying the period for which forecasts are generated for a time series" .
:lookback a :Configuration_item ;
    skos:prefLabel "lookback" ;
    :category :parameter ;
    :has_datatype :integer .
:lookback_autokeras_time_series_forecasting a :Configuration_item ;
    skos:prefLabel "lookback autokeras time series forecasting" ;
    :category :parameter ;
    skos:broader :lookback ;
    :has_datatype :integer ;
    rdfs:seeAlso <https://autokeras.com> .
:lookback_evalml_time_series_forecasting a :Configuration_item ;
    skos:prefLabel "lookback evalml time series forecasting" ;
    :category :parameter ;
    skos:broader :lookback ;
    :has_datatype :integer ;
    :required "true"^^xsd:boolean ;
    rdfs:seeAlso <https://evalml.alteryx.com/en/stable/api_index.html> .
:gap a :Configuration_item ;
    skos:prefLabel "gap" ;
    :category :parameter ;
    :has_datatype :integer .
:gap_autokeras_time_series_forecasting a :Configuration_item ;
    skos:prefLabel "gap autokeras time series forecasting" ;
    :category :parameter ;
    skos:broader :gap ;
    :has_datatype :integer ;
    rdfs:seeAlso <https://autokeras.com> .
:gap_evalml_time_series_forecasting a :Configuration_item ;
    skos:prefLabel "gap evalml time series forecasting" ;
    :category :parameter ;
    skos:broader :gap ;
    :has_datatype :integer ;
    :required "true"^^xsd:boolean ;
    rdfs:seeAlso <https://evalml.alteryx.com/en/stable/api_index.html> .
:validation_split a :Configuration_item ;
    skos:prefLabel "validation split" ;
    :category :parameter ;
    :has_datatype :integer .
:validation_split_autokeras a :Configuration_item ;
    skos:prefLabel "validation split autokeras" ;
    :category :parameter ;
    skos:broader :validation_split ;
    :has_datatype :integer ;
    rdfs:seeAlso <https://autokeras.com> .
:validation_split_flaml a :Configuration_item ;
    skos:prefLabel "validation split flaml" ;
    :category :parameter ;
    skos:broader :validation_split ;
    :has_datatype :integer ;
    rdfs:seeAlso <https://microsoft.github.io/FLAML/docs/reference/automl/automl> .
:eval_method a :Configuration_item ;
    skos:prefLabel "eval method" ;
    :category :parameter ;
    :has_datatype :single_value ;
    rdfs:comment "Specifying the method for validating the prediction performance" .
:eval_method_flaml a :Configuration_item ;
    skos:prefLabel "eval method Flaml" ;
    :category :parameter ;
    skos:broader :eval_method ;
    :has_datatype :single_value ;
    :parameter_value :auto_evaluation , :cross_validation , :holdout ;
    rdfs:comment "Specifying the method for validating the prediction performance" ;
    rdfs:seeAlso <https://microsoft.github.io/FLAML/docs/reference/automl/automl> .
:cross_validation_fold a :Configuration_item ;
    skos:prefLabel "cross validation fold" ;
    :category :parameter ;
    :has_datatype :integer .
:cross_validation_fold_flaml a :Configuration_item ;
    skos:prefLabel "cross validation fold flaml" ;
    :category :parameter ;
    skos:broader :cross_validation_fold ;
    :has_datatype :integer .
:cross_validation_fold_pycaret a :Configuration_item ;
    skos:prefLabel "cross validation fold pycaret" ;
    :category :parameter ;
    skos:broader :cross_validation_fold ;
    :has_datatype :integer .
:split_type a :Configuration_item ;
    skos:prefLabel "split type" ;
    :category :parameter ;
    :has_datatype :single_value .
:split_type_flaml_classification a :Configuration_item ;
    skos:prefLabel "split type flaml classification" ;
    :category :parameter ;
    skos:broader :split_type ;
    :has_datatype :single_value ;
    :parameter_value :auto_split , :stratified , :uniform , :time , :group .
:split_type_flaml_regression a :Configuration_item ;
    skos:prefLabel "split type flaml regression" ;
    :category :parameter ;
    skos:broader :split_type ;
    :has_datatype :single_value ;
    :parameter_value :auto_split , :uniform , :time .
:split_type_flaml_time_series_forecasting a :Configuration_item ;
    skos:prefLabel "split type flaml time series forecasting" ;
    :category :parameter ;
    skos:broader :split_type ;
    :has_datatype :single_value ;
    :parameter_value :auto_split , :time .
:split_type_flaml_ranking a :Configuration_item ;
    skos:prefLabel "split type flaml ranking" ;
    :category :parameter ;
    skos:broader :split_type ;
    :has_datatype :single_value ;
    :parameter_value :auto_split , :group .
:hyperparameter_optimization_method a :Configuration_item ;
    skos:prefLabel "hyperparameter optimization method" ;
    :category :parameter ;
    :has_datatype :single_value .
:hyperparameter_optimization_method_flaml a :Configuration_item ;
    skos:prefLabel "hyperparameter optimization method flaml" ;
    :category :parameter ;
    skos:broader :hyperparameter_optimization_method ;
    :has_datatype :single_value ;
    :parameter_value :auto_optimization_approach , :blendsearch , :frugal_optimization_for_costrelated_hyperparameters .
:optimize_thresholds a :Configuration_item ;
    skos:prefLabel "optimize thresholds" ;
    :category :parameter ;
    :has_datatype :boolean .
:optimize_thresholds_evalml a :Configuration_item ;
    skos:prefLabel "optimize thresholds evalml" ;
    :category :parameter ;
    skos:broader :optimize_thresholds ;
    :has_datatype :boolean .
:ensembling a :Configuration_item ;
    skos:prefLabel "ensembling" ;
    :category :parameter ;
    :has_datatype :boolean .
:ensembling_evalml a :Configuration_item ;
    skos:prefLabel "ensembling evalml" ;
    :category :parameter ;
    skos:broader :ensembling ;
    :has_datatype :boolean .
:max_batches a :Configuration_item ;
    skos:prefLabel "max batches" ;
    :category :parameter ;
    :has_datatype :integer .
:max_batches_evalml a :Configuration_item ;
    skos:prefLabel "max batches evalml" ;
    :category :parameter ;
    skos:broader :max_batches ;
    :has_datatype :integer .
:allow_long_running_models a :Configuration_item ;
    skos:prefLabel "allow long running models" ;
    :category :parameter ;
    :has_datatype :boolean .
:allow_long_running_models_evalml a :Configuration_item ;
    skos:prefLabel "allow long running models evalml" ;
    :category :parameter ;
    skos:broader :allow_long_running_models ;
    :has_datatype :boolean .
:pipelines_per_batch a :Configuration_item ;
    skos:prefLabel "pipelines per batch" ;
    :category :parameter ;
    :has_datatype :integer .
:pipelines_per_batch_evalml a :Configuration_item ;
    skos:prefLabel "pipelines per batch evalml" ;
    :category :parameter ;
    skos:broader :pipelines_per_batch ;
    :has_datatype :integer .
:exclude_featurizers a :Configuration_item ;
    skos:prefLabel "exclude featurizers" ;
    :category :parameter ;
    :has_datatype :list .
:exclude_featurizers_evalml a :Configuration_item ;
    skos:prefLabel "exclude featurizers evalml" ;
    :category :parameter ;
    skos:broader :exclude_featurizers ;
    :has_datatype :list ;
    :parameter_value :datetime_featurizer , :email_featurizer , :url_featurizer , :natural_language_featurizer , :time_series_featurizer .
:max_models a :Configuration_item ;
    skos:prefLabel "max models" ;
    :category :parameter ;
    :has_datatype :integer .
:max_models_h2o_automl a :Configuration_item ;
    skos:prefLabel "max models h2o AutoML" ;
    :category :parameter ;
    skos:broader :max_models ;
    :has_datatype :integer .
:sort_metric a :Configuration_item ;
    skos:prefLabel "sort metric" ;
    :category :parameter ;
    :has_datatype :single_value .
:sort_metric_h2o_automl a :Configuration_item ;
    skos:prefLabel "sort metric h2o AutoML" ;
    :category :parameter ;
    skos:broader :sort_metric ;
    :has_datatype :single_value ;
    :parameter_value :accuracy , :area_under_roc_curve , :area_under_precision_recall_curve , :log_loss , :mean_absolute_error , :mean_per_class_error , :mean_residual_deviance , :root_mean_squared_error , :root_mean_squared_log_error .
:number_clusters a :Configuration_Item ;
    skos:prefLabel "Number Clusters" ;
    :category :parameter ;
    :has_datatype :integer .
:number_clusters_pycaret_clustering a :Configuration_Item ;
    skos:prefLabel "Number Clusters Pycaret Clustering" ;
    :category :parameter ;
    skos:broader :number_clusters ;
    :has_datatype :integer .


# Enum

:category_type a :Enum ;
    skos:prefLabel "category type" ;
    :category :category_type ;
    rdfs:comment "Category for specifying category types of enums in the ML ontology" .
:datatype a :Enum ;
    skos:prefLabel "datatype" ;
    :category :category_type ;
    rdfs:comment "Category type for specifying datatypes, e.g., of parameters, in the ML ontology" .
:task_configuration a :Enum ;
    skos:prefLabel "task configuration" ;
    :category :category_type ;
    rdfs:comment "Category type for specifying configurations of AutoML solutions in class :Configuration_item" .
:parameter a :Enum ;
    skos:prefLabel "parameter" ;
    :category :category_type ;
    rdfs:comment "Category type for specifying parameters AutoML solutions in class :Configuration_item" .
:hardware a :Enum ;
    skos:prefLabel "hardware" ;
    :category :category_type ;
    rdfs:comment "Category for specifying hardware, e.g., for configuring AutoML solutions" .
:characteristic a :Enum ;
    skos:prefLabel "characteristic" ;
    :category :category_type ;
    rdfs:comment "Category for specifying basic properties of datasets or ML approaches that can be used to chacterize ML approaches or ML prediction performance measures; e.g., balanced / unbalanced datasets that influence the choice of ML prediction performance measures." .
:dataset_type a :Enum ;
    skos:prefLabel "dataset type" ;
    :category :category_type ;
    rdfs:comment "Category for specifying types of datasets, e.g., tabular, text, image, etc." .
:tuner_approach a :Enum ;
    skos:prefLabel "tuner approach" ;
    :category :category_type ;
    rdfs:comment "Category type for specifying tuner approaches, to be used in class :Configuration_item" .
:inheritance_type a :Enum ;
    skos:prefLabel "inheritance type" ;
    :category :category_type ;
    rdfs:comment "Category for specifying inheritance types of properties, to be used for SPARQL inferencing" .
:column_role a :Enum ;
    skos:prefLabel "column role" ;
    :category :category_type ;
    rdfs:comment "Category for specifying roles of culumns in a dataset, e.g., prediction target" .
:evaluation_approach a :Enum ;
    skos:prefLabel "evaluation approach" ;
    :category :category_type ;
    rdfs:comment "Category type for specifying eval methods, to be used in class :Configuration_item" .
:split_approach a :Enum ;
    skos:prefLabel "split approach" ;
    :category :category_type ;
    rdfs:comment "Category type for specifying split types, to be used in class :Configuration_item" .
:hyperparameter_optimization_approach a :Enum ;
    skos:prefLabel "hyperparameter optimization approach" ;
    :category :category_type ;
    rdfs:comment "Category type for specifying hyperparameter optimization approaches, to be used in class :Configuration_item" .
:featurizers a :Enum ;
    skos:prefLabel "featurizers" ;
    :category :category_type ;
    rdfs:comment "Category type for specifying featurizers, to be used in class :Configuration_item" .
:integer a :Enum ;
    skos:prefLabel "integer" ;
    skos:altLabel "int" ;
    :category :datatype ;
    rdfs:comment "Datatype for representing integer numbers, e.g., 42" ;
    rdfs:seeAlso <https://www.wikidata.org/entity/Q729138> .
:float a :Enum ;
    skos:prefLabel "float" ;
    :category :datatype ;
    rdfs:comment "Datatype for representing floating point numbers, e.g., 3.14" ;
    rdfs:seeAlso <https://www.wikidata.org/entity/Q117879> .
:boolean a :Enum ;
    skos:prefLabel "boolean" ;
    skos:altLabel "bool" ;
    :category :datatype ;
    rdfs:comment "Datatype for representing boolean values, i.e., true and false" ;
    rdfs:seeAlso <https://www.wikidata.org/entity/Q520777> .
:string a :Enum ;
    skos:prefLabel "string" ;
    :category :datatype ;
    rdfs:comment "Datatype for representing a sequence of characters, e.g., 'hello world'" ;
    rdfs:seeAlso <https://www.wikidata.org/entity/Q184754> .
:categorical a :Enum ;
    skos:prefLabel "categorical" ;
    :category :datatype ;
    rdfs:comment "Datatype for representing categorical variables that can take on one of a limited, and usually fixed, number of possible values, e.g., low, medium, high" ;
    rdfs:seeAlso <https://www.wikidata.org/entity/Q2285707> .
:datetime a :Enum ;
    skos:prefLabel "datetime" ;
    :category :datatype ;
    rdfs:comment "Datatype for representing a date and time" ;
    rdfs:seeAlso <https://www.wikidata.org/entity/Q116880167> .
:list a :Enum ;
    skos:prefLabel "list" ;
    :category :datatype ;
    rdfs:comment "Denotes a collection of options which are provided as a parameter of a :Configuration_item" .
:single_value a :Enum ;
    skos:prefLabel "single value" ;
    :category :datatype ;
    rdfs:comment "Denotes a single value from a list of options which is provided as a parameter of a :Configuration_item" .
:index a :Enum ;
    skos:prefLabel "index" ;
    :category :column_role ;
    rdfs:comment "Marks a column of a dataset as index which can be used to uniquely identify individual rows but which should not be used as a feature for ML training." .
:target a :Enum ;
    skos:prefLabel "target" ;
    :category :column_role ;
    rdfs:comment "Marks a column of a dataset as the prediction target (goal) for machine learning, e.g, in classification or regression." .
:ignore a :Enum ;
    skos:prefLabel "ignore" ;
    :category :column_role ;
    rdfs:comment "Marks a column of a dataset as to be ignored / omitted as a feature for training a ML model." .
:balanced_dataset a :Enum ;
    skos:prefLabel "balanced dataset" ;
    :category :characteristic ;
    rdfs:comment "Characterizes balanced datasets, i.e., datasets with an even distribution of target classes." .
:unbalanced_dataset a :Enum ;
    skos:prefLabel "unbalanced dataset" ;
    :category :characteristic ;
    rdfs:comment "Characterizes unbalanced datasets, i.e., datasets with an uneven distribution of target classes." .
:missing_values a :Enum ;
    skos:prefLabel "missing values" ;
    :category :characteristic ;
    rdfs:comment "Characterizes dataset columns to have missing values" .
:numerical_features a :Enum ;
    skos:prefLabel "numerical features" ;
    :category :characteristic ;
    rdfs:comment "Characterizes datasets to have features (columns) of numeric datatypes" .
:categorical_features a :Enum ;
    skos:prefLabel "categorical features" ;
    :category :characteristic ;
    rdfs:comment "Characterizes datasets to have categorical features (columns), i.e. with a limited number of values, e.g., low, medium, high" .
:text_features a :Enum ;
    skos:prefLabel "text features" ;
    :category :characteristic ;
    rdfs:comment "Characterizes datasets to have textual features (columns) , i.e., with datatype string" .
:small_dataset a :Enum ;
    skos:prefLabel "small dataset" ;
    :category :characteristic ;
    rdfs:comment "Denotes a dataset of relatively small size, i.e., with only a few thousand samples" .
:large_dataset a :Enum ;
    skos:prefLabel "large dataset" ;
    :category :characteristic ;
    rdfs:comment "Denotes a dataset of relatively large size, i.e., with at least tens of thousands of samples" .
:fast_training a :Enum ;
    skos:prefLabel "fast training" ;
    :category :characteristic ;
    rdfs:comment "Characterizes a reatively short training time compared to a training with an ML model of different type with the same dataset, e.g., training a knn model" .
:long_training_time a :Enum ;
    skos:prefLabel "long training time" ;
    :category :characteristic ;
    rdfs:comment "Characterizes a reatively long training time compared to a training with an ML model of different type with the same dataset, e.g., training a deep neural network" .
:many_features a :Enum ;
    skos:prefLabel "many features" ;
    :category :characteristic ;
    rdfs:comment "Chacterizes a dataset with a relatively large number of features (columns), i.e., more than 1,000" .
:accurate a :Enum ;
    skos:prefLabel "accurate" ;
    :category :characteristic ;
    rdfs:comment "Characterizes an ML model type to usually produces a better prediction performance than other model types trained with the same dataset, e.g., neural networks" .
:small_memory_footprint a :Enum ;
    skos:prefLabel "small memory footprint" ;
    :category :characteristic ;
    rdfs:comment "Characterizes an ML model type with relatively small energy consumption for training and prediction compared to other ML models, e.g., decision trees" .
:large_memory_footprint a :Enum ;
    skos:prefLabel "large memory footprint" ;
    :category :characteristic ;
    rdfs:comment "Characterizes an ML model type with relatively large energy consumption for training and prediction compared to other ML models, e.g., neural networks" .
:explainable a :Enum ;
    skos:prefLabel "explainable" ;
    :category :characteristic ;
    rdfs:comment "Characterizes an ML model type to allow humans to interpret the reasoning for a prediction, e.g., decision trees" .
:scalable a :Enum ;
    skos:prefLabel "scalable" ;
    :category :characteristic ;
    rdfs:comment "Characterizes an ML model type to be scaled to very large datasets (big data)" .
:tabular a :Enum ;
    skos:prefLabel "tabular" ;
    :category :dataset_type ;
    rdfs:comment "A dataset presented in a tabular form, i.e., a table with rows and columns in comma-separated value format [filetype: *.csv, *.xlsx, *.xls, *.arff]" ;
    :supported_by_oma_ml "true"^^xsd:boolean .
:text a :Enum ;
    skos:prefLabel "text" ;
    :category :dataset_type ;
    rdfs:comment "A dataset containing texts. The dataset must be represented as a table with rows and one or more text columns [filetype: *.csv, *.xlsx, *.xls, *.arff]" ;
    :supported_by_oma_ml "true"^^xsd:boolean .
:image a :Enum ;
    skos:prefLabel "image" ;
    :category :dataset_type ;
    rdfs:comment "A dataset containing images in some common format, e.g., *.jpg. Image files must be stored in a zipped folder structure with 'train' and 'test' subdirectories each containing folders named according to the labels to be predicted [filetype: *.zip]" ;
    :supported_by_oma_ml "true"^^xsd:boolean .
:video a :Enum ;
    skos:prefLabel "video" ;
    :category :dataset_type ;
    rdfs:comment "A dataset containing video files" .
:audio a :Enum ;
    skos:prefLabel "audio" ;
    :category :dataset_type ;
    rdfs:comment "A dataset containing audio files" .
:graph a :Enum ;
    skos:prefLabel "graph" ;
    :category :dataset_type ;
    rdfs:comment "A dataset containing graphs" .
:time_series_longitudinal a :Enum ;
    skos:prefLabel "time series longitudinal" ;
    :category :dataset_type ;
    rdfs:comment "Longitudinal data are data in which each variable is measured repeatedly over time. A dataset of longitudinal data (also called panel data) for time series classification has 3 dimensions: num_samples, num_features, num_timesteps [filetype: *.ts]" ;
    rdfs:seeAlso <https://www.stathelp.se/en/xtset_en.html> .
:time_series a :Enum ;
    skos:prefLabel "time series" ;
    :category :dataset_type ;
    rdfs:comment "A dataset for time series data, represented as a table with rows and columns ordered according to a timestamp column [filetype: *.csv, *.xlsx, *.xls, *.arff]" ;
    rdfs:seeAlso <https://auto.gluon.ai/stable/tutorials/timeseries/forecasting-quick-start.html#loading-time-series-data-as-a-timeseriesdataframe> ;
    :supported_by_oma_ml "true"^^xsd:boolean .
:greedy a :Enum ;
    skos:prefLabel "greedy" ;
    :category :tuner_approach ;
    rdfs:comment "Greedy approach for ML model tuning" .
:bayesian a :Enum ;
    skos:prefLabel "bayesian" ;
    :category :tuner_approach ;
    rdfs:comment "Baysian approach for ML model tuning" .
:hyperband a :Enum ;
    skos:prefLabel "hyperband" ;
    :category :tuner_approach ;
    rdfs:comment "Hyperband approach for ML model tuning" .
:random a :Enum ;
    skos:prefLabel "random" ;
    :category :tuner_approach ;
    rdfs:comment "Random approach for ML model tuning" .
:grid_search a :Enum ;
    skos:prefLabel "grid search" ;
    :category :tuner_approach ;
    rdfs:comment "Grid search approach for ML model tuning" .
:skopt a :Enum ;
    skos:prefLabel "skopt" ;
    :category :tuner_approach ;
    rdfs:comment "skopt approach for ML model tuning" .
:async_successive_halving a :Enum ;
    skos:prefLabel "async successive halving" ;
    :category :tuner_approach ;
    rdfs:comment "Async successive halving approach for ML model tuning" .
:async_ea a :Enum ;
    skos:prefLabel "async ea" ;
    :category :tuner_approach ;
    rdfs:comment "Asynchronous approach for ML model tuning" .
:broader_inherited a :Enum ;
    skos:prefLabel "broader inherited" ;
    :category :inheritance_type ;
    rdfs:comment "Denotes that an RDF object can be inherited via SPARQL inferencing from one RDF subject to another if they are in a skos:broader relationship. Example: :artificial_neural_network :used_for :classification. :convolutional_neural_network skos:broader :artificial_neural_network. => :convolutional_neural_network :used_for :classification." .
:auto_evaluation a :Enum ;
    skos:prefLabel "auto evaluation" ;
    :category :evaluation_approach .
:cross_validation a :Enum ;
    skos:prefLabel "cross validation" ;
    :category :evaluation_approach .
:holdout a :Enum ;
    skos:prefLabel "holdout" ;
    :category :evaluation_approach .
:auto_split a :Enum ;
    skos:prefLabel "auto split" ;
    :category :split_approach .
:stratified a :Enum ;
    skos:prefLabel "stratified" ;
    :category :split_approach .
:uniform a :Enum ;
    skos:prefLabel "uniform" ;
    :category :split_approach .
:time a :Enum ;
    skos:prefLabel "time" ;
    :category :split_approach .
:group a :Enum ;
    skos:prefLabel "group" ;
    :category :split_approach .
:auto_optimization_approach a :Enum ;
    skos:prefLabel "auto optimization approach" ;
    :category :hyperparameter_optimization_approach .
:blendsearch a :Enum ;
    skos:prefLabel "BlendSearch" ;
    :category :hyperparameter_optimization_approach .
:frugal_optimization_for_costrelated_hyperparameters a :Enum ;
    skos:prefLabel "Frugal Optimization for Costrelated Hyperparameters" ;
    skos:altLabel "CFO" ;
    :category :hyperparameter_optimization_approach .
:datetime_featurizer a :Enum ;
    skos:prefLabel "Datetime Featurizer" ;
    :category :featurizers .
:email_featurizer a :Enum ;
    skos:prefLabel "Email Featurizer" ;
    :category :featurizers .
:url_featurizer a :Enum ;
    skos:prefLabel "URL Featurizer" ;
    :category :featurizers .
:natural_language_featurizer a :Enum ;
    skos:prefLabel "Natural Language Featurizer" ;
    :category :featurizers .
:time_series_featurizer a :Enum ;
    skos:prefLabel "Time Series Featurizer" ;
    :category :featurizers .


# spSelect Queries

:query_get_all_dataset_types a sp:Select ;
    skos:prefLabel "Query get all dataset types" ;
    sp:text '''PREFIX : <http://h-da.de/ml-ontology/>
SELECT ?t
WHERE {
        ?t a :Enum;
           :category :dataset_type .
}''' ;
    rdfs:comment "SPARQL query to get all dataset types" .
:query_get_all_ml_tasks a sp:Select ;
    skos:prefLabel "Query get all ML tasks" ;
    sp:text '''PREFIX : <http://h-da.de/ml-ontology/>
SELECT ?t ?a
WHERE {
        ?t a :ML_task;
           :belongs_to ?a .
}''' ;
    rdfs:comment "SPARQL query to get all ML tasks an the ML areas they belong to" .
:query_get_all_ml_approaches a sp:Select ;
    skos:prefLabel "Query get all ML approaches" ;
    sp:text '''PREFIX : <http://h-da.de/ml-ontology/>
SELECT *
WHERE {
        ?a a :ML_approach;
           :used_for ?t .
}''' ;
    rdfs:comment "SPARQL query to get all ML approaches and the ML tasks they can be used for" .
:query_get_all_preprocessing_approaches a sp:Select ;
    skos:prefLabel "Query get all preprocessing approaches" ;
    sp:text '''PREFIX : <http://h-da.de/ml-ontology/>
SELECT *
WHERE {
        ?p a :Preprocessing_approach.
                  OPTIONAL {?p :used_for ?t} .
}''' ;
    rdfs:comment "SPARQL query to get all preprocessing approaches and the ML tasks they can be used for" .
:query_get_all_metrics a sp:Select ;
    skos:prefLabel "Query get all metrics" ;
    sp:text '''PREFIX : <http://h-da.de/ml-ontology/>
SELECT *
WHERE {
        ?m a :Metric;
           :used_for ?t .
}''' ;
    rdfs:comment "SPARQL query to get all performance metrics the the ML tasks they can be used for" .
:query_get_all_ml_libraries a sp:Select ;
    skos:prefLabel "Query get all ML libraries" ;
    sp:text '''PREFIX : <http://h-da.de/ml-ontology/>
PREFIX skos: <http://www.w3.org/2004/02/skos/core#>
SELECT *
WHERE {
        ?m a :ML_library ;
           skos:prefLabel ?l.
}''' ;
    rdfs:comment "SPARQL query to get all ML libraries with their names" .
:query_get_all_automl_solutions a sp:Select ;
    skos:prefLabel "Query get all AutoML solutions" ;
    sp:text '''PREFIX : <http://h-da.de/ml-ontology/>
SELECT *
WHERE {
        ?a a :AutoML_solution ;
           :used_for ?l.
}''' ;
    rdfs:comment "SPARQL query to get AutoML solutions and the ML libraries they are used for" .
:query_get_all_predefined_sparql_queries a sp:Select ;
    skos:prefLabel "Query get all predefined SPARQL queries" ;
    sp:text '''PREFIX : <http://h-da.de/ml-ontology/>
PREFIX skos: <http://www.w3.org/2004/02/skos/core#>
PREFIX sp: <http://spinrdf.org/sp#>
PREFIX rdfs: <http://www.w3.org/2000/01/rdf-schema#>
SELECT *
WHERE {
        ?q a sp:Select ;
           sp:text ?t;
           rdfs:comment ?c .
}''' ;
    rdfs:comment "SPARQL query to get all predefined SPARQL queries" .
:query_get_all_predefined_sparql_insert_inference_rules a sp:Select ;
    skos:prefLabel "Query get all predefined SPARQL insert inference rules" ;
    sp:text '''PREFIX : <http://h-da.de/ml-ontology/>
PREFIX skos: <http://www.w3.org/2004/02/skos/core#>
PREFIX sp: <http://spinrdf.org/sp#>
PREFIX rdfs: <http://www.w3.org/2000/01/rdf-schema#>
SELECT *
WHERE {
        ?q a sp:InsertData ;
           sp:text ?t;
           rdfs:comment ?c .
}''' ;
    rdfs:comment "SPARQL query to get all predefined SPARQL insert inference rules" .


# spInsertData Inferencing

:inference_rule_broader_inheritance a sp:InsertData ;
    skos:prefLabel "Inference rule broader inheritance" ;
    sp:text '''PREFIX : <http://h-da.de/ml-ontology/>
PREFIX rdf: <http://www.w3.org/1999/02/22-rdf-syntax-ns#>
PREFIX skos: <http://www.w3.org/2004/02/skos/core#>
INSERT {?s ?p ?o .}
WHERE  {?p a rdf:Property ;
                        :inheritance :broader_inherited .
        ?s skos:broader+ ?b .
        ?b ?p ?o .}''' ;
    rdfs:comment "SPARQL update statement to insert new triples with subjects that are in a (transitive) skos:broader relationship for existing triples with a predicate of inheritance type :broader_inherited" .


# spSelect Quality Checks

:check_class_instance a sp:Select ;
    skos:prefLabel "Check class instance" ;
    sp:text '''PREFIX : <http://h-da.de/ml-ontology/>
SELECT ?class ?subject ?predicate ?object
WHERE {
        ?subject ?predicate ?object .
        OPTIONAL {?subject a ?class .}
        FILTER isIRI(?object)
        FILTER(STRSTARTS(str(?object), str(:)))
        FILTER NOT EXISTS {?object a ?c}
}''' ;
    rdfs:comment "All objects should be instances of some class -> ok if query returns nothing; otherwise check ?object of triple in ?class" .
:check_unique_class a sp:Select ;
    skos:prefLabel "Check unique class" ;
    sp:text '''PREFIX : <http://h-da.de/ml-ontology/>
SELECT DISTINCT ?subject ?class1 ?class2
WHERE {
        ?subject a ?class1 .
        ?subject a ?class2 .
        FILTER(?class1 != ?class2)
}''' ;
    rdfs:comment "No object should be instance of several classes -> ok if query retuns nothing; otherwise check redundant ?class1 and ?class2" .
:check_predicate_declared a sp:Select ;
    skos:prefLabel "Check predicate declared" ;
    sp:text '''PREFIX : <http://h-da.de/ml-ontology/>
PREFIX rdf: <http://www.w3.org/1999/02/22-rdf-syntax-ns#>
SELECT DISTINCT ?predicate
WHERE {
        ?s ?predicate ?o .
        FILTER(STRSTARTS(str(?predicate), str(:)))
        FILTER NOT EXISTS {?predicate a rdf:Property}
}''' ;
    rdfs:comment "Predicates should be declared -> ok if query returns nothing; otherwise check ?predicate" .
:check_predicates_with_domain_and_range_datatypes a sp:Select ;
    skos:prefLabel "Check predicates with domain and range datatypes" ;
    sp:text '''PREFIX : <http://h-da.de/ml-ontology/>
PREFIX rdf: <http://www.w3.org/1999/02/22-rdf-syntax-ns#>
PREFIX rdfs: <http://www.w3.org/2000/01/rdf-schema#>
PREFIX skos: <http://www.w3.org/2004/02/skos/core#>
SELECT DISTINCT ?predicate ?domain ?range
WHERE {
        ?s ?predicate ?o .
        ?s a ?domain .
        ?o a ?range .
}
ORDER BY ?predicate''' ;
    rdfs:comment "Lists all used predicates and their subject / object datatypes -> check whether subject datatypes (?domain) and object datatypes (?range) make sense" .
