### Ontology file generated from ML_Ontology.xlsx.
### 2023-02-17 14:34:47.237325


# PREFIXES

@prefix : <http://h-da.de/ml-ontology/> .
@prefix rdf: <http://www.w3.org/1999/02/22-rdf-syntax-ns#> .
@prefix rdfs: <http://www.w3.org/2000/01/rdf-schema#> .
@prefix xsd: <http://www.w3.org/2001/XMLSchema#> .
@prefix skos: <http://www.w3.org/2004/02/skos/core#> .


# rdfsClass

:ML_area a rdfs:Class ;
    skos:prefLabel "ML area" ;
    rdfs:comment "Broad category of ML, depending on the nature of the feedback available to the learning system; e.g., feedback by supervisor (supervised learning), without feedback (unsupervised learning), feedback by software application (reinforcement learning)." .
:ML_task a rdfs:Class ;
    skos:prefLabel "ML task" ;
    rdfs:comment "Problem that is to be solved by ML, e.g., assign categories to data records (classification), predict numeric values (regression), group data records (clustering), etc." .
:ML_approach a rdfs:Class ;
    skos:prefLabel "ML approach" ;
    rdfs:comment "A set of technologies suitable for solving ML tasks, e.g., artificial neural networks (including gradient descent, backpropagation, etc.)" .
:Preprocessing_approach a rdfs:Class ;
    skos:prefLabel "Preprocessing approach" ;
    rdfs:comment "A set of technologies suited for preprossing ML datasets" .
:Metric a rdfs:Class ;
    skos:prefLabel "Metric" ;
    rdfs:comment "Metric for assessing the prediction quality of a ML system based on a dataset, e.g., for classification tasks measures on values in a confusion matrix like accuracy, F1 score etc." .
:ML_library a rdfs:Class ;
    skos:prefLabel "ML library" ;
    rdfs:comment "Examples: scikit-learn, Tensorflow, Keras" .
:AutoML_solution a rdfs:Class ;
    skos:prefLabel "AutoML solution" ;
    rdfs:comment "Examples: Autosklearn for Scikit-learn, Auto-Keras for Keras, and Google AutoML for Tensorﬂow" .
:Configuration_item a rdfs:Class ;
    skos:prefLabel "Configuration item" ;
    rdfs:comment "Example configuration items for AutoML solutions: metric, time limit, memory limit etc." .
:Enum a rdfs:Class ;
    skos:prefLabel "Enum" ;
    rdfs:comment "Enumeration values for different categories" .


# rdfProperty

:automl_solution a rdf:Property ;
    skos:prefLabel "AutoML solution" ;
    rdfs:comment ":Configuration_item -> :AutoML_solution" .
:belongs_to a rdf:Property ;
    skos:prefLabel "belongs to" ;
    :inheritance :broader_inherited ;
    rdfs:comment "{ :ML_task, ML_approach} -> :ML_area" .
:can_perform a rdf:Property ;
    skos:prefLabel "can perform" ;
    rdfs:comment ":AutoML_solution -> :ML_task" .
:category a rdf:Property ;
    skos:prefLabel "category" ;
    rdfs:comment "{:Configuration_item, :Enum} -> :Enum" .
:constraint a rdf:Property ;
    skos:prefLabel "constraint" ;
    rdfs:comment ":Configuration_item -> string" .
:has_dataset_type a rdf:Property ;
    skos:prefLabel "has dataset type" ;
    rdfs:comment ":ML_task -> :Enum" .
:has_datatype a rdf:Property ;
    skos:prefLabel "has datatype" ;
    rdfs:comment ":Configuration_item -> :Enum" .
:inheritance a rdf:Property ;
    skos:prefLabel "inheritance" ;
    rdfs:comment "rdf:Property -> :Enum(:inheritance_type)" .
:ml_task a rdf:Property ;
    skos:prefLabel "ML task" ;
    rdfs:comment ":configuration_item -> :ML_task" .
:not_possible_if a rdf:Property ;
    skos:prefLabel "not possible if" ;
    :inheritance :broader_inherited ;
    rdfs:comment "{:ML_approach; :Preprocessing_approach} -> :Enum" .
:not_recommended_if a rdf:Property ;
    skos:prefLabel "not recommended if" ;
    :inheritance :broader_inherited ;
    rdfs:comment "{:ML_approach; :Metric} -> :Enum" .
:parameter_value a rdf:Property ;
    skos:prefLabel "parameter value" ;
    rdfs:comment ":Configuration_item -> {:Configuraiton_item; :Enum; :ML_approach; :Metric; :Proprocessing_approach}" .
:performance a rdf:Property ;
    skos:prefLabel "performance" ;
    :inheritance :broader_inherited ;
    rdfs:comment "{:ML_approach; :Preprocessing_approach} -> :Enum" .
:possible_if a rdf:Property ;
    skos:prefLabel "possible if" ;
    :inheritance :broader_inherited ;
    rdfs:comment "{:ML_approach; :Preprocessing_approach} -> :Enum" .
:recommended_if a rdf:Property ;
    skos:prefLabel "recommended if" ;
    :inheritance :broader_inherited ;
    rdfs:comment ":Metric -> :Enum" .
:supported_by_oma_ml a rdf:Property ;
    skos:prefLabel "supported by OMA-ML" ;
    rdfs:comment ":AutoML_solution -> boolean" .
:used_for a rdf:Property ;
    skos:prefLabel "used for" ;
    :inheritance :broader_inherited ;
    rdfs:comment "{:ML_approach, :Metric, :Preprocessing_approach} -> :ML_task; :AutoML_solution -> :ML_library" .


# ML_area

:supervised_learning a :ML_area ;
    skos:prefLabel "supervised learning" ;
    skos:altLabel "SL" ;
    rdfs:comment "Supervised learning (SL) is the machine learning task of learning a function that maps an input to an output based on example input-output pairs." ;
    rdfs:seeAlso <https://www.wikidata.org/entity/Q334384> .
:unsupervised_learning a :ML_area ;
    skos:prefLabel "unsupervised learning" ;
    skos:altLabel "UL" ;
    rdfs:comment "Unsupervised learning (UL) is a type of algorithm that learns patterns from untagged data." ;
    rdfs:seeAlso <https://www.wikidata.org/entity/Q1152135> .
:reinforcement_learning a :ML_area ;
    skos:prefLabel "reinforcement learning" ;
    skos:altLabel "RL" ;
    rdfs:comment "Reinforcement learning (RL) is an area of machine learning concerned with how intelligent agents ought to take actions in an environment in order to maximize the notion of cumulative reward." ;
    rdfs:seeAlso <https://www.wikidata.org/entity/Q830687> .


# ML_task

:action_recognition a :ML_task ;
    skos:prefLabel "action recognition" ;
    :belongs_to :supervised_learning ;
    :has_dataset_type :video .
:anomaly_detection a :ML_task ;
    skos:prefLabel "anomaly detection" ;
    :belongs_to :supervised_learning , :unsupervised_learning ;
    rdfs:comment "the identification of rare items, events or observations which raise suspicions by differing significantly from the expected or majority of the data" ;
    rdfs:seeAlso <https://www.wikidata.org/entity/Q3560506> .
:audio_classification a :ML_task ;
    skos:prefLabel "audio classification" ;
    skos:broader :classification ;
    :belongs_to :supervised_learning ;
    :has_dataset_type :audio .
:audio_regression a :ML_task ;
    skos:prefLabel "audio regression" ;
    skos:broader :regression ;
    :belongs_to :supervised_learning ;
    :has_dataset_type :audio .
:binary_classification a :ML_task ;
    skos:prefLabel "binary classification" ;
    skos:broader :classification ;
    :belongs_to :supervised_learning ;
    rdfs:comment "the task of classifying the elements of a given set into two groups (predicting which group each one belongs to) on the basis of a classification rule" ;
    rdfs:seeAlso <https://www.wikidata.org/entity/Q3560506> .
:classification a :ML_task ;
    skos:prefLabel "classification" ;
    :belongs_to :supervised_learning ;
    rdfs:comment "Prediction of discrete categorical values" .
:clustering a :ML_task ;
    skos:prefLabel "clustering" ;
    :belongs_to :unsupervised_learning ;
    rdfs:comment "task of grouping a set of objects in such a way that objects in the same group (called a cluster) are more similar (in some sense or another) to each other than to those in other groups" ;
    rdfs:seeAlso <https://www.wikidata.org/entity/Q622825> .
:collaborative_graph_filtering a :ML_task ;
    skos:prefLabel "collaborative graph filtering" ;
    :belongs_to :supervised_learning ;
    :has_dataset_type :graph .
:community_detection a :ML_task ;
    skos:prefLabel "community detection" ;
    :belongs_to :supervised_learning ;
    :has_dataset_type :graph ;
    rdfs:comment "organization of vertices in clusters, with many edges joining vertices of the same cluster and comparatively few edges joining vertices of different clusters." ;
    rdfs:seeAlso <https://www.wikidata.org/entity/Q105222918> .
:entity_extraction a :ML_task ;
    skos:prefLabel "entity extraction" ;
    :belongs_to :supervised_learning ;
    :has_dataset_type :text ;
    rdfs:comment "extraction of named entity mentions in unstructured text into pre-defined categories" ;
    rdfs:seeAlso <https://www.wikidata.org/entity/Q403574> .
:feature_extraction a :ML_task ;
    skos:prefLabel "feature extraction" ;
    skos:broader :feature_reduction ;
    :belongs_to :unsupervised_learning ;
    rdfs:comment "process of building informative, nonredundant derived values from an initial set of measured data to facilitate learning, generalization and interpretation" ;
    rdfs:seeAlso <https://www.wikidata.org/entity/Q1026626> .
:feature_reduction a :ML_task ;
    skos:prefLabel "feature reduction" ;
    skos:altLabel "dimension reduction" ;
    :belongs_to :unsupervised_learning ;
    rdfs:comment "process of reducing the number of features in a resource heavy computation without losing important information." .
:feature_selection a :ML_task ;
    skos:prefLabel "feature selection" ;
    skos:broader :feature_reduction ;
    :belongs_to :unsupervised_learning ;
    rdfs:comment "procedure in machine learning and statistics" ;
    rdfs:seeAlso <https://www.wikidata.org/entity/Q446488> .
:graph_matching a :ML_task ;
    skos:prefLabel "graph matching" ;
    :belongs_to :supervised_learning ;
    :has_dataset_type :graph ;
    rdfs:comment "problem of finding similarity between graphs" ;
    rdfs:seeAlso <https://www.wikidata.org/entity/Q39045684> .
:image_classification a :ML_task ;
    skos:prefLabel "image classification" ;
    skos:broader :classification ;
    :belongs_to :supervised_learning ;
    :has_dataset_type :image ;
    rdfs:comment "set of methods to group images" ;
    rdfs:seeAlso <https://www.wikidata.org/entity/Q98526763> ;
    :supported_by_oma_ml "True" .
:image_object_tracking a :ML_task ;
    skos:prefLabel "image object tracking" ;
    :belongs_to :supervised_learning ;
    :has_dataset_type :image .
:image_regression a :ML_task ;
    skos:prefLabel "image regression" ;
    skos:broader :regression ;
    :belongs_to :supervised_learning ;
    :has_dataset_type :image .
:image_segmentation a :ML_task ;
    skos:prefLabel "image segmentation" ;
    :belongs_to :supervised_learning , :unsupervised_learning ;
    :has_dataset_type :image ;
    rdfs:comment "division of an image into sets of pixels for further processing" ;
    rdfs:seeAlso <https://www.wikidata.org/wiki/Q56933> .
:instance_segmentation a :ML_task ;
    skos:prefLabel "instance segmentation" ;
    :belongs_to :supervised_learning ;
    :has_dataset_type :image ;
    rdfs:comment "Instance segmentation is a task for detecting and localizing an object in an image" .
:link_prediction a :ML_task ;
    skos:prefLabel "link prediction" ;
    :belongs_to :supervised_learning ;
    :has_dataset_type :graph ;
    rdfs:comment "problem in network theory of predicting the existence of an unobserved link between two entities in a network" ;
    rdfs:seeAlso <https://www.wikidata.org/entity/Q98925312> .
:multiclass_classification a :ML_task ;
    skos:prefLabel "multiclass classification" ;
    skos:broader :classification ;
    :belongs_to :supervised_learning ;
    rdfs:comment "problem of classifying instances into one of multiple classes" ;
    rdfs:seeAlso <https://www.wikidata.org/entity/Q6934605> .
:object_detection a :ML_task ;
    skos:prefLabel "object detection" ;
    :belongs_to :supervised_learning ;
    :has_dataset_type :image ;
    rdfs:comment "computer technology related to computer vision and image processing" ;
    rdfs:seeAlso <https://www.wikidata.org/entity/Q3045304> .
:outlier_detection a :ML_task ;
    skos:prefLabel "outlier detection" ;
    :belongs_to :supervised_learning ;
    :has_dataset_type :tabular ;
    rdfs:comment "the identification of rare items, events or observations which raise suspicions by differing significantly from the expected or majority of the data" ;
    rdfs:seeAlso <https://www.wikidata.org/entity/Q3560506> .
:ranking a :ML_task ;
    skos:prefLabel "ranking" ;
    :belongs_to :supervised_learning ;
    :has_dataset_type :tabular ;
    rdfs:comment "process of ordering items in a set by criteria" ;
    rdfs:seeAlso <https://www.wikidata.org/entity/Q526719> .
:recommendation a :ML_task ;
    skos:prefLabel "recommendation" ;
    :belongs_to :supervised_learning , :unsupervised_learning .
:regression a :ML_task ;
    skos:prefLabel "regression" ;
    :belongs_to :supervised_learning ;
    rdfs:comment "Prediction of continuous numerical values" ;
    rdfs:seeAlso <https://www.wikidata.org/entity/Q208042> .
:remote_sensing a :ML_task ;
    skos:prefLabel "remote sensing" ;
    :belongs_to :supervised_learning ;
    :has_dataset_type :image .
:sentence_similarity a :ML_task ;
    skos:prefLabel "sentence similarity" ;
    :belongs_to :supervised_learning ;
    :has_dataset_type :text .
:sentiment_analysis a :ML_task ;
    skos:prefLabel "sentiment analysis" ;
    :belongs_to :supervised_learning ;
    :has_dataset_type :text ;
    rdfs:comment "use of natural language processing, text analysis and computational linguistics to identify and extract subjective information in source materials" ;
    rdfs:seeAlso <https://www.wikidata.org/entity/Q2271421> .
:tabular_classification a :ML_task ;
    skos:prefLabel "tabular classification" ;
    skos:broader :classification ;
    :belongs_to :supervised_learning ;
    :has_dataset_type :tabular ;
    rdfs:comment "classification of data rows of a table" ;
    :supported_by_oma_ml "True" .
:tabular_regression a :ML_task ;
    skos:prefLabel "tabular regression" ;
    skos:broader :regression ;
    :belongs_to :supervised_learning ;
    :has_dataset_type :tabular ;
    rdfs:comment "prediction of continuous values for rows in a table" ;
    :supported_by_oma_ml "True" .
:text_analytics a :ML_task ;
    skos:prefLabel "text analytics" ;
    :belongs_to :supervised_learning , :unsupervised_learning ;
    :has_dataset_type :text ;
    rdfs:comment "Process of changing text documents that are unstructured  into structured data" .
:text_classification a :ML_task ;
    skos:prefLabel "text classification" ;
    skos:broader :classification ;
    :belongs_to :supervised_learning ;
    :has_dataset_type :text ;
    rdfs:comment "classification of texts" ;
    rdfs:seeAlso <https://www.wikidata.org/entity/Q102190569> ;
    :supported_by_oma_ml "True" .
:text_regression a :ML_task ;
    skos:prefLabel "text regression" ;
    skos:broader :regression ;
    :belongs_to :supervised_learning ;
    :has_dataset_type :text ;
    rdfs:comment "Process of mapping text to numerical values" .
:time_series_analysis a :ML_task ;
    skos:prefLabel "time series analysis" ;
    :belongs_to :supervised_learning ;
    :has_dataset_type :tabular ;
    rdfs:comment "area of statistics" ;
    rdfs:seeAlso <https://www.wikidata.org/entity/Q11850042> .
:time_series_classification a :ML_task ;
    skos:prefLabel "time series classification" ;
    skos:broader :classification ;
    :belongs_to :supervised_learning ;
    :has_dataset_type :time_series_longitudinal ;
    rdfs:comment "Classification of time series" ;
    :supported_by_oma_ml "True" .
:time_series_forecasting a :ML_task ;
    skos:prefLabel "time series forecasting" ;
    :belongs_to :supervised_learning ;
    :has_dataset_type :time_series ;
    rdfs:comment "The prediction of events through a sequenc of time" ;
    :supported_by_oma_ml "True" .
:topic_modeling a :ML_task ;
    skos:prefLabel "topic modeling" ;
    :belongs_to :unsupervised_learning ;
    rdfs:comment "set of techniques in computational linguistics and related fields" ;
    rdfs:seeAlso <https://www.wikidata.org/entity/Q96468792> .
:translation a :ML_task ;
    skos:prefLabel "translation" ;
    :belongs_to :supervised_learning ;
    :has_dataset_type :text ;
    rdfs:comment "communication of the meaning of a source-language text by means of an equivalent target-language text" ;
    rdfs:seeAlso <https://www.wikidata.org/entity/Q7553> .
:vertex_classification a :ML_task ;
    skos:prefLabel "vertex classification" ;
    skos:broader :classification ;
    :belongs_to :supervised_learning ;
    :has_dataset_type :graph ;
    rdfs:comment "Mapping a system of vertices, for which it is then classified and counts the types for vertices" .
:video_classification a :ML_task ;
    skos:prefLabel "video classification" ;
    skos:broader :classification ;
    :belongs_to :supervised_learning ;
    :has_dataset_type :video ;
    rdfs:comment "Videos will either fall under analog or digital categories, they are further subdivided by standard definition, high definition, how color and luminace are kept seperate or combine" .
:video_object_tracking a :ML_task ;
    skos:prefLabel "video object tracking" ;
    :belongs_to :supervised_learning ;
    :has_dataset_type :video ;
    rdfs:comment "Process of tacking a moving object over a period of time" .
:video_regression a :ML_task ;
    skos:prefLabel "video regression" ;
    skos:broader :regression ;
    :belongs_to :supervised_learning ;
    :has_dataset_type :video .
:association_rule_learning a :ML_task ;
    skos:prefLabel "association rule learning" ;
    :belongs_to :supervised_learning ;
    :has_dataset_type :tabular ;
    rdfs:comment "Association rule learning is a rule-based machine learning method for discovering interesting relations between variables in large databases. It is intended to identify strong rules discovered in databases using some measures of interestingness." ;
    rdfs:seeAlso <https://www.wikidata.org/wiki/Q386780> .


# ML_approach

:adaboost a :ML_approach ;
    skos:prefLabel "adaboost" ;
    :used_for :classification ;
    rdfs:seeAlso <https://www.wikidata.org/entity/Q2823869> .
:agglomerative_clustering a :ML_approach ;
    skos:prefLabel "agglomerative clustering" ;
    skos:broader :hierarchical_clustering ;
    :used_for :clustering ;
    rdfs:comment "A bottom up clustering method where clusters have subclusters, where these subclusters can also have subclusters" .
:arsenal_ensemble a :ML_approach ;
    skos:prefLabel "Arsenal ensemble" ;
    skos:altLabel "Arsenal" ;
    skos:broader :ensemble_classifier ;
    :used_for :time_series_classification ;
    rdfs:comment "Arsenal ensemble." .
:artificial_neural_network a :ML_approach ;
    skos:prefLabel "artificial neural network" ;
    skos:altLabel "ANN" , "neural network" ;
    :used_for :classification , :regression , :anomaly_detection , :time_series_classification ;
    :possible_if :numerical_features ;
    :performance :long_training_time , :accurate ;
    rdfs:comment "computational model used in machine learning, based on connected, hierarchical functions" ;
    rdfs:seeAlso <https://www.wikidata.org/entity/Q192776> .
:autoencoder a :ML_approach ;
    skos:prefLabel "autoencoder" ;
    skos:altLabel "AE" ;
    skos:broader :artificial_neural_network ;
    :used_for :anomaly_detection ;
    rdfs:comment "neural network that learns efficient data encoding in an unsupervised manner" ;
    rdfs:seeAlso <https://www.wikidata.org/entity/Q786435> .
:autoregressive_integrated_moving_average a :ML_approach ;
    skos:prefLabel "autoregressive integrated moving average" ;
    skos:altLabel "ARIMA" ;
    :used_for :time_series_analysis ;
    rdfs:comment "statistical model used in time series analysis" ;
    rdfs:seeAlso <https://www.wikidata.org/entity/Q2566298> .
:bag_of_sfa_symbols a :ML_approach ;
    skos:prefLabel "Bag-of-SFA-Symbols" ;
    skos:altLabel "BOSS" ;
    skos:broader :ensemble_classifier ;
    :used_for :time_series_classification ;
    rdfs:comment "Ensemble of bag of Symbolic Fourier Approximation Symbols" .
:bayesian_linear_regression a :ML_approach ;
    skos:prefLabel "Bayesian linear regression" ;
    skos:broader :linear_regression ;
    :used_for :regression ;
    :possible_if :small_dataset ;
    rdfs:comment "approach to linear regression in which the statistical analysis is undertaken within the context of Bayesian inference" ;
    rdfs:seeAlso <https://www.wikidata.org/entity/Q4874474> .
:bayesian_neural_network a :ML_approach ;
    skos:prefLabel "Bayesian neural network" ;
    skos:broader :artificial_neural_network ;
    :possible_if :numerical_features ;
    rdfs:comment "probability model which is factored by applying a single conditional probability distribution for each variable for the given model" .
:bernoulli_naive_bayes a :ML_approach ;
    skos:prefLabel "Bernoulli naive bayes" ;
    :used_for :classification ;
    rdfs:comment "Naive Bayes classifier for multivariate Bernoulli models." .
:boltzman_machine a :ML_approach ;
    skos:prefLabel "Boltzman machine" ;
    skos:broader :artificial_neural_network ;
    rdfs:comment "A type of stochastic recurrent neural network" .
:boosted_decision_tree a :ML_approach ;
    skos:prefLabel "boosted decision tree" ;
    skos:broader :decision_tree ;
    :performance :large_memory_footprint ;
    rdfs:comment "A ensemble learning method where the current tree's errors will  be corrected by the next tree and the next tree's errors will be corrected by the tree after, and so on" .
:c_means a :ML_approach ;
    skos:prefLabel "c-means" ;
    :used_for :clustering , :anomaly_detection ;
    rdfs:comment "Soft clustering where each data point is assigned a probability score to belong to that cluster" .
:canonical_correlation_analysis a :ML_approach ;
    skos:prefLabel "canonical correlation analysis" ;
    skos:altLabel "CCA" ;
    :used_for :feature_reduction ;
    :possible_if :numerical_features ;
    rdfs:comment "way of inferring information from cross-covariance matrices" ;
    rdfs:seeAlso <https://www.wikidata.org/entity/Q115542> .
:canonical_interval_forest a :ML_approach ;
    skos:prefLabel "Canonical Interval Forest" ;
    skos:altLabel "CIF" ;
    :used_for :time_series_classification ;
    rdfs:comment "Canonical Interval Forest Classifier" .
:canonical_time_series_characteristics a :ML_approach ;
    skos:prefLabel "Canonical Time-series Characteristics" ;
    skos:altLabel "catch22" ;
    :used_for :time_series_classification ;
    rdfs:comment "Canonical Time-series Characteristics (catch22) classifier." .
:catboost a :ML_approach ;
    skos:prefLabel "catboost" ;
    skos:broader :gradient_boosting_tree ;
    :used_for :classification , :regression ;
    :performance :accurate , :explainable ;
    rdfs:comment "yandex open source gradient boosting framework on decision trees" ;
    rdfs:seeAlso <https://www.wikidata.org/entity/Q104853624> .
:collaborative_filtering a :ML_approach ;
    skos:prefLabel "collaborative filtering" ;
    :used_for :recommendation ;
    rdfs:comment "uses algorithms to filter data from user reviews to make personalized recommendations for users with similar preferences" ;
    rdfs:seeAlso <https://www.wikidata.org/entity/Q94702> .
:conceptual_clustering a :ML_approach ;
    skos:prefLabel "conceptual clustering" ;
    :used_for :clustering ;
    rdfs:comment "machine learning paradigm" ;
    rdfs:seeAlso <https://www.wikidata.org/entity/Q5158434> .
:conditional_markov_model a :ML_approach ;
    skos:prefLabel "conditional markov model" ;
    skos:broader :markov_model ;
    rdfs:comment "A model that has two phases, structural phase and statistical phase" .
:conditional_random_field a :ML_approach ;
    skos:prefLabel "conditional random field" ;
    skos:altLabel "CRF" ;
    :used_for :time_series_analysis ;
    rdfs:comment "class of statistical modeling method applied in pattern recognition and machine learning and used for structured prediction" ;
    rdfs:seeAlso <https://www.wikidata.org/entity/Q1124538> .
:contractable_boss a :ML_approach ;
    skos:prefLabel "Contractable BOSS" ;
    skos:altLabel "cBOSS" ;
    skos:broader :ensemble_classifier ;
    :used_for :time_series_classification ;
    rdfs:comment "Contractable Bag of Symbolic Fourier Approximation Symbols" .
:convolutional_neural_network a :ML_approach ;
    skos:prefLabel "convolutional neural network" ;
    skos:altLabel "CNN" ;
    skos:broader :artificial_neural_network ;
    :used_for :image_classification , :time_series_classification ;
    rdfs:comment "A class of deep neural networks, most commonly applied to analyzing visual imagery." ;
    rdfs:seeAlso <https://www.wikidata.org/entity/Q17084460> .
:decision_tree a :ML_approach ;
    skos:prefLabel "decision tree" ;
    :used_for :classification , :regression ;
    :performance :fast_training , :explainable ;
    rdfs:comment "decision support tool that uses a tree-like model of decisions and their possible consequences, including chance event outcomes, resource costs, and utility" ;
    rdfs:seeAlso <https://www.wikidata.org/entity/Q831366> .
:deep_convolutional_lstm a :ML_approach ;
    skos:prefLabel "Deep Convolutional LSTM" ;
    skos:altLabel "DeepConvLSTM" ;
    skos:broader :artificial_neural_network ;
    :used_for :time_series_classification .
:density_based_clustering a :ML_approach ;
    skos:prefLabel "density-based clustering" ;
    :used_for :clustering ;
    rdfs:comment "Algorithm that finds non linear shapes structure based on their density" ;
    rdfs:seeAlso <https://www.wikidata.org/entity/Q56388089> .
:density_based_spatial_clustering_of_applications_with_noise a :ML_approach ;
    skos:prefLabel "density-based spatial clustering of applications with noise" ;
    skos:altLabel "DBSCAN" ;
    skos:broader :density_based_clustering ;
    :used_for :clustering ;
    rdfs:comment "data clustering algorithm" ;
    rdfs:seeAlso <https://www.wikidata.org/entity/Q1114630> .
:diverse_representation_canonical_interval_forest a :ML_approach ;
    skos:prefLabel "Diverse Representation Canonical Interval Forest" ;
    skos:altLabel "DrCIF" ;
    :used_for :time_series_classification ;
    rdfs:comment "Diverse Representation Canonical Interval Forest Classifier (DrCIF)." .
:elastic_ensemble a :ML_approach ;
    skos:prefLabel "Elastic Ensemble" ;
    skos:altLabel "EE" ;
    skos:broader :ensemble_classifier ;
    :used_for :time_series_classification ;
    :performance :long_training_time ;
    rdfs:comment "EE is an ensemble of elastic nearest neighbor classifiers" .
:ensemble skos:prefLabel "ensemble" ;
    :used_for :tabular_classification , :tabular_regression .
:expectation_maximization_clustering a :ML_approach ;
    skos:prefLabel "expectation maximization clustering" ;
    :used_for :clustering ;
    rdfs:comment "iterative method for finding maximum likelihood estimates in statistical models" ;
    rdfs:seeAlso <https://www.wikidata.org/entity/Q1275153> .
:exponential_smoothing a :ML_approach ;
    skos:prefLabel "exponential smoothing" ;
    :used_for :time_series_regresion ;
    rdfs:comment "is a rule of thumb technique for smoothing time series data using the exponential window function." .
:extra_tree a :ML_approach ;
    skos:prefLabel "extra tree" ;
    skos:broader :decision_tree ;
    :used_for :classification ;
    rdfs:comment "ensemble learning technique which aggregates the results of multiple de-correlated decision trees collected in a “forest” to output it’s classification result" .
:feed_forward_neural_network a :ML_approach ;
    skos:prefLabel "feed-forward neural network" ;
    skos:altLabel "FFN" ;
    skos:broader :artificial_neural_network ;
    rdfs:comment "artificial neural network wherein connections between the nodes do not form a cycle" ;
    rdfs:seeAlso <https://www.wikidata.org/entity/Q5441227> .
:fresh_prince a :ML_approach ;
    skos:prefLabel "Fresh PRINCE" ;
    :used_for :time_series_classification ;
    rdfs:comment "Fresh Pipeline with RotatIoN forest Classifier." .
:gated_recurrent_unit a :ML_approach ;
    skos:prefLabel "gated recurrent unit" ;
    skos:altLabel "GRU" ;
    skos:broader :artificial_neural_network ;
    rdfs:comment "mechanisms in recurrent neural networks" ;
    rdfs:seeAlso <https://www.wikidata.org/entity/Q25325415> .
:gaussian_mixture_model a :ML_approach ;
    skos:prefLabel "Gaussian mixture model" ;
    skos:altLabel "GMM" ;
    :used_for :clustering ;
    rdfs:comment "A model that is a mixture of several Gaussian distributions" .
:gaussian_naives_bayes a :ML_approach ;
    skos:prefLabel "Gaussian naives bayes" ;
    skos:altLabel "GNB" ;
    skos:broader :naive_bayes ;
    rdfs:comment "probabilistic machine learning algorithm used for many classification functions that is based on the Bayes theorem" .
:gaussian_process a :ML_approach ;
    skos:prefLabel "Gaussian process" ;
    skos:altLabel "GP" ;
    :used_for :classification , :regression ;
    :not_recommended_if :many_features ;
    rdfs:comment "particular kind of statistical model where observations occur in a continuous domain, e.g. time or space. In a Gaussian process, every point in some continuous input space is associated with a normally distributed random variable" ;
    rdfs:seeAlso <https://www.wikidata.org/entity/Q1496376> .
:generalized_linear_model a :ML_approach ;
    skos:prefLabel "generalized linear model" ;
    skos:altLabel "GLM" ;
    :used_for :classification ;
    rdfs:comment "class of statistical models" ;
    rdfs:seeAlso <https://www.wikidata.org/entity/Q1501882> .
:generative_adversarial_network a :ML_approach ;
    skos:prefLabel "generative adversarial network" ;
    skos:altLabel "GAN" ;
    skos:broader :artificial_neural_network ;
    rdfs:comment "deep learning method" ;
    rdfs:seeAlso <https://www.wikidata.org/entity/Q25104379> .
:gradient_boosting_tree a :ML_approach ;
    skos:prefLabel "gradient boosting tree" ;
    skos:broader :boosted_decision_tree ;
    :used_for :classification , :regression , :ranking ;
    :performance :accurate , :explainable ;
    rdfs:comment "Ensemble of weak predictors, which are often decision trees" .
:hidden_markov_model a :ML_approach ;
    skos:prefLabel "hidden markov model" ;
    skos:altLabel "HMM" ;
    skos:broader :markov_model ;
    :used_for :time_series_analysis , :anomaly_detection ;
    rdfs:comment "statistical Markov model" ;
    rdfs:seeAlso <https://www.wikidata.org/entity/Q176769> .
:hierachical_dbscan a :ML_approach ;
    skos:prefLabel "hierachical dbscan" ;
    skos:altLabel "HDBSCAN" ;
    skos:broader :density_based_spatial_clustering_of_applications_with_noise ;
    :used_for :clustering ;
    rdfs:comment "grouping of objects such that the objects in a cluster are similar to one another and are unrelated to the objects in other groups" .
:hierarchical_clustering a :ML_approach ;
    skos:prefLabel "hierarchical clustering" ;
    :used_for :clustering ;
    rdfs:comment "method of cluster analysis which seeks to build a hierarchy of clusters" ;
    rdfs:seeAlso <https://www.wikidata.org/entity/Q1277447> .
:hierarchical_vote_collective_of_transformation_based_ensembles_v1 a :ML_approach ;
    skos:prefLabel "Hierarchical Vote Collective of Transformation-based Ensembles V1" ;
    skos:altLabel "HIVE-COTE V1" ;
    skos:broader :ensemble_classifier ;
    :used_for :time_series_classification ;
    :performance :long_training_time , :accurate ;
    rdfs:comment "Hierarchical Vote Collective of Transformation-based Ensembles (HIVE-COTE) V1." .
:hierarchical_vote_collective_of_transformation_based_ensembles_v2 a :ML_approach ;
    skos:prefLabel "Hierarchical Vote Collective of Transformation-based Ensembles V2" ;
    skos:altLabel "HIVE-COTE V2" ;
    skos:broader :ensemble_classifier ;
    :used_for :time_series_classification ;
    :performance :long_training_time , :accurate ;
    rdfs:comment "Hierarchical Vote Collective of Transformation-based Ensembles (HIVE-COTE) V2" .
:inception_fully_convolutional_network a :ML_approach ;
    skos:prefLabel "Inception Fully Convolutional Network" ;
    skos:altLabel "InceptionFCN" ;
    skos:broader :artificial_neural_network ;
    :used_for :time_series_classification .
:inception_time a :ML_approach ;
    skos:prefLabel "Inception Time" ;
    skos:altLabel "InceptionTime" ;
    skos:broader :artificial_neural_network ;
    :used_for :time_series_classification ;
    :performance :scalable ;
    rdfs:comment "InceptionTime is an ensemble of deep Convolutional Neural Network (CNN) models, inspired by the Inception-v4 architecture." .
:independent_component_analysis a :ML_approach ;
    skos:prefLabel "independent component analysis" ;
    skos:altLabel "ICA" ;
    :used_for :feature_reduction ;
    :possible_if :numerical_features ;
    rdfs:comment "in signal processing, a computational method" ;
    rdfs:seeAlso <https://www.wikidata.org/entity/Q1259145> .
:individual_boss a :ML_approach ;
    skos:prefLabel "Individual BOSS" ;
    skos:altLabel "IndividualBOSS" ;
    skos:broader :ensemble_classifier ;
    :used_for :time_series_classification ;
    rdfs:comment "Single bag of Symbolic Fourier Approximation Symbols" .
:individual_temporal_dictionary_ensemble a :ML_approach ;
    skos:prefLabel "Individual Temporal Dictionary Ensemble" ;
    skos:altLabel "IndividualTDE" ;
    skos:broader :ensemble_classifier ;
    :used_for :time_series_classification ;
    rdfs:comment "Single TDE classifier, an extension of the Bag of SFA Symbols (BOSS) model." .
:k_means a :ML_approach ;
    skos:prefLabel "k-means" ;
    :used_for :clustering ;
    :possible_if :numerical_features ;
    rdfs:comment "vector quantization method that partitions n observations into k clusters in which each observation belongs to the cluster with the nearest mean, serving as a prototype of the cluster" ;
    rdfs:seeAlso <https://www.wikidata.org/entity/Q310401> .
:k_modes a :ML_approach ;
    skos:prefLabel "k-modes" ;
    skos:broader :k_means ;
    :used_for :clustering ;
    :possible_if :categorical_features , :text_features ;
    rdfs:comment "Using dissimilarities, quantification of the total mismatches between two objects" .
:k_nearest_neighbor a :ML_approach ;
    skos:prefLabel "k-nearest neighbor" ;
    skos:altLabel "kNN" ;
    :used_for :classification , :regression ;
    :performance :fast_training ;
    rdfs:comment "classification algorithm" ;
    rdfs:seeAlso <https://www.wikidata.org/entity/Q1071612> .
:kernel_svm a :ML_approach ;
    skos:prefLabel "kernel svm" ;
    skos:broader :support_vector_machine ;
    :performance :accurate ;
    rdfs:comment "set of mathematical functions that are defined as the kernel" .
:kohonen_network a :ML_approach ;
    skos:prefLabel "Kohonen network" ;
    skos:broader :artificial_neural_network ;
    rdfs:comment "type of artificial neural network" ;
    rdfs:seeAlso <https://www.wikidata.org/entity/Q1136838> .
:lasso_regression a :ML_approach ;
    skos:prefLabel "Lasso regression" ;
    skos:broader :linear_regression ;
    :used_for :classification , :regression ;
    rdfs:comment "regularization algorithm that assists in the elimination of irrelevant parameters, thus helping in the concentration of selection and regularizes the models" .
:latent_dirichlet_allocation a :ML_approach ;
    skos:prefLabel "latent dirichlet allocation" ;
    skos:altLabel "LDA" ;
    :used_for :feature_reduction , :topic_modeling ;
    rdfs:comment "generative statistical model that allows sets of observations to be explained by unobserved groups that explain why some parts of the data are similar" ;
    rdfs:seeAlso <https://www.wikidata.org/entity/Q269236> .
:light_gradient_boosting_machine a :ML_approach ;
    skos:prefLabel "light gradient boosting machine" ;
    skos:altLabel "LGBM" ;
    skos:broader :gradient_boosting_tree ;
    :used_for :classification , :regression ;
    :performance :accurate , :explainable ;
    rdfs:comment "machine learning software" ;
    rdfs:seeAlso <https://www.wikidata.org/entity/Q57267665> .
:linear_regression a :ML_approach ;
    skos:prefLabel "linear regression" ;
    :used_for :regression ;
    :performance :fast_training ;
    rdfs:comment "statistical approach for modeling the relationship between a scalar dependent variable and one or more explanatory variables" ;
    rdfs:seeAlso <https://www.wikidata.org/entity/Q10861030> .
:linear_svc a :ML_approach ;
    skos:prefLabel "linear SVC" ;
    skos:broader :support_vector_machine ;
    :used_for :classification ;
    rdfs:comment "Similar to SVC with parameter kernel=’linear’, but implemented in terms of liblinear rather than libsvm, so it has more flexibility in the choice of penalties and loss functions and should scale better to large numbers of samples." .
:linear_svm a :ML_approach ;
    skos:prefLabel "linear SVM" ;
    skos:broader :support_vector_machine ;
    :not_recommended_if :large_dataset ;
    :performance :fast_training ;
    rdfs:comment "A linearly scalable routine that it creates an SVM model in a CPU time which scales linearly with the size of the training data set" .
:local_linear_embedding a :ML_approach ;
    skos:prefLabel "local linear embedding" ;
    skos:altLabel "LLE" ;
    :used_for :feature_reduction ;
    rdfs:comment "unsupervised method for non-linear dimensionality reduction that can discover non-linear structures in the data set, and also preserve the distances within local neighborhoods" .
:logistic_regression a :ML_approach ;
    skos:prefLabel "logistic regression" ;
    :used_for :classification , :regression , :ranking ;
    :performance :fast_training ;
    rdfs:comment "statistical model" ;
    rdfs:seeAlso <https://www.wikidata.org/entity/Q1132755> .
:long_short_term_memory a :ML_approach ;
    skos:prefLabel "long short term memory" ;
    skos:altLabel "LSTM" ;
    skos:broader :artificial_neural_network ;
    :used_for :time_series_analysis ;
    rdfs:comment "recurrent neural network architecture" ;
    rdfs:seeAlso <https://www.wikidata.org/entity/Q6673524> .
:markov_model a :ML_approach ;
    skos:prefLabel "Markov model" ;
    skos:altLabel "MM" ;
    rdfs:comment "probability tool" ;
    rdfs:seeAlso <https://www.wikidata.org/entity/Q6771326> .
:martrix_profile a :ML_approach ;
    skos:prefLabel "Martrix Profile" ;
    skos:altLabel "MP" ;
    :used_for :time_series_classification ;
    rdfs:comment "Martrix Profile (MP) classifier" .
:maximum_entropy_markov_model a :ML_approach ;
    skos:prefLabel "maximum entropy Markov model" ;
    skos:altLabel "MEMM" ;
    skos:broader :markov_model ;
    rdfs:seeAlso <https://www.wikidata.org/entity/Q6795829> .
:multi_scale_convolutional_neural_networks a :ML_approach ;
    skos:prefLabel "Multi-Scale Convolutional Neural Networks" ;
    skos:altLabel "MCNN" ;
    skos:broader :artificial_neural_network ;
    :used_for :time_series_classification ;
    :performance :scalable ;
    rdfs:comment "A novel end-to-end neural network model, MCNN, incorporates feature extraction and classification in a single framework." .
:multilayer_perceptron a :ML_approach ;
    skos:prefLabel "multilayer perceptron" ;
    skos:altLabel "MLP" ;
    skos:broader :feed_forward_neural_network ;
    rdfs:comment "type of feedforward neural network" ;
    rdfs:seeAlso <https://www.wikidata.org/entity/Q2991667> .
:multinominal_naive_bayes a :ML_approach ;
    skos:prefLabel "multinominal naive bayes" ;
    :used_for :classification ;
    :possible_if :large_dataset , :text_features ;
    :performance :fast_training ;
    rdfs:comment "classification algorithm" ;
    rdfs:seeAlso <https://www.wikidata.org/entity/Q812530> .
:multivariate_symbolic_extension a :ML_approach ;
    skos:prefLabel "MUltivariate Symbolic Extension" ;
    skos:altLabel "MUSE" ;
    :used_for :time_series_classification ;
    rdfs:comment "MUltivariate Symbolic Extension" .
:ordering_points_to_identify_the_clustering_structure a :ML_approach ;
    skos:prefLabel "ordering points to identify the clustering structure" ;
    skos:altLabel "OPTICS" ;
    :used_for :clustering .
:passive_aggressive_classifier a :ML_approach ;
    skos:prefLabel "passive aggressive classifier" ;
    :used_for :classification ;
    rdfs:comment "The passive-aggressive algorithms are a family of algorithms for large-scale learning. They are similar to the Perceptron in that they do not require a learning rate. However, contrary to the Perceptron, they include a regularization parameter C." .
:perceptron a :ML_approach ;
    skos:prefLabel "perceptron" ;
    skos:broader :artificial_neural_network ;
    rdfs:comment "algorithm for supervised learning of binary classifiers" ;
    rdfs:seeAlso <https://www.wikidata.org/entity/Q690207> .
:poisson_regression a :ML_approach ;
    skos:prefLabel "poisson regression" ;
    skos:broader :linear_regression ;
    :used_for :regression ;
    rdfs:comment "statistical model for count data" ;
    rdfs:seeAlso <https://www.wikidata.org/entity/Q954529> .
:polynomial_regression a :ML_approach ;
    skos:prefLabel "polynomial regression" ;
    :used_for :regression ;
    rdfs:seeAlso <https://www.wikidata.org/entity/Q45343> .
:prophet a :ML_approach ;
    skos:prefLabel "prophet" ;
    :used_for :time_series_analysis .
:proximity_forest a :ML_approach ;
    skos:prefLabel "Proximity Forest" ;
    skos:altLabel "PF" ;
    skos:broader :ensemble_classifier ;
    :used_for :time_series_classification ;
    rdfs:comment "Proximity Forest classifier models a decision tree forest which uses distance measures to partition data" .
:proximity_stump a :ML_approach ;
    skos:prefLabel "Proximity Stump" ;
    skos:broader :decision_stump ;
    :used_for :time_series_classification ;
    rdfs:comment "Proximity Stump classifier models a decision stump which uses a distance measure to partition data." .
:proximity_tree a :ML_approach ;
    skos:prefLabel "Proximity Tree" ;
    skos:broader :decision_tree ;
    :used_for :time_series_classification ;
    rdfs:comment "A decision tree which uses distance measures to partition data" .
:random_forest a :ML_approach ;
    skos:prefLabel "random forest" ;
    skos:broader :decision_tree ;
    :used_for :classification , :regression ;
    :performance :fast_training , :accurate ;
    rdfs:comment "statistical algorithm that is used to cluster points of data in functional groups" ;
    rdfs:seeAlso <https://www.wikidata.org/entity/Q245748> .
:random_interval a :ML_approach ;
    skos:prefLabel "Random Interval" ;
    :used_for :time_series_classification ;
    rdfs:comment "Random Interval Classifier." .
:random_interval_spectral_ensemble a :ML_approach ;
    skos:prefLabel "Random Interval Spectral Ensemble" ;
    skos:altLabel "RISE" ;
    :used_for :time_series_classification ;
    rdfs:comment "Random Interval Spectral Ensemble" .
:random_kitchen_sinks_sampler a :ML_approach ;
    skos:prefLabel "random kitchen sinks sampler" ;
    rdfs:comment "Approximate a RBF kernel feature map using random Fourier features." .
:recurrent_nn a :ML_approach ;
    skos:prefLabel "recurrent nn" ;
    skos:altLabel "RNN" ;
    skos:broader :artificial_neural_network ;
    :used_for :time_series_analysis ;
    rdfs:comment "class of artificial neural network where connections between units form a directed graph along a temporal sequence" ;
    rdfs:seeAlso <https://www.wikidata.org/entity/Q1457734> .
:residual_neural_network a :ML_approach ;
    skos:prefLabel "Residual Neural Network" ;
    skos:altLabel "ResNet" ;
    skos:broader :artificial_neural_network ;
    :used_for :image_classification , :time_series_classification ;
    rdfs:comment "Deep Convolutional and LSTM Recurrent Neural Networks for Multimodal Wearable Activity Recognition" .
:ridge_regression a :ML_approach ;
    skos:prefLabel "ridge regression" ;
    skos:broader :linear_regression ;
    :used_for :classification , :regression ;
    rdfs:comment "regularization technique for ill-posed problems" ;
    rdfs:seeAlso <https://www.wikidata.org/entity/Q2778212> .
:seasonal_autoregressive_integrated_moving_average_exogenous a :ML_approach ;
    skos:prefLabel "seasonal autoregressive integrated moving average exogenous" ;
    skos:altLabel "SARIMAX" ;
    :used_for :time_series_analysis .
:self_organizing_map a :ML_approach ;
    skos:prefLabel "self-organizing map" ;
    skos:altLabel "SOM" ;
    :used_for :clustering , :anomaly_detection , :feature_reduction ;
    rdfs:comment "type of artificial neural network" ;
    rdfs:seeAlso <https://www.wikidata.org/entity/Q1136838> .
:self_organizing_tree_algorithm a :ML_approach ;
    skos:prefLabel "self-organizing tree algorithm" ;
    skos:altLabel "SOTA" ;
    :used_for :clustering , :anomaly_detection .
:shapelet_transform_classifier a :ML_approach ;
    skos:prefLabel "Shapelet Transform Classifier" ;
    :used_for :time_series_classification ;
    :performance :long_training_time ;
    rdfs:comment "Shapelet Transform Classifier." .
:signature_classifier a :ML_approach ;
    skos:prefLabel "Signature Classifier" ;
    :used_for :time_series_classification ;
    rdfs:comment "Classification module using signature-based features." .
:singular_value_decomposition a :ML_approach ;
    skos:prefLabel "singular value decomposition" ;
    skos:altLabel "SVD" ;
    :used_for :feature_reduction , :recommendation ;
    :possible_if :numerical_features ;
    rdfs:comment "matrix decomposition" ;
    rdfs:seeAlso <https://www.wikidata.org/entity/Q420904> .
:spectral_clustering a :ML_approach ;
    skos:prefLabel "spectral clustering" ;
    :used_for :clustering ;
    rdfs:seeAlso <https://www.wikidata.org/entity/Q2976589> .
:stochastic_gradient_descent a :ML_approach ;
    skos:prefLabel "stochastic gradient descent" ;
    skos:altLabel "SGD" ;
    :used_for :classification , :regression ;
    rdfs:comment "optimization algorithm" ;
    rdfs:seeAlso <https://www.wikidata.org/entity/Q7617819> .
:summary_statistic a :ML_approach ;
    skos:prefLabel "Summary statistic" ;
    :used_for :time_series_classification ;
    rdfs:comment "Summary statistic classifier." .
:supervised_time_series_forest a :ML_approach ;
    skos:prefLabel "Supervised Time Series Forest" ;
    skos:altLabel "STSF" ;
    :used_for :time_series_classification ;
    :performance :fast_training , :explainable , :scalable ;
    rdfs:comment "Supervised Time Series Forest (STSF)" .
:support_vector_machine a :ML_approach ;
    skos:prefLabel "support vector machine" ;
    skos:altLabel "SVM" ;
    :used_for :classification , :regression , :anomaly_detection ;
    :not_recommended_if :many_features ;
    rdfs:comment "set of methods for supervised statistical learning" ;
    rdfs:seeAlso <https://www.wikidata.org/entity/Q282453> .
:support_vector_regression a :ML_approach ;
    skos:prefLabel "support vector regression" ;
    skos:broader :linear_regression ;
    :used_for :regression ;
    rdfs:seeAlso <https://www.wikidata.org/entity/Q57534282> .
:temporal_dictionary_ensemble a :ML_approach ;
    skos:prefLabel "Temporal Dictionary Ensemble" ;
    skos:altLabel "TDE" ;
    skos:broader :ensemble_classifier ;
    :used_for :time_series_classification ;
    rdfs:comment "Temporal Dictionary Ensemble" .
:time_series_combination_of_heterogeneous_and_integrated_embedding_forest a :ML_approach ;
    skos:prefLabel "Time Series Combination of Heterogeneous and Integrated Embedding Forest" ;
    skos:altLabel "TS-CHIEF" ;
    :used_for :time_series_classification ;
    :performance :long_training_time ;
    rdfs:comment "Time Series Combination of Heterogeneous and Integrated Embedding Forest" .
:time_series_forest a :ML_approach ;
    skos:prefLabel "Time series forest" ;
    skos:altLabel "TSF" ;
    :used_for :time_series_classification ;
    :performance :fast_training , :explainable , :scalable ;
    rdfs:comment "Time series forest (TSF) classifier." .
:transformer a :ML_approach ;
    skos:prefLabel "transformer" ;
    skos:broader :artificial_neural_network .
:temporal_fusion_transformer a :ML_approach ;
    skos:prefLabel "temporal fusion transformer" ;
    skos:broader :transformer ;
    :used_for :time_series_forecasting .
:variational_bayesian_gaussian_mixture_model a :ML_approach ;
    skos:prefLabel "variational Bayesian Gaussian mixture model" ;
    skos:altLabel "VB-GMM" ;
    skos:broader :gaussian_mixture_model ;
    :used_for :clustering ;
    rdfs:comment "Screening of miRNA target genes in coronary artery disease by variational Bayesian Gaussian mixture model" ;
    rdfs:seeAlso <https://www.wikidata.org/entity/Q64233346> .
:word_extraction_for_time_series_classification a :ML_approach ;
    skos:prefLabel "Word Extraction for Time Series Classification" ;
    skos:altLabel "WEASEL" ;
    :used_for :time_series_classification ;
    rdfs:comment "Word Extraction for Time Series Classification" .
:word2vector a :ML_approach ;
    skos:prefLabel "word2vector" ;
    :used_for :text_analytics .
:xgboost a :ML_approach ;
    skos:prefLabel "xgboost" ;
    skos:altLabel "XGB" ;
    skos:broader :gradient_boosting_tree ;
    :used_for :classification , :regression ;
    :performance :accurate , :explainable ;
    rdfs:comment "scalable machine learning system for tree boosting" ;
    rdfs:seeAlso <https://www.wikidata.org/entity/Q23793561> .
:ridge_classifier a :ML_approach ;
    skos:prefLabel "Ridge Classifier" ;
    :used_for :classification .
:linear_discriminant_analysis a :ML_approach ;
    skos:prefLabel "Linear Discriminant Analysis" ;
    :used_for :classification .
:quadratic_discriminant_analysis a :ML_approach ;
    skos:prefLabel "Quadratic Discriminant Analysis" ;
    :used_for :classification .


# Preprocessing_approach

:kernel_approximation a :Preprocessing_approach ;
    skos:prefLabel "kernel approximation" ;
    :used_for :classification , :regression .
:principal_component_analysis a :Preprocessing_approach ;
    skos:prefLabel "principal component analysis" ;
    skos:altLabel "PCA" ;
    :used_for :feature_reduction , :anomaly_detection ;
    :possible_if :numerical_features ;
    :performance :fast_training ;
    rdfs:comment "conversion of a set of observations of possibly correlated variables into a set of values of linearly uncorrelated variables called principal components" ;
    rdfs:seeAlso <https://www.wikidata.org/entity/Q2873> .
:kernel_principal_component_analysis a :Preprocessing_approach ;
    skos:prefLabel "kernel principal component analysis" ;
    skos:altLabel "kernel PCA" ;
    skos:broader :principal_component_analysis ;
    :used_for :feature_reduction , :anomaly_detection ;
    :possible_if :numerical_features ;
    :performance :fast_training ;
    rdfs:comment "multivariate analysis technique with kernel method" ;
    rdfs:seeAlso <https://www.wikidata.org/entity/Q17093020> .
:nystroem_kernel_approximation a :Preprocessing_approach ;
    skos:prefLabel "Nystroem kernel approximation" ;
    skos:broader :kernel_approximation .
:radial_basis_function_kernel a :Preprocessing_approach ;
    skos:prefLabel "radial basis function kernel" ;
    skos:broader :kernel_approximation ;
    rdfs:seeAlso <https://www.wikidata.org/entity/Q7280263> .
:rocket a :Preprocessing_approach ;
    skos:prefLabel "ROCKET" .
:minirocket a :Preprocessing_approach ;
    skos:prefLabel "MiniROCKET" .


# Metric

:accuracy a :Metric ;
    skos:prefLabel "accuracy" ;
    :used_for :classification ;
    :recommended_if :balanced_dataset ;
    :not_recommended_if :unbalanced_dataset ;
    rdfs:comment "Closeness to true value or to each other" ;
    rdfs:seeAlso <https://www.wikidata.org/entity/Q272035> .
:area_under_roc_curve a :Metric ;
    skos:prefLabel "area under roc curve" ;
    skos:altLabel "AUC" ;
    :used_for :classification ;
    rdfs:comment "A Simple Generalisation of the Area Under the ROC Curve for Multiple Class Classification Problems" ;
    rdfs:seeAlso <https://www.wikidata.org/entity/Q55878266> .
:area_under_roc_curve_macro a :Metric ;
    skos:prefLabel "area under roc curve macro" ;
    skos:altLabel "AUC macro" ;
    :used_for :classification ;
    rdfs:comment "AUC score for multiclass classification using macro averaging." .
:area_under_roc_curve_micro a :Metric ;
    skos:prefLabel "area under roc curve micro" ;
    skos:altLabel "AUC micro" ;
    :used_for :classification ;
    rdfs:comment "AUC score for multiclass classification using micro averaging." .
:area_under_roc_curve_weighted a :Metric ;
    skos:prefLabel "area under roc curve weighted" ;
    skos:altLabel "AUC weighted" ;
    :used_for :classification ;
    rdfs:comment "AUC score for multiclass classification using weighted averaging." .
:average_precision a :Metric ;
    skos:prefLabel "average precision" ;
    skos:altLabel "AP" ;
    :used_for :classification .
:balanced_accuracy a :Metric ;
    skos:prefLabel "balanced accuracy" ;
    :used_for :classification .
:binary_accuracy a :Metric ;
    skos:prefLabel "binary accuracy" ;
    :used_for :classification ;
    rdfs:comment "Calculates how often predictions match binary labels." .
:binary_cross_entropy a :Metric ;
    skos:prefLabel "binary cross entropy" ;
    :used_for :classification .
:binary_intersection_over_union a :Metric ;
    skos:prefLabel "binary intersection over union" ;
    skos:altLabel "binary IoU" ;
    :used_for :image_segmentation ;
    rdfs:comment "computes the Intersection-Over-Union metric for class 0 and / or 1" .
:categorical_accuracy a :Metric ;
    skos:prefLabel "categorical accuracy" ;
    :used_for :classification ;
    rdfs:comment "Calculates how often predictions match one-hot labels." .
:categorical_cross_entropy a :Metric ;
    skos:prefLabel "categorical cross entropy" ;
    :used_for :classification .
:categorical_hinge a :Metric ;
    skos:prefLabel "categorical hinge" ;
    :used_for :classification .
:coefficient_of_determination a :Metric ;
    skos:prefLabel "coefficient of determination" ;
    skos:altLabel "R2" ;
    :used_for :regression ;
    rdfs:comment "indicator for how well data points fit a line or curve" ;
    rdfs:seeAlso <https://www.wikidata.org/entity/Q192830> .
:cohens_kappa a :Metric ;
    skos:prefLabel "cohens kappa" ;
    rdfs:comment "Statistic measuring inter-rater agreement for categorical items kappa" ;
    rdfs:seeAlso <https://www.wikidata.org/entity/Q1107106> .
:cosine_similarity a :Metric ;
    skos:prefLabel "cosine similarity" ;
    :used_for :regression .
:critical_success_index a :Metric ;
    skos:prefLabel "critical success index" ;
    skos:altLabel "CSI" , "Threat score" , "TS" .
:explained_variance a :Metric ;
    skos:prefLabel "explained variance" ;
    skos:altLabel "Max Error" ;
    :used_for :regression ;
    rdfs:comment "explained variacne score for regression" .
:f_measure a :Metric ;
    skos:prefLabel "F-measure" ;
    skos:altLabel "F" , "F1" , "F1-score" ;
    :used_for :classification ;
    :recommended_if :unbalanced_dataset ;
    rdfs:comment "measure of a test's accuracy" ;
    rdfs:seeAlso <https://www.wikidata.org/entity/Q6975395> .
:f_measure_macro a :Metric ;
    skos:prefLabel "F-measure macro" ;
    skos:altLabel "F1 macro" ;
    :used_for :classification .
:f_measure_micro a :Metric ;
    skos:prefLabel "F-measure micro" ;
    skos:altLabel "F1 micro" ;
    :used_for :classification .
:f_measure_samples a :Metric ;
    skos:prefLabel "F-measure samples" ;
    :used_for :classification .
:f_measure_weighted a :Metric ;
    skos:prefLabel "F-measure weighted" ;
    skos:altLabel "F1 weighted" ;
    :used_for :classification .
:false_discovery_rate a :Metric ;
    skos:prefLabel "false discovery rate" ;
    skos:altLabel "FDR" ;
    rdfs:comment "https://www.wikidata.org/entity/Q58618170" ;
    rdfs:seeAlso <https://www.wikidata.org/entity/Q58618170> .
:false_negative_rate a :Metric ;
    skos:prefLabel "false negative rate" ;
    skos:altLabel "FNR" , "miss rate" .
:false_negatives a :Metric ;
    skos:prefLabel "false negatives" ;
    :used_for :classification .
:false_omission_rate a :Metric ;
    skos:prefLabel "false omission rate" ;
    skos:altLabel "FOR" .
:false_positive_rate a :Metric ;
    skos:prefLabel "false positive rate" ;
    skos:altLabel "FPR" , "fall-out" ;
    rdfs:seeAlso <https://www.wikidata.org/entity/Q5432725> .
:false_positives a :Metric ;
    skos:prefLabel "false positives" ;
    :used_for :classification .
:fowlkes_mallows_index a :Metric ;
    skos:prefLabel "fowlkes mallows index" ;
    skos:altLabel "FM" ;
    rdfs:seeAlso <https://www.wikidata.org/entity/Q5476477> .
:gini a :Metric ;
    skos:prefLabel "gini" ;
    skos:altLabel "Gini" ;
    :used_for :classification ;
    rdfs:comment "The Gini Coefficient is an index to measure inequality." .
:hinge a :Metric ;
    skos:prefLabel "hinge" ;
    :used_for :classification .
:informedness a :Metric ;
    skos:prefLabel "informedness" ;
    skos:altLabel "bookmaker informedness" , "BM" .
:intersection_over_union a :Metric ;
    skos:prefLabel "intersection over union" ;
    skos:altLabel "IoU" ;
    :used_for :image_segmentation .
:kullback_leibler_divergence a :Metric ;
    skos:prefLabel "kullback-leibler divergence" ;
    skos:altLabel "KL divergence" .
:log_cosh_error a :Metric ;
    skos:prefLabel "log cosh error" ;
    :used_for :regression .
:log_loss a :Metric ;
    skos:prefLabel "log loss" ;
    skos:altLabel "Log loss" ;
    :used_for :classification ;
    rdfs:comment "average cross-entropy between the distribution of the true labels and the predictions" ;
    rdfs:seeAlso <https://www.wikidata.org/entity/Q22667762> .
:markedness a :Metric ;
    skos:prefLabel "markedness" ;
    skos:altLabel "MK" , "deltaP" ;
    rdfs:comment "state of standing out as unusual or difficult in comparison to a more common or regular form" ;
    rdfs:seeAlso <https://www.wikidata.org/entity/Q1897166> .
:matthews_correlation_coefficient a :Metric ;
    skos:prefLabel "matthews correlation coefficient" ;
    skos:altLabel "MCC" ;
    rdfs:comment "statistics and Probability" ;
    rdfs:seeAlso <https://www.wikidata.org/entity/Q6791500> .
:max_error a :Metric ;
    skos:prefLabel "max error" ;
    skos:altLabel "Max Error" ;
    :used_for :regression ;
    rdfs:comment "Maximum residual error for regression" .
:mean a :Metric ;
    skos:prefLabel "mean" .
:mean_absolute_error a :Metric ;
    skos:prefLabel "mean absolute error" ;
    skos:altLabel "MAE" ;
    :used_for :regression ;
    rdfs:comment "measure of difference between two continuous variables" ;
    rdfs:seeAlso <https://www.wikidata.org/entity/Q6803609> .
:mean_absolute_percentage_error a :Metric ;
    skos:prefLabel "mean absolute percentage error" ;
    skos:altLabel "MAPE" ;
    :used_for :regression , :time_series_forecasting ;
    rdfs:comment "measure of prediction accuracy of a forecast" ;
    rdfs:seeAlso <https://www.wikidata.org/entity/Q6803607> .
:symmetric_mean_absolute_percentage_error a :Metric ;
    skos:prefLabel "symmetric mean absolute percentage error" ;
    skos:altLabel "SMAPE" ;
    :used_for :time_series_forecasting .
:mean_absolute_scaled_error a :Metric ;
    skos:prefLabel "mean absolute scaled error" ;
    skos:altLabel "MASE" ;
    :used_for :time_series_forecasting ;
    rdfs:comment "measure of forecasting quality" ;
    rdfs:seeAlso <https://www.wikidata.org/wiki/Q6803610> .
:mean_intersection_over_union a :Metric ;
    skos:prefLabel "mean intersection-over-union" ;
    skos:altLabel "mean intersection-over-union" ;
    :used_for :image_segmentation .
:mean_metric_wrapper a :Metric ;
    skos:prefLabel "mean metric wrapper" .
:mean_relative_error a :Metric ;
    skos:prefLabel "mean relative error" ;
    :used_for :regression .
:mean_squared_error a :Metric ;
    skos:prefLabel "mean squared error" ;
    skos:altLabel "MSE" ;
    :used_for :regression ;
    rdfs:comment "Average of the squares of the errors between estimated and actual values" ;
    rdfs:seeAlso <https://www.wikidata.org/entity/Q1940696> .
:mean_squared_log_error a :Metric ;
    skos:prefLabel "mean squared log error" ;
    :used_for :regression .
:mean_tensor a :Metric ;
    skos:prefLabel "mean tensor" .
:median_absolute_error a :Metric ;
    skos:prefLabel "median absolute error" ;
    skos:altLabel "Median AE" ;
    :used_for :regression .
:metric a :Metric ;
    skos:prefLabel "metric" .
:negative_predictive_value a :Metric ;
    skos:prefLabel "negative predictive value" ;
    skos:altLabel "NPV" ;
    rdfs:comment "in biostatistics, the proportion of patients with negative test results who are correctly diagnosed" ;
    rdfs:seeAlso <https://www.wikidata.org/entity/Q2776546> .
:normalized_discounted_cumulative_gain a :Metric ;
    skos:prefLabel "normalized discounted cumulative gain" ;
    skos:altLabel "NDCG" ;
    :used_for :ranking .
:one_hot_intersection_over_union a :Metric ;
    skos:prefLabel "one hot intersection over union" ;
    :used_for :image_segmentation .
:one_hot_mean_intersection_over_union a :Metric ;
    skos:prefLabel "one hot mean intersection over union" ;
    skos:altLabel "one hot mean IoU" ;
    :used_for :image_segmentation .
:pac_score a :Metric ;
    skos:prefLabel "pac score" ;
    skos:altLabel "PAC-Bayesian AUC classification and scoring" ;
    :used_for :classification .
:pearson_correlation_coefficient a :Metric ;
    skos:prefLabel "pearson correlation coefficient" ;
    skos:altLabel "pearsonr" ;
    :used_for :regression ;
    rdfs:comment "type of coefficient" ;
    rdfs:seeAlso <https://www.wikidata.org/entity/Q1136628> .
:poisson a :Metric ;
    skos:prefLabel "poisson" .
:precision a :Metric ;
    skos:prefLabel "precision" ;
    skos:altLabel "positive predictive value" , "PPV" ;
    :used_for :classification ;
    rdfs:comment "reason for preferred rank based on level of detail, time precision (e.g. day instead of year)" ;
    rdfs:seeAlso <https://www.wikidata.org/entity/Q71536040> .
:precision_at_recall a :Metric ;
    skos:prefLabel "precision at recall" ;
    :used_for :classification ;
    rdfs:comment "Computes best precision where recall is >= specified value." .
:precision_macro a :Metric ;
    skos:prefLabel "precision macro" ;
    :used_for :classification .
:precision_micro a :Metric ;
    skos:prefLabel "precision micro" ;
    :used_for :classification .
:precision_samples a :Metric ;
    skos:prefLabel "precision samples" ;
    :used_for :classification .
:precision_weighted a :Metric ;
    skos:prefLabel "precision weighted" ;
    :used_for :classification .
:prevalence_threshold a :Metric ;
    skos:prefLabel "prevalence threshold" ;
    skos:altLabel "PT" .
:recall a :Metric ;
    skos:prefLabel "recall" ;
    skos:altLabel "sensitivity" , "hit rate" , "true positive rate" , "TPR" ;
    :used_for :classification ;
    rdfs:comment "retrieval of events or information from the past" ;
    rdfs:seeAlso <https://www.wikidata.org/entity/Q18733> .
:recall_at_precision a :Metric ;
    skos:prefLabel "recall at precision" ;
    :used_for :classification .
:recall_macro a :Metric ;
    skos:prefLabel "recall macro" ;
    :used_for :classification .
:recall_micro a :Metric ;
    skos:prefLabel "recall micro" ;
    :used_for :classification .
:recall_samples a :Metric ;
    skos:prefLabel "recall samples" ;
    :used_for :classification .
:recall_weighted a :Metric ;
    skos:prefLabel "recall weighted" ;
    :used_for :classification .
:receiver_operating_characteristic_curve a :Metric ;
    skos:prefLabel "receiver operating characteristic curve" ;
    skos:altLabel "ROC AUC" ;
    :used_for :classification , :regression .
:receiver_operating_characteristic_curve_one_vs_one a :Metric ;
    skos:prefLabel "receiver operating characteristic curve one vs one" ;
    skos:altLabel "ROC AUC OVO" ;
    :used_for :classification , :regression .
:receiver_operating_characteristic_curve_one_vs_rest a :Metric ;
    skos:prefLabel "receiver operating characteristic curve one vs rest" ;
    skos:altLabel "ROC AUC OVR" ;
    :used_for :classification , :regression .
:rooted_mean_squared_error a :Metric ;
    skos:prefLabel "rooted mean squared error" ;
    skos:altLabel "RMSE" ;
    :used_for :regression .
:rooted_mean_squared_log_error a :Metric ;
    skos:prefLabel "rooted mean squared log error" ;
    skos:altLabel "RMSLE" ;
    :used_for :regression .
:rooted_mean_squared_scaled_error a :Metric ;
    skos:prefLabel "rooted mean squared scaled error" ;
    skos:altLabel "RMSSE" ;
    :used_for :time_series_forecasting .
:sensitifity_at_specificity a :Metric ;
    skos:prefLabel "sensitifity at specificity" ;
    :used_for :classification .
:sparse_categorical_accuracy a :Metric ;
    skos:prefLabel "sparse categorical accuracy" ;
    :used_for :classification ;
    rdfs:comment "Calculates how often predictions match integer labels." .
:sparse_categorical_crossentropy a :Metric ;
    skos:prefLabel "sparse categorical crossentropy" ;
    :used_for :classification .
:sparse_top_k_categorical_accuracy a :Metric ;
    skos:prefLabel "sparse top k categorical accuracy" ;
    :used_for :classification ;
    rdfs:comment "Computes how often integer targets are in the top K predictions." .
:spearman_rank_correlation_coefficient a :Metric ;
    skos:prefLabel "Spearman rank correlation coefficient" ;
    skos:altLabel "spearmanr" ;
    :used_for :regression ;
    rdfs:comment "nonparametric measure of rank correlation" ;
    rdfs:seeAlso <https://www.wikidata.org/entity/Q1126730> .
:specificity a :Metric ;
    skos:prefLabel "specificity" ;
    skos:altLabel "selectivity" , "true negative rate" , "TNR" .
:specificity_at_sensitivity a :Metric ;
    skos:prefLabel "specificity at sensitivity" ;
    :used_for :classification .
:squared_hinge a :Metric ;
    skos:prefLabel "squared hinge" ;
    :used_for :classification .
:sum a :Metric ;
    skos:prefLabel "sum" .
:top_k_categorical_accuracy a :Metric ;
    skos:prefLabel "top k categorical accuracy" ;
    :used_for :classification ;
    rdfs:comment "Computes how often targets are in the top K predictions." .
:true_negatives a :Metric ;
    skos:prefLabel "true negatives" ;
    skos:altLabel "TN" ;
    :used_for :classification .
:true_positives a :Metric ;
    skos:prefLabel "true positives" ;
    skos:altLabel "TP" ;
    :used_for :classification .
:r2 a :Metric ;
    skos:prefLabel "r2" ;
    skos:altLabel "R2 scrore" ;
    :used_for :regression .
:brier a :Metric ;
    skos:prefLabel "brier" ;
    :used_for :classification .
:mean_poisson_deviance a :Metric ;
    skos:prefLabel "mean poisson deviance" ;
    :used_for :regression .
:mean_gamma_deviance a :Metric ;
    skos:prefLabel "mean gamma deviance" ;
    :used_for :regression .
:d2_absolute_error a :Metric ;
    skos:prefLabel "d2 absolute error" ;
    :used_for :regression .
:d2_pinball_score a :Metric ;
    skos:prefLabel "d2 pinball score" ;
    :used_for :regression .
:d2_tweedie_score a :Metric ;
    skos:prefLabel "d2 tweedie score" ;
    :used_for :regression .
:coverage a :Metric ;
    skos:prefLabel "Coverage" ;
    :used_for :time_series_forecasting ;
    rdfs:comment "Percentage of actual values that are within the prediction intervall" .


# ML_library

:catboost_lib a :ML_library ;
    skos:prefLabel "CatBoost" ;
    rdfs:seeAlso <https://www.wikidata.org/entity/Q55656976> .
:fastai_lib a :ML_library ;
    skos:prefLabel "Fastai" ;
    rdfs:seeAlso <https://www.wikidata.org/entity/Q96377821> .
:h2o_lib a :ML_library ;
    skos:prefLabel "H2O" ;
    rdfs:seeAlso <https://www.wikidata.org/entity/Q16972732> .
:keras_lib a :ML_library ;
    skos:prefLabel "Keras" ;
    skos:broader :tensorflow_lib ;
    rdfs:seeAlso <https://www.wikidata.org/entity/Q28470421> .
:lightgbm_lib a :ML_library ;
    skos:prefLabel "LightGBM" ;
    rdfs:seeAlso <https://www.wikidata.org/entity/Q57267665> .
:mxnet_lib a :ML_library ;
    skos:prefLabel "MXNET" ;
    rdfs:seeAlso <https://www.wikidata.org/entity/Q22348165> .
:prophet_lib a :ML_library ;
    skos:prefLabel "Prophet" ;
    rdfs:comment "Prophet is a procedure for forecasting time series data based on an additive model where non-linear trends are fit with yearly, weekly, and daily seasonality, plus holiday effects. It works best with time series that have strong seasonal effects and several seasons of historical data. Prophet is robust to missing data and shifts in the trend, and typically handles outliers well." .
:pytorch_lib a :ML_library ;
    skos:prefLabel "Pytorch" ;
    rdfs:seeAlso <https://www.wikidata.org/entity/Q47509047> .
:scikit_learn_lib a :ML_library ;
    skos:prefLabel "Scikit-learn" ;
    skos:altLabel "sklearn" ;
    rdfs:seeAlso <https://www.wikidata.org/entity/Q1026367> .
:mllib_lib a :ML_library ;
    skos:prefLabel "MLlib" ;
    rdfs:comment "MLlib fits into Spark's APIs and interoperates with NumPy in Python (as of Spark 0.9) and R libraries (as of Spark 1.5). You can use any Hadoop data source (e.g. HDFS, HBase, or local files), making it easy to plug into Hadoop workflows." .
:statsmodel_lib a :ML_library ;
    skos:prefLabel "Statsmodel" ;
    rdfs:seeAlso <https://www.wikidata.org/entity/Q25304899> .
:tensorflow_lib a :ML_library ;
    skos:prefLabel "TensorFlow" ;
    rdfs:seeAlso <https://www.wikidata.org/entity/Q21447895> .
:weka_lib a :ML_library ;
    skos:prefLabel "Weka" ;
    rdfs:seeAlso <https://www.wikidata.org/entity/Q115494> .
:xgboost_lib a :ML_library ;
    skos:prefLabel "XGBoost" ;
    rdfs:seeAlso <https://www.wikidata.org/entity/Q23793561> .
:sktime_lib a :ML_library ;
    skos:prefLabel "sktime" ;
    rdfs:comment "sktime provides an easy-to-use, flexible and modular open-source framework for a wide range of time series machine learning tasks. It offers scikit-learn compatible interfaces and model composition tools, with the goal to make the ecosystem more usable and interoperable as a whole." .
:tslearn_lib a :ML_library ;
    skos:prefLabel "tslearn" ;
    rdfs:comment "tslearn is a Python package that provides machine learning tools for the analysis of time series. This package builds on (and hence depends on) scikit-learn, numpy and scipy libraries." .
:pywavelets_lib a :ML_library ;
    skos:prefLabel "PyWavelets" ;
    rdfs:comment "PyWavelets is open source wavelet transform software for Python. It combines a simple high level interface with low level C and Cython performance." .
:pmdarima_lib a :ML_library ;
    skos:prefLabel "pmdarima" ;
    rdfs:comment "Pmdarima is a statistical library designed to fill the void in Python's time series analysis capabilities." .
:gluonts_lib a :ML_library ;
    skos:prefLabel "GluonTS" ;
    rdfs:comment "GluonTS is a Python package for probabilistic time series modeling, focusing on deep learning based models, based on PyTorch and MXNet." .
:pytorch_forecasting_lib a :ML_library ;
    skos:prefLabel "Pytorch-Forecasting" ;
    rdfs:comment "PyTorch Forecasting aims to ease state-of-the-art timeseries forecasting with neural networks for both real-world cases and research alike. The goal is to provide a high-level API with maximum flexibility for professionals and reasonable defaults for beginners. Specifically, the package provides" .
:ibm_snap_ml_lib a :ML_library ;
    skos:prefLabel "IBM Snap ML" ;
    rdfs:comment "Snap ML is a library for training generalized linear models.It supports a large number of classical machine learning models and scales gracefully to data sets with billions of examples and/or features. It offers distributed training, GPU acceleration and supports sparse data structures." .
:pyflux_lib a :ML_library ;
    skos:prefLabel "PyFlux" ;
    rdfs:comment "PyFlux is a library for time series analysis and prediction." .
:tsfresh_lib a :ML_library ;
    skos:prefLabel "tsfresh" ;
    rdfs:seeAlso <https://www.wikidata.org/entity/Q107384267> .
:greykite_lib a :ML_library ;
    skos:prefLabel "GreyKite" ;
    rdfs:comment "A flexible, intuitive and fast forecasting library" .
:kats_lib a :ML_library ;
    skos:prefLabel "Kats" ;
    rdfs:comment "Kats, a kit to analyze time series data, a lightweight, easy-to-use, generalizable, and extendable framework to perform time series analysis, from understanding the key statistics and characteristics, detecting change points and anomalies, to forecasting future trends." .


# AutoML_solution

:adanet a :AutoML_solution ;
    skos:prefLabel "Adanet" ;
    :used_for :tensorflow_lib ;
    :can_perform :tabular_classification , :tabular_regression .
:alphad3m a :AutoML_solution ;
    skos:prefLabel "Alphad3m" ;
    :used_for :scikit_learn_lib , :pywavelets_lib , :pytorch ;
    :can_perform :tabular_classification , :tabular_regression , :clustering , :time_series_forecasting , :time_series_classification , :text_classification , :text_regression , :image_classification , :object_detection , :remote_sensing , :video_classification , :audio_classification , :audio_regression , :collaborative_graph_filtering , :graph_matching , :vertex_classification , :link_prediction , :community_detection .
:analytics_zoo_chronos a :AutoML_solution ;
    skos:prefLabel "Analytics Zoo Chronos" ;
    :used_for :prophet_lib , :tensorflow_lib , :pytorch_lib , :pmdarima_lib ;
    :can_perform :time_series_forecasting .
:atm a :AutoML_solution ;
    skos:prefLabel "ATM" ;
    :used_for :scikit_learn_lib ;
    :can_perform :tabular_classification , :tabular_regression .
:auto_timeseries a :AutoML_solution ;
    skos:prefLabel "Auto_TimeSeries" ;
    :used_for :scikit_learn_lib , :pmdarima_lib , :prophet_lib , :pyflux_lib , :statsmodel_lib , :xgboost_lib ;
    :can_perform :time_series_forecasting .
:auto_weka a :AutoML_solution ;
    skos:prefLabel "Auto-Weka" ;
    :used_for :weka_lib ;
    :can_perform :tabular_classification , :tabular_regression , :clustering , :time_series_forecasting .
:autocve a :AutoML_solution ;
    skos:prefLabel "AutoCVE" ;
    :used_for :xgboost_lib , :scikit_learn_lib ;
    :can_perform :tabular_classification .
:autogluon a :AutoML_solution ;
    skos:prefLabel "Autogluon" ;
    :used_for :scikit_learn_lib , :catboost_lib , :lightgbm_lib , :xgboost_lib , :pytorch_lib , :mxnet_lib ;
    :supported_by_oma_ml "True" ;
    :can_perform :tabular_classification , :tabular_regression , :text_classification , :text_regression , :sentiment_analysis , :sentence_similarity , :image_classification , :object_detection , :video_classification , :video_object_tracking , :action_recognition , :time_series_forecasting .
:autokeras a :AutoML_solution ;
    skos:prefLabel "Autokeras" ;
    :used_for :keras_lib ;
    :supported_by_oma_ml "True" ;
    :can_perform :tabular_classification , :tabular_regression , :time_series_forecasting , :text_classification , :text_regression , :image_classification , :image_regression .
:autopytorch a :AutoML_solution ;
    skos:prefLabel "Autopytorch" ;
    :used_for :pytorch_lib , :pytorch_forecasting_lib ;
    :supported_by_oma_ml "True" ;
    :can_perform :tabular_classification , :tabular_regression , :image_classification , :time_series_forecasting .
:autosklearn a :AutoML_solution ;
    skos:prefLabel "Autosklearn" ;
    :used_for :scikit_learn_lib ;
    :supported_by_oma_ml "True" ;
    :can_perform :tabular_classification , :tabular_regression .
:autots a :AutoML_solution ;
    skos:prefLabel "AutoTS" ;
    :used_for :prophet_lib , :pytorch_lib , :gluonts_lib , :pmdarima_lib , :tensorflow_lib ;
    :can_perform :time_series_forecasting .
:aws_sagemaker_autopilot a :AutoML_solution ;
    skos:prefLabel "AWS Sagemaker Autopilot" ;
    :used_for :scikit_learn_lib , :tsfresh_lib , :gluon_ts , :xgboost_lib , :fastai_lib ;
    :can_perform :tabular_classification , :tabular_regression , :time_series_classification .
:azure_automl a :AutoML_solution ;
    skos:prefLabel "Azure AutoML" ;
    :can_perform :tabular_classification , :tabular_regression , :time_series_forecasting , :text_classification , :image_classification , :object_detection , :instance_segmentation .
:databricks a :AutoML_solution ;
    skos:prefLabel "Databricks" ;
    :used_for :pmdarima_lib , :prophet_lib , :tensorflow_lib , :xgboost_lib ;
    :can_perform :time_series_forecasting .
:datarobot a :AutoML_solution ;
    skos:prefLabel "DataRobot" ;
    :used_for :pmdarima_lib , :prophet_lib , :tensorflow_lib , :xgboost_lib ;
    :can_perform :time_series_forecasting , :time_series_classification .
:evalml a :AutoML_solution ;
    skos:prefLabel "EvalML" ;
    :used_for :scikit_learn_lib , :catboost_lib , :lightgbm_lib , :xgboost_lib ;
    :supported_by_oma_ml "True" ;
    :can_perform :tabular_classification , :tabular_regression , :time_series_forecasting , :time_series_classification , :text_classification , :text_regression .
:fedot a :AutoML_solution ;
    skos:prefLabel "FEDOT" ;
    :used_for :scikit_learn_lib , :statsmodel_lib ;
    :can_perform :time_series_forecasting .
:flaml a :AutoML_solution ;
    skos:prefLabel "FLAML" ;
    :used_for :scikit_learn_lib , :catboost_lib , :lightgbm_lib , :xgboost_lib , :prophet_lib ;
    :supported_by_oma_ml "True" ;
    :can_perform :tabular_classification , :tabular_regression , :ranking , :time_series_forecasting , :text_classification .
:google_automl a :AutoML_solution ;
    skos:prefLabel "Google AutoML" ;
    :used_for :tensorflow_lib ;
    :can_perform :tabular_classification , :tabular_regression , :time_series_forecasting .
:h2o_automl a :AutoML_solution ;
    skos:prefLabel "H2O Automl" ;
    :used_for :h2o_lib , :xgboost_lib ;
    :can_perform :tabular_classification , :tabular_regression , :time_series_forecasting , :text_classification , :sentiment_analysis , :entity_extraction , :translation , :image_classification , :image_object_tracking , :video_classification , :video_object_tracking , :action_recognition .
:ibm_autoai a :AutoML_solution ;
    skos:prefLabel "IBM AutoAI" ;
    :used_for :ibm_snap_ml_lib , :scikit_learn_lib , :tensorflow_lib , :xgboost_lib ;
    :can_perform :time_series_forecasting .
:mcfly a :AutoML_solution ;
    skos:prefLabel "Mcfly" ;
    :used_for :tensorflow_lib ;
    :supported_by_oma_ml "True" ;
    :can_perform :time_series_classification .
:merlion a :AutoML_solution ;
    skos:prefLabel "Merlion" ;
    :used_for :lightgbm_lib , :prophet_lib , :scikit_learn_lib , :statsmodel_lib , :greykite_lib , :kats_lib ;
    :can_perform :time_series_forecasting .
:mlbox a :AutoML_solution ;
    skos:prefLabel "MLBOX" ;
    :used_for :keras_lib , :scikit_learn_lib ;
    :can_perform :tabular_classification , :tabular_regression .
:mljar a :AutoML_solution ;
    skos:prefLabel "MLJAR" ;
    :used_for :scikit_learn_lib , :catboost_lib , :lightgbm_lib , :xgboost_lib ;
    :supported_by_oma_ml "True" ;
    :can_perform :tabular_classification , :tabular_regression .
:rapidminer a :AutoML_solution ;
    skos:prefLabel "Rapidminer" ;
    :used_for :weka_lib , :h2o_lib ;
    :can_perform :tabular_classification , :tabular_regression , :clustering , :outlier_detection , :time_series_forecasting .
:remi_ai a :AutoML_solution ;
    skos:prefLabel "Remi AI" ;
    :can_perform :time_series_forecasting .
:tpot a :AutoML_solution ;
    skos:prefLabel "TPOT" ;
    :used_for :scikit_learn_lib , :pytorch_lib ;
    :supported_by_oma_ml "True" ;
    :can_perform :tabular_classification , :tabular_regression .
:transmogrifai a :AutoML_solution ;
    skos:prefLabel "TransmogrifAI" ;
    :used_for :spark_mllib ;
    :can_perform :tabular_classification , :tabular_regression .
:pycaret a :AutoML_solution ;
    skos:prefLabel "Pycaret" ;
    :used_for :scikit_learn_lib , :catboost_lib , :lightgbm_lib , :xgboost_lib ;
    :supported_by_oma_ml "True" ;
    :can_perform :tabular_classification , :tabular_regression , :clustering , :anomaly_detection , :time_series_forecasting .


# Enum

:category_type a :Enum ;
    skos:prefLabel "category type" ;
    :category :category_type .
:datatype a :Enum ;
    skos:prefLabel "datatype" ;
    :category :category_type ;
    rdfs:comment "part of RDF; used with RDF literals to represent values such as strings, numbers and dates. The datatype abstraction used in RDF is compatible with XML Schema" ;
    rdfs:seeAlso <https://www.wikidata.org/entity/Q31385480> .
:task_configuration a :Enum ;
    skos:prefLabel "task configuration" ;
    :category :category_type .
:parameter a :Enum ;
    skos:prefLabel "parameter" ;
    :category :category_type ;
    rdfs:comment "variable in computer programming; special kind of variable, used in a subroutine to refer to one of the pieces of data provided as input to the subroutine. These pieces of data are called arguments" ;
    rdfs:seeAlso <https://www.wikidata.org/entity/Q1410440> .
:approach a :Enum ;
    skos:prefLabel "approach" ;
    :category :category_type .
:hardware a :Enum ;
    skos:prefLabel "hardware" ;
    :category :category_type ;
    rdfs:comment "physical components of a computer" ;
    rdfs:seeAlso <https://www.wikidata.org/entity/Q3966> .
:limitation a :Enum ;
    skos:prefLabel "limitation" ;
    :category :category_type .
:characteristic a :Enum ;
    skos:prefLabel "characteristic" ;
    :category :category_type ;
    rdfs:comment "Basic properties of datasets or ML approaches that can be used to chacterize ML approaches or ML prediction performance measures; e.g., balanced / unbalanced datasets that influence the choice of ML prediction performance measures." .
:dataset_type a :Enum ;
    skos:prefLabel "dataset type" ;
    :category :category_type .
:tuner_approach a :Enum ;
    skos:prefLabel "tuner approach" ;
    :category :category_type .
:inheritance_type a :Enum ;
    skos:prefLabel "inheritance type" ;
    :category :category_type .
:column_role a :Enum ;
    skos:prefLabel "column role" ;
    :category :category_type .
:integer a :Enum ;
    skos:prefLabel "integer" ;
    :category :datatype ;
    rdfs:comment "datum of integral data type" ;
    rdfs:seeAlso <https://www.wikidata.org/entity/Q729138> .
:float a :Enum ;
    skos:prefLabel "float" ;
    :category :datatype ;
    rdfs:comment "computer format for representing real numbers" ;
    rdfs:seeAlso <https://www.wikidata.org/entity/Q117879> .
:boolean a :Enum ;
    skos:prefLabel "boolean" ;
    :category :datatype ;
    rdfs:comment "basic computing representation of truth and falsehood" ;
    rdfs:seeAlso <https://www.wikidata.org/entity/Q520777> .
:string a :Enum ;
    skos:prefLabel "string" ;
    :category :datatype ;
    rdfs:comment "data type representing a finite sequence of encoded characters" ;
    rdfs:seeAlso <https://www.wikidata.org/entity/Q184754> .
:categorical a :Enum ;
    skos:prefLabel "categorical" ;
    :category :datatype .
:datetime a :Enum ;
    skos:prefLabel "datetime" ;
    :category :datatype .
:time_delta a :Enum ;
    skos:prefLabel "time delta" ;
    :category :datatype .
:list a :Enum ;
    skos:prefLabel "list" ;
    :category :datatype .
:single_value a :Enum ;
    skos:prefLabel "single value" ;
    :category :datatype ;
    rdfs:comment "Denotes a single value from a list of options which is provided as a parameter of a :Configuration_item" .
:index a :Enum ;
    skos:prefLabel "index" ;
    :category :column_role .
:target a :Enum ;
    skos:prefLabel "target" ;
    :category :column_role .
:ignore a :Enum ;
    skos:prefLabel "ignore" ;
    :category :column_role .
:balanced_dataset a :Enum ;
    skos:prefLabel "balanced dataset" ;
    :category :characteristic .
:unbalanced_dataset a :Enum ;
    skos:prefLabel "unbalanced dataset" ;
    :category :characteristic .
:missing_values a :Enum ;
    skos:prefLabel "missing values" ;
    :category :characteristic .
:numerical_features a :Enum ;
    skos:prefLabel "numerical features" ;
    :category :characteristic .
:ordinal_features a :Enum ;
    skos:prefLabel "ordinal features" ;
    :category :characteristic .
:categorical_features a :Enum ;
    skos:prefLabel "categorical features" ;
    :category :characteristic .
:text_features a :Enum ;
    skos:prefLabel "text features" ;
    :category :characteristic .
:small_dataset a :Enum ;
    skos:prefLabel "small dataset" ;
    :category :characteristic .
:large_dataset a :Enum ;
    skos:prefLabel "large dataset" ;
    :category :characteristic .
:fast_training a :Enum ;
    skos:prefLabel "fast training" ;
    :category :characteristic .
:long_training_time a :Enum ;
    skos:prefLabel "long training time" ;
    :category :characteristic .
:many_features a :Enum ;
    skos:prefLabel "many features" ;
    :category :characteristic .
:accurate a :Enum ;
    skos:prefLabel "accurate" ;
    :category :characteristic .
:small_memory_footprint a :Enum ;
    skos:prefLabel "small memory footprint" ;
    :category :characteristic .
:large_memory_footprint a :Enum ;
    skos:prefLabel "large memory footprint" ;
    :category :characteristic .
:explainable a :Enum ;
    skos:prefLabel "explainable" ;
    :category :characteristic .
:scalable a :Enum ;
    skos:prefLabel "scalable" ;
    :category :characteristic .
:tabular a :Enum ;
    skos:prefLabel "tabular" ;
    :category :dataset_type ;
    rdfs:comment "A dataset presented in a tabular (table with rows and columns) form (CSV file)?=?.csv?=?Additional-Info-About-File-Structure" ;
    :supported_by_oma_ml "True" .
:text a :Enum ;
    skos:prefLabel "text" ;
    :category :dataset_type ;
    rdfs:comment "A dataset presented in a tabular (table with rows and columns) form (CSV file)?=?.csv?=?Additional-Info-About-File-Structure" ;
    :supported_by_oma_ml "True" .
:image a :Enum ;
    skos:prefLabel "image" ;
    :category :dataset_type ;
    rdfs:comment "A dataset presented in a folder structure of image files ordered by label form (ZIP file)?=?.zip?=?Additional-Info-About-File-Structure" ;
    :supported_by_oma_ml "True" .
:video a :Enum ;
    skos:prefLabel "video" ;
    :category :dataset_type ;
    :supported_by_oma_ml "false" .
:audio a :Enum ;
    skos:prefLabel "audio" ;
    :category :dataset_type ;
    :supported_by_oma_ml "false" .
:graph a :Enum ;
    skos:prefLabel "graph" ;
    :category :dataset_type ;
    :supported_by_oma_ml "false" .
:time_series_longitudinal a :Enum ;
    skos:prefLabel "time series longitudinal" ;
    :category :dataset_type ;
    rdfs:comment "Longitudinal data - also called panel data - for time series classification, which has 3 dimensions: (num_samples, num_features, num_timesteps)?=?.ts?=?Additional-Info-About-File-Structure" ;
    :supported_by_oma_ml "True" .
:time_series a :Enum ;
    skos:prefLabel "time series" ;
    :category :dataset_type ;
    rdfs:comment "A dataset presented in a tabular (table with rows and columns) form (CSV file)?=?.csv?=?Additional-Info-About-File-Structure" ;
    :supported_by_oma_ml "True" .
:greedy a :Enum ;
    skos:prefLabel "greedy" ;
    :category :tuner_approach ;
    rdfs:comment "algorithm that makes locally optimal choices in a sequence of steps with the goal of reaching a global optimum" ;
    rdfs:seeAlso <https://www.wikidata.org/entity/Q504353> .
:bayesian a :Enum ;
    skos:prefLabel "bayesian" ;
    :category :tuner_approach .
:hyperband a :Enum ;
    skos:prefLabel "hyperband" ;
    :category :tuner_approach .
:random a :Enum ;
    skos:prefLabel "random" ;
    :category :tuner_approach .
:grid_search a :Enum ;
    skos:prefLabel "grid search" ;
    :category :tuner_approach .
:skopt a :Enum ;
    skos:prefLabel "skopt" ;
    :category :tuner_approach .
:broader_inherited a :Enum ;
    skos:prefLabel "broader inherited" ;
    :category :inheritance_type .


# Configuration_item

:tabular_classification_in_autosklearn a :Configuration_item ;
    skos:prefLabel "tabular classification in Autosklearn" ;
    :category :task_configuration ;
    :automl_solution :autosklearn ;
    :ml_task :tabular_classification ;
    :parameter_value :time_limit_autosklearn , :time_limit_per_run_autosklearn , :ensemble_size_autosklearn , :ensemble_nbest_autosklearn , :use_approach_autosklearn_classification , :metric_autosklearn_classification , :exclude_preprocessor_autosklearn .
:tabular_regression_in_autosklearn a :Configuration_item ;
    skos:prefLabel "tabular regression in Autosklearn" ;
    :category :task_configuration ;
    :automl_solution :autosklearn ;
    :ml_task :tabular_regression ;
    :parameter_value :metric_autosklearn_regression , :exclude_preprocessor_autosklearn .
:tabular_classification_in_autokeras a :Configuration_item ;
    skos:prefLabel "tabular classification in AutoKeras" ;
    :category :task_configuration ;
    :automl_solution :autokeras ;
    :ml_task :tabular_classification ;
    :parameter_value :metric_autokeras_tabular_classification , :loss_autokeras_tabular_classification , :max_trials_autokeras , :tuner_autokeras_tabular_classification , :max_model_size_autokeras .
:tabular_regression_in_autokeras a :Configuration_item ;
    skos:prefLabel "tabular regression in AutoKeras" ;
    :category :task_configuration ;
    :automl_solution :autokeras ;
    :ml_task :tabular_regression ;
    :parameter_value :metric_autokeras_tabular_regression , :loss_autokeras_tabular_regression , :max_trials_autokeras , :tuner_autokeras_tabular_regression , :max_model_size_autokeras .
:tabular_classification_in_flaml a :Configuration_item ;
    skos:prefLabel "tabular classification in FLAML" ;
    :category :task_configuration ;
    :automl_solution :flaml ;
    :ml_task :tabular_classification ;
    :parameter_value :use_approach_flaml_tabular_classification , :metric_flaml_tabular_classification .
:tabular_regression_in_flaml a :Configuration_item ;
    skos:prefLabel "tabular regression in FLAML" ;
    :category :task_configuration ;
    :automl_solution :flaml ;
    :ml_task :tabular_regression ;
    :parameter_value :use_approach_flaml_tabular_regression , :metric_flaml_tabular_regression .
:ranking_in_flaml a :Configuration_item ;
    skos:prefLabel "ranking in FLAML" ;
    :category :task_configuration ;
    :automl_solution :flaml ;
    :ml_task :ranking ;
    :parameter_value :use_approach_flaml_ranking , :metric_flaml_ranking .
:time_series_analysis_in_flaml a :Configuration_item ;
    skos:prefLabel "time series analysis in FLAML" ;
    :category :task_configuration ;
    :automl_solution :flaml ;
    :ml_task :time_series_analysis ;
    :parameter_value :use_approach_flaml_time_series_analysis , :metric_flaml_time_series_analysis .
:text_classification_in_flaml a :Configuration_item ;
    skos:prefLabel "text classification in FLAML" ;
    :category :task_configuration ;
    :automl_solution :flaml ;
    :ml_task :text_classification ;
    :parameter_value :use_approach_flaml_text_classification , :metric_flaml_text_classification .
:text_regression_in_flaml a :Configuration_item ;
    skos:prefLabel "text regression in FLAML" ;
    :category :task_configuration ;
    :automl_solution :flaml ;
    :ml_task :text_regression ;
    :parameter_value :use_approach_flaml_text_regression , :metric_flaml_text_regression .
:tabular_classification_in_auto_pytorch a :Configuration_item ;
    skos:prefLabel "tabular classification in Auto-PyTorch" ;
    :category :task_configuration ;
    :automl_solution :autopytorch ;
    :ml_task :tabular_classification ;
    :parameter_value :use_approach_auto_pytorch_classification , :metric_auto_pytorch_classification .
:tabular_regression_in_auto_pytorch a :Configuration_item ;
    skos:prefLabel "tabular regression in Auto-PyTorch" ;
    :category :task_configuration ;
    :automl_solution :autopytorch ;
    :ml_task :tabular_regression ;
    :parameter_value :use_approach_auto_pytorch_regression , :metric_auto_pytorch_regression .
:tabular_classification_in_autogluon a :Configuration_item ;
    skos:prefLabel "tabular classification in AutoGluon" ;
    :category :task_configuration ;
    :automl_solution :autogluon ;
    :ml_task :tabular_classification ;
    :parameter_value :use_approach_autogluon_classification , :metric_autogluon_tabular_classification .
:tabular_regression_in_autogluon a :Configuration_item ;
    skos:prefLabel "tabular regression in AutoGluon" ;
    :category :task_configuration ;
    :automl_solution :autogluon ;
    :ml_task :tabular_regression ;
    :parameter_value :use_approach_autogluon_regression , :metric_autogluon_tabular_regression .
:image_classification_in_autogluon a :Configuration_item ;
    skos:prefLabel "image classification in AutoGluon" ;
    :category :task_configuration ;
    :automl_solution :autogluon ;
    :ml_task :image_classification ;
    :parameter_value :use_approach_autogluon_image_classification , :metric_autogluon_image_classification .
:text_classification_in_autogluon a :Configuration_item ;
    skos:prefLabel "text classification in AutoGluon" ;
    :category :task_configuration ;
    :automl_solution :autogluon ;
    :ml_task :text_classification ;
    :parameter_value :use_approach_autogluon_text_classification , :metric_autogluon_text_classification .
:text_regression_in_autogluon a :Configuration_item ;
    skos:prefLabel "text regression in AutoGluon" ;
    :category :task_configuration ;
    :automl_solution :autogluon ;
    :ml_task :text_regression ;
    :parameter_value :use_approach_autogluon_text_regression , :metric_autogluon_text_regression .
:object_detection_in_autogluon a :Configuration_item ;
    skos:prefLabel "object detection in AutoGluon" ;
    :category :task_configuration ;
    :automl_solution :autogluon ;
    :ml_task :object_detection ;
    :parameter_value :use_approach_autogluon_object_detection .
:time_series_forecasting_in_autogluon a :Configuration_item ;
    skos:prefLabel "time series forecasting in AutoGluon" ;
    :category :task_configuration ;
    :automl_solution :autogluon ;
    :ml_task :time_series_forecasting ;
    :parameter_value :metric_autogluon_time_series_forecasting .
:tabular_classification_in_autocve a :Configuration_item ;
    skos:prefLabel "tabular classification in AutoCVE" ;
    :category :task_configuration ;
    :automl_solution :autocve ;
    :ml_task :tabular_classification ;
    :parameter_value :use_approach_autocve_classification , :metric_autocve_classification .
:time_series_classification_in_mcfly a :Configuration_item ;
    skos:prefLabel "time series classification in mcfly" ;
    :category :task_configuration ;
    :automl_solution :mcfly ;
    :ml_task :time_series_classification ;
    :parameter_value :use_approach_mcfly_time_series_classification , :metric_mcfly_time_series_classification .
:image_classification_in_autokeras a :Configuration_item ;
    skos:prefLabel "image classification in AutoKeras" ;
    :category :task_configuration ;
    :automl_solution :autokeras ;
    :ml_task :image_classification ;
    :parameter_value :metric_autokeras_image_classification , :loss_autokeras_image_classification , :max_trials_autokeras , :tuner_autokeras_image_classification , :max_model_size_autokeras .
:image_regression_in_autokeras a :Configuration_item ;
    skos:prefLabel "image regression in AutoKeras" ;
    :category :task_configuration ;
    :automl_solution :autokeras ;
    :ml_task :image_regression ;
    :parameter_value :metric_autokeras_image_regression , :loss_autokeras_image_regression , :max_trials_autokeras , :tuner_autokeras_image_regression , :max_model_size_autokeras .
:text_classification_in_autokeras a :Configuration_item ;
    skos:prefLabel "text classification in AutoKeras" ;
    :category :task_configuration ;
    :automl_solution :autokeras ;
    :ml_task :text_classification ;
    :parameter_value :metric_autokeras_text_classification , :loss_autokeras_text_classification , :max_trials_autokeras , :tuner_autokeras_text_classification , :max_model_size_autokeras .
:text_regression_in_autokeras a :Configuration_item ;
    skos:prefLabel "text regression in AutoKeras" ;
    :category :task_configuration ;
    :automl_solution :autokeras ;
    :ml_task :text_regression ;
    :parameter_value :metric_autokeras_text_regression , :loss_autokeras_text_regression , :max_trials_autokeras , :tuner_autokeras_text_regression , :max_model_size_autokeras .
:tabular_classification_in_evalml a :Configuration_item ;
    skos:prefLabel "tabular classification in EvalML" ;
    :category :task_configuration ;
    :automl_solution :evalml ;
    :ml_task :tabular_classification ;
    :parameter_value :use_approach_evalml_tabular_classification , :metric_evalml_tabular_classification , :tuner_class_evalml .
:tabular_regression_in_evalml a :Configuration_item ;
    skos:prefLabel "tabular regression in EvalML" ;
    :category :task_configuration ;
    :automl_solution :evalml ;
    :ml_task :tabular_regression ;
    :parameter_value :use_approach_evalml_tabular_regression , :metric_evalml_tabular_regression , :tuner_class_evalml .
:text_classification_in_evalml a :Configuration_item ;
    skos:prefLabel "text classification in EvalML" ;
    :category :task_configuration ;
    :automl_solution :evalml ;
    :ml_task :text_classification ;
    :parameter_value :use_approach_evalml_tabular_classification , :metric_evalml_text_classification , :tuner_class_evalml .
:text_regression_in_evalml a :Configuration_item ;
    skos:prefLabel "text regression in EvalML" ;
    :category :task_configuration ;
    :automl_solution :evalml ;
    :ml_task :text_regression ;
    :parameter_value :use_approach_evalml_tabular_regression , :metric_evalml_text_regression , :tuner_class_evalml .
:time_series_classification_in_evalml a :Configuration_item ;
    skos:prefLabel "time series classification in EvalML" ;
    :category :task_configuration ;
    :automl_solution :evalml ;
    :ml_task :time_series_classification ;
    :parameter_value :use_approach_evalml_time_series_classification , :metric_evalml_classification , :tuner_class_evalml .
:time_series_regression_in_evalml a :Configuration_item ;
    skos:prefLabel "time series regression in EvalML" ;
    :category :task_configuration ;
    :automl_solution :evalml ;
    :ml_task :time_series_forecasting ;
    :parameter_value :use_approach_evalml_time_series_regression , :metric_evalml_time_series_regression , :tuner_class_evalml .
:time_series_forecasting_in_autokeras a :Configuration_item ;
    skos:prefLabel "time series forecasting in AutoKeras" ;
    :category :task_configuration ;
    :automl_solution :autokeras ;
    :ml_task :time_series_forecasting ;
    :parameter_value :metric_autokeras_time_series_forecasting , :loss_autokeras_time_series_forecasting , :max_trials_autokeras , :tuner_autokeras_time_series_forecasting , :max_model_size_autokeras .
:tabular_classification_mljar a :Configuration_item ;
    skos:prefLabel "tabular classification MLJAR" ;
    :category :task_configuration ;
    :automl_solution :mljar ;
    :ml_task :tabular_classification ;
    :parameter_value :metric_mljar_tabular_classification .
:tabular_regression_mljar a :Configuration_item ;
    skos:prefLabel "tabular regression MLJAR" ;
    :category :task_configuration ;
    :automl_solution :mljar ;
    :ml_task :tabular_regression ;
    :parameter_value :metric_mljar_tabular_regression .
:tabular_classification_pycaret a :Configuration_item ;
    skos:prefLabel "tabular classification PyCaret" ;
    :category :task_configuration ;
    :automl_solution :pycaret ;
    :ml_task :tabular_classification ;
    :parameter_value :metric_pycaret_tabular_classification .
:tabular_regression_pycaret a :Configuration_item ;
    skos:prefLabel "tabular regression PyCaret" ;
    :category :task_configuration ;
    :automl_solution :pycaret ;
    :ml_task :tabular_regression ;
    :parameter_value :metric_pycaret_tabular_regression .
:time_series_forecasting__pycaret a :Configuration_item ;
    skos:prefLabel "time series forecasting  PyCaret" ;
    :category :task_configuration ;
    :automl_solution :pycaret ;
    :ml_task :time_series_forecasting ;
    :parameter_value :metric_pycaret_time_series_forecasting .
:ensemble_nbest a :Configuration_item ;
    skos:prefLabel "ensemble_nbest" ;
    :category :parameter ;
    :has_datatype :integer .
:ensemble_nbest_autosklearn a :Configuration_item ;
    skos:prefLabel "ensemble nbest autosklearn" ;
    :category :parameter ;
    :has_datatype :integer .
:ensemble_size a :Configuration_item ;
    skos:prefLabel "ensemble size" ;
    :category :parameter ;
    :has_datatype :integer .
:ensemble_size_autosklearn a :Configuration_item ;
    skos:prefLabel "ensemble size autosklearn" ;
    :category :parameter ;
    :has_datatype :integer .
:use_approach a :Configuration_item ;
    skos:prefLabel "use approach" ;
    :category :parameter .
:use_approach_autosklearn_classification a :Configuration_item ;
    skos:prefLabel "use approach Autosklearn classification" ;
    :category :parameter ;
    skos:broader :use_approach ;
    :has_datatype :list ;
    :parameter_value :adaboost , :decision_tree , :extra_tree , :gradient_boosting_tree , :k_nearest_neighbor , :linear_svm , :multilayer_perceptron , :random_forest , :gaussian_naives_bayes .
:use_approach_flaml_tabular_classification a :Configuration_item ;
    skos:prefLabel "use approach FLAML tabular classification" ;
    :category :parameter ;
    skos:broader :use_approach ;
    :has_datatype :list ;
    :parameter_value :gradient_boosting_tree , :random_forest , :extra_tree , :logistic_regression , :k_nearest_neighbor .
:use_approach_autosklearn_regression a :Configuration_item ;
    skos:prefLabel "use approach Autosklearn regression" ;
    :category :parameter ;
    skos:broader :use_approach ;
    :has_datatype :list ;
    :parameter_value :adaboost , :bayesian_linear_regression , :decision_tree , :extra_tree , :gaussian_process , :gradient_boosting_tree , :k_nearest_neighbor , :linear_svm , :multilayer_perceptron , :random_forest .
:use_approach_flaml_tabular_regression a :Configuration_item ;
    skos:prefLabel "use approach FLAML tabular regression" ;
    :category :parameter ;
    skos:broader :use_approach ;
    :has_datatype :list ;
    :parameter_value :gradient_boosting_tree , :random_forest , :extra_tree , :k_nearest_neighbor .
:use_approach_flaml_time_series_analysis a :Configuration_item ;
    skos:prefLabel "use approach FLAML time series analysis" ;
    :category :parameter ;
    skos:broader :use_approach ;
    :has_datatype :list ;
    :parameter_value :prophet , :auto_regressive_integrated_moving_average , :autoregressive_integrated_moving_average .
:use_approach_flaml_ranking a :Configuration_item ;
    skos:prefLabel "use approach FLAML ranking" ;
    :category :parameter ;
    skos:broader :use_approach ;
    :parameter_value :logistic_regression , :gradient_boosting_tree .
:use_approach_flaml_text_classification a :Configuration_item ;
    skos:prefLabel "use approach FLAML text classification" ;
    :category :parameter ;
    skos:broader :use_approach ;
    :has_datatype :list ;
    :parameter_value :transformer .
:use_approach_flaml_text_regression a :Configuration_item ;
    skos:prefLabel "use approach FLAML text regression" ;
    :category :parameter ;
    skos:broader :use_approach ;
    :has_datatype :list ;
    :parameter_value :transformer .
:use_approach_auto_pytorch_classification a :Configuration_item ;
    skos:prefLabel "use approach Auto-Pytorch classification" ;
    :category :parameter ;
    skos:broader :use_approach ;
    :has_datatype :list ;
    :parameter_value :multilayer_perceptron .
:use_approach_auto_pytorch_regression a :Configuration_item ;
    skos:prefLabel "use approach Auto-Pytorch regression" ;
    :category :parameter ;
    skos:broader :use_approach ;
    :has_datatype :list ;
    :parameter_value :multilayer_perceptron .
:use_approach_autocve_classification a :Configuration_item ;
    skos:prefLabel "use approach AutoCVE classification" ;
    :category :parameter ;
    skos:broader :use_approach ;
    :has_datatype :list ;
    :parameter_value :gradient_boosting_tree , :gaussian_naives_bayes , :decision_tree , :extra_tree , :random_forest , :k_nearest_neighbor , :linear_svm , :logistic_regression , :stochastic_gradient_descent , :multilayer_perceptron .
:use_approach_autogluon_classification a :Configuration_item ;
    skos:prefLabel "use approach AutoGluon classification" ;
    :category :parameter ;
    skos:broader :use_approach ;
    :has_datatype :list ;
    :parameter_value :gradient_boosting_tree , :multilayer_perceptron , :k_nearest_neighbor , :random_forest , :extra_tree , :logistic_regression .
:use_approach_autogluon_regression a :Configuration_item ;
    skos:prefLabel "use approach AutoGluon regression" ;
    :category :parameter ;
    skos:broader :use_approach ;
    :has_datatype :list ;
    :parameter_value :gradient_boosting_tree , :multilayer_perceptron , :k_nearest_neighbor , :ridge_regression , :random_forest , :extra_tree .
:use_approach_autogluon_image_classification a :Configuration_item ;
    skos:prefLabel "use approach AutoGluon image classification" ;
    :category :parameter ;
    skos:broader :use_approach ;
    :has_datatype :list ;
    :parameter_value :multilayer_perceptron .
:use_approach_autogluon_object_detection a :Configuration_item ;
    skos:prefLabel "use approach AutoGluon object detection" ;
    :category :parameter ;
    skos:broader :use_approach ;
    :has_datatype :list ;
    :parameter_value :multilayer_perceptron .
:use_approach_autogluon_text_classification a :Configuration_item ;
    skos:prefLabel "use approach AutoGluon text classification" ;
    :category :parameter ;
    skos:broader :use_approach ;
    :has_datatype :list ;
    :parameter_value :multilayer_perceptron .
:use_approach_autogluon_text_regression a :Configuration_item ;
    skos:prefLabel "use approach AutoGluon text regression" ;
    :category :parameter ;
    skos:broader :use_approach ;
    :has_datatype :list ;
    :parameter_value :multilayer_perceptron .
:use_approch_mcfly_time_series_classification a :Configuration_item ;
    skos:prefLabel "use approch mcfly time series classification" ;
    :category :parameter ;
    skos:broader :use_approach ;
    :has_datatype :list ;
    :parameter_value :inception_time , :residual_neural_network , :deep_convolutional_lstm , :convolutional_neural_network .
:use_approach_evalml_tabular_classification a :Configuration_item ;
    skos:prefLabel "use approach EvalML tabular classification" ;
    :category :parameter ;
    skos:broader :use_approach ;
    :has_datatype :list ;
    :parameter_value :catboost , :decision_tree , :extra_tree , :light_gradient_boosting_machine , :linear_regression , :random_forest , :xgboost .
:use_approach_evalml_tabular_regression a :Configuration_item ;
    skos:prefLabel "use approach EvalML tabular regression" ;
    :category :parameter ;
    skos:broader :use_approach ;
    :has_datatype :list ;
    :parameter_value :catboost , :decision_tree , :extra_tree , :light_gradient_boosting_machine , :linear_regression , :random_forest , :xgboost .
:use_approach_evalml_time_series_regression a :Configuration_item ;
    skos:prefLabel "use approach EvalML time series regression" ;
    :category :parameter ;
    skos:broader :use_approach ;
    :has_datatype :list ;
    :parameter_value :auto_regressive_integrated_moving_average , :catboost , :decision_tree , :exponential_smoothing , :extra_tree , :k_nearest_neighbor , :linear_regression , :random_forest , :xgboost .
:use_approach_evalml_time_series_classification a :Configuration_item ;
    skos:prefLabel "use approach EvalML time series classification" ;
    :category :parameter ;
    skos:broader :use_approach ;
    :has_datatype :list ;
    :parameter_value :caboost , :decision_tree , :extra_tree , :k_nearest_neighbor , :linear_regression , :random_forest , :xgboost .
:exclude_preprocessor a :Configuration_item ;
    skos:prefLabel "exclude preprocessor" ;
    :category :parameter .
:exclude_preprocessor_autosklearn a :Configuration_item ;
    skos:prefLabel "exclude preprocessor Autosklearn" ;
    :category :parameter ;
    skos:broader :exclude_preprocessor ;
    :has_datatype :list ;
    :parameter_value :kernel_principal_component_analysis , :radial_basis_function_kernel , :nystroem_kernel_approximation .
:configuration_via_metalearning a :Configuration_item ;
    skos:prefLabel "configuration via metalearning" ;
    :category :parameter ;
    :has_datatype :integer .
:metric a :Configuration_item ;
    skos:prefLabel "metric" ;
    :category :parameter .
:metric_autosklearn_classification a :Configuration_item ;
    skos:prefLabel "metric Autosklearn classification" ;
    :category :parameter ;
    skos:broader :metric ;
    :has_datatype :single_value ;
    :parameter_value :accuracy , :balanced_accuracy , :roc_auc , :average_precision , :log_loss , :precision_macro , :precision_micro , :precision_samples , :precision_weighted , :recall_macro , :recall_micro , :recall_samples , :recall_weighted , :f1_macro , :f1_micro , :f1_samples , :f1_weighted .
:metric_autokeras_tabular_classification a :Configuration_item ;
    skos:prefLabel "metric autokeras tabular classification" ;
    :category :parameter ;
    skos:broader :metric ;
    :has_datatype :single_value ;
    :parameter_value :accuracy , :binary_accuracy , :categorical_accuracy , :sparse_categorical_accuracy , :top_k_categorical_accuracy , :sparse_top_k_categorical_accuracy , :binary_cross_entropy , :categorical_cross_entropy , :poisson , :area_under_roc_curve , :precision , :recall , :true_positives , :true_negatives , :false_positives , :false_negatives , :hinge , :squared_hinge , :categorical_hinge .
:metric_flaml_tabular_classification a :Configuration_item ;
    skos:prefLabel "metric FLAML tabular classification" ;
    :category :parameter ;
    skos:broader :metric ;
    :has_datatype :single_value ;
    :parameter_value :accuracy , :receiver_operating_characteristic_curve , :receiver_operating_characteristic_curve_one_vs_rest , :log_loss , :receiver_operating_characteristic_curve_one_vs_one , :average_precision_score , :f_measure , :f_measure_micro , :f_measure_macro , :area_under_roc_curve_weighted .
:metric_autosklearn_regression a :Configuration_item ;
    skos:prefLabel "metric Autosklearn regression" ;
    :category :parameter ;
    skos:broader :metric ;
    :has_datatype :single_value ;
    :parameter_value :mean_absolute_error , :mean_squared_error , :root_mean_squared_error , :mean_squared_log_error , :median_absolute_error , :r2 .
:metric_autokeras_tabular_regression a :Configuration_item ;
    skos:prefLabel "metric autokeras tabular regression" ;
    :category :parameter ;
    skos:broader :metric ;
    :has_datatype :single_value ;
    :parameter_value :mean_squared_error , :root_mean_squared_error , :mean_absolute_error , :mean_absolute_percentage_error , :mean_squared_log_error , :cosine_similarity , :log_cosh_error .
:metric_flaml_tabular_regression a :Configuration_item ;
    skos:prefLabel "metric FLAML tabular regression" ;
    :category :parameter ;
    skos:broader :metric ;
    :has_datatype :single_value ;
    :parameter_value :coefficient_of_determination , :mean_squared_error , :rooted_mean_squared_error , :mean_absolute_error , :receiver_operating_characteristic_curve_one_vs_rest , :receiver_operating_characteristic_curve_one_vs_one , :receiver_operating_characteristic_curve , :mean_absolute_percentage_error , :r2 , :area_under_roc_curve_weighted .
:metric_flaml_text_classification a :Configuration_item ;
    skos:prefLabel "metric FLAML text classification" ;
    :category :parameter ;
    skos:broader :metric ;
    :has_datatype :single_value ;
    :parameter_value :accuracy , :receiver_operating_characteristic_curve , :receiver_operating_characteristic_curve_one_vs_rest , :log_loss , :receiver_operating_characteristic_curve_one_vs_one , :average_precision_score , :f_measure , :f_measure_micro , :f_measure_macro , :area_under_roc_curve_weighted .
:metric_flaml_text_regression a :Configuration_item ;
    skos:prefLabel "metric FLAML text regression" ;
    :category :parameter ;
    skos:broader :metric ;
    :has_datatype :single_value ;
    :parameter_value :coefficient_of_determination , :mean_squared_error , :rooted_mean_squared_error , :mean_absolute_error , :receiver_operating_characteristic_curve_one_vs_rest , :receiver_operating_characteristic_curve_one_vs_one , :receiver_operating_characteristic_curve , :mean_absolute_percentage_error , :r2 , :area_under_roc_curve_weighted .
:metric_flaml_ranking a :Configuration_item ;
    skos:prefLabel "metric FLAML ranking" ;
    :category :parameter ;
    skos:broader :metric ;
    :has_datatype :single_value ;
    :parameter_value :normalized_discounted_cumulative_gain .
:metric_flaml_time_series_analysis a :Configuration_item ;
    skos:prefLabel "metric FLAML time series analysis" ;
    :category :parameter ;
    skos:broader :metric ;
    :has_datatype :single_value ;
    :parameter_value :mean_absolute_percentage_error .
:metric_autogluon_tabular_regression a :Configuration_item ;
    skos:prefLabel "metric AutoGluon tabular regression" ;
    :category :parameter ;
    skos:broader :metric ;
    :has_datatype :single_value ;
    :parameter_value :rooted_mean_squared_error , :mean_squared_error , :mean_absolute_error , :median_absolute_error , :mean_absolute_percentage_error , :r2 .
:metric_autogluon_tabular_classification a :Configuration_item ;
    skos:prefLabel "metric AutoGluon tabular classification" ;
    :category :parameter ;
    skos:broader :metric ;
    :has_datatype :single_value ;
    :parameter_value :accuracy , :balanced_accuracy , :f_measure , :f_measure_macro , :f_measure_micro , :f_measure_weighted , :receiver_operating_characteristic_curve , :receiver_operating_characteristic_curve_one_vs_one , :average_precision_score , :precision , :precision_macro , :precision_micro , :precision_weighted , :recall , :recall_macro , :recall_micro , :recall_weighted , :log_loss , :pac_score .
:metric_autogluon_text_classification a :Configuration_item ;
    skos:prefLabel "metric AutoGluon text classification" ;
    :category :parameter ;
    skos:broader :metric ;
    :has_datatype :single_value ;
    :parameter_value :accuracy , :balanced_accuracy , :f_measure , :f_measure_macro , :f_measure_micro , :f_measure_weighted , :receiver_operating_characteristic_curve , :receiver_operating_characteristic_curve_one_vs_one , :average_precision_score , :precision , :precision_macro , :precision_micro , :precision_weighted , :recall , :recall_macro , :recall_micro , :recall_weighted , :log_loss , :pac_score .
:metric_autogluon_text_regression a :Configuration_item ;
    skos:prefLabel "metric AutoGluon text regression" ;
    :category :parameter ;
    skos:broader :metric ;
    :has_datatype :single_value ;
    :parameter_value :rooted_mean_squared_error , :mean_squared_error , :mean_absolute_error , :median_absolute_error , :r2 , :spearman_rank_correlation_coefficient , :pearson_correlation_coefficient .
:metric_autogluon_image_classification a :Configuration_item ;
    skos:prefLabel "metric AutoGluon image classification" ;
    :category :parameter ;
    skos:broader :metric ;
    :has_datatype :single_value ;
    :parameter_value :accuracy .
:metric_autogluon_time_series_forecasting a :Configuration_item ;
    skos:prefLabel "metric AutoGluon time series forecasting" ;
    :category :parameter ;
    skos:broader :metric ;
    :parameter_value :mean_absolute_percentage_error , :symmetric_mean_absolute_percentage_error , :mean_absolute_scaled_error , :mean_squared_error , :rooted_mean_squared_error .
:metric_auto_pytorch_classification a :Configuration_item ;
    skos:prefLabel "metric Auto Pytorch classification" ;
    :category :parameter ;
    skos:broader :metric ;
    :has_datatype :list ;
    :parameter_value :accuracy , :balanced_accuracy , :f_measure , :f_measure_macro , :f_measure_micro , :f_measure_weighted , :f_measure_samples , :receiver_operating_characteristic_curve , :average_precision_score , :log_loss , :precision , :precision_macro , :precision_micro , :precision_weighted , :precision_samples , :recall , :recall_macro , :recall_micro , :recall_weighted , :recall_samples .
:metric_auto_pytorch_regression a :Configuration_item ;
    skos:prefLabel "metric Auto Pytorch regression" ;
    :category :parameter ;
    skos:broader :metric ;
    :has_datatype :list ;
    :parameter_value :rooted_mean_squared_error , :mean_squared_error , :mean_absolute_error , :median_absolute_error , :coefficient_of_determination , :mean_squared_log_error .
:metric_autocve_classification a :Configuration_item ;
    skos:prefLabel "metric AutoCVE classification" ;
    :category :parameter ;
    skos:broader :metric ;
    :has_datatype :single_value ;
    :parameter_value :accuracy .
:metric_mcfly_time_series_classification a :Configuration_item ;
    skos:prefLabel "metric mcfly time series classification" ;
    :category :parameter ;
    skos:broader :metric ;
    :has_datatype :list ;
    :parameter_value :accuracy , :balanced_accuracy , :f_measure , :f_measure_macro , :f_measure_micro , :f_measure_weighted , :f_measure_samples , :receiver_operating_characteristic_curve , :average_precision_score , :log_loss , :precision , :precision_macro , :precision_micro , :precision_weighted , :precision_samples , :recall , :recall_macro , :recall_micro , :recall_weighted , :recall_samples .
:metric_autokeras_image_classification a :Configuration_item ;
    skos:prefLabel "metric AutoKeras image classification" ;
    :category :parameter ;
    skos:broader :metric ;
    :has_datatype :single_value ;
    :parameter_value :accuracy , :binary_accuracy , :categorical_accuracy , :sparse_categorical_accuracy , :top_k_categorical_accuracy , :sparse_top_k_categorical_accuracy , :binary_cross_entropy , :categorical_cross_entropy , :poisson , :area_under_roc_curve , :precision , :recall , :true_positives , :true_negatives , :false_positives , :false_negatives , :hinge , :squared_hinge , :categorical_hinge .
:metric_autokeras_text_classification a :Configuration_item ;
    skos:prefLabel "metric AutoKeras text classification" ;
    :category :parameter ;
    skos:broader :metric ;
    :has_datatype :single_value ;
    :parameter_value :accuracy , :binary_accuracy , :categorical_accuracy , :sparse_categorical_accuracy , :top_k_categorical_accuracy , :sparse_top_k_categorical_accuracy , :binary_cross_entropy , :categorical_cross_entropy , :poisson , :area_under_roc_curve , :precision , :recall , :true_positives , :true_negatives , :false_positives , :false_negatives , :hinge , :squared_hinge , :categorical_hinge .
:metric_autokeras_image_regression a :Configuration_item ;
    skos:prefLabel "metric AutoKeras image regression" ;
    :category :parameter ;
    skos:broader :metric ;
    :has_datatype :single_value ;
    :parameter_value :mean_squared_error , :root_mean_squared_error , :mean_absolute_error , :mean_absolute_percentage_error , :mean_squared_log_error , :cosine_similarity , :log_cosh_error .
:metric_autokeras_text_regression a :Configuration_item ;
    skos:prefLabel "metric AutoKeras text regression" ;
    :category :parameter ;
    skos:broader :metric ;
    :has_datatype :single_value ;
    :parameter_value :mean_squared_error , :root_mean_squared_error , :mean_absolute_error , :mean_absolute_percentage_error , :mean_squared_log_error , :cosine_similarity , :log_cosh_error .
:metric_autokeras_time_series_forecasting a :Configuration_item ;
    skos:prefLabel "metric AutoKeras time series forecasting" ;
    :category :parameter ;
    skos:broader :metric ;
    :has_datatype :single_value ;
    :parameter_value :mean_squared_error , :root_mean_squared_error , :mean_absolute_error , :mean_absolute_percentage_error , :mean_squared_log_error , :cosine_similarity , :log_cosh_error .
:metric_evalml_tabular_classification a :Configuration_item ;
    skos:prefLabel "metric EvalML tabular classification" ;
    :category :parameter ;
    skos:broader :metric ;
    :has_datatype :single_value ;
    :parameter_value :accuracy , :balanced_accuracy , :f_measure , :f_measure_micro , :f_measure_macro , :f_measure_weighted , :precision , :precision_macro , :precision_micro , :precision_weighted , :recall , :recall_micro , :recall_macro , :recall_weighted , :area_under_roc_curve , :area_under_roc_curve_micro , :area_under_roc_curve_macro , :area_under_roc_curve_weighted , :gini , :log_loss , :matthews_correlation_coefficient .
:metric_evalml_tabular_regression a :Configuration_item ;
    skos:prefLabel "metric EvalML tabular regression" ;
    :category :parameter ;
    skos:broader :metric ;
    :has_datatype :single_value ;
    :parameter_value :rooted_mean_squared_error , :mean_squared_log_error , :rooted_mean_squared_log_error , :r2 , :mean_absolute_error , :mean_squared_error , :median_absolute_error , :max_error , :explained_variance .
:metric_evalml_text_classification a :Configuration_item ;
    skos:prefLabel "metric EvalML text classification" ;
    :category :parameter ;
    skos:broader :metric ;
    :has_datatype :single_value ;
    :parameter_value :accuracy , :balanced_accuracy , :f_measure , :f_measure_micro , :f_measure_macro , :f_measure_weighted , :precision , :precision_macro , :precision_micro , :precision_weighted , :recall , :recall_micro , :recall_macro , :recall_weighted , :area_under_roc_curve , :area_under_roc_curve_micro , :area_under_roc_curve_macro , :area_under_roc_curve_weighted , :gini , :log_loss , :matthews_correlation_coefficient .
:metric_evalml_text_regression a :Configuration_item ;
    skos:prefLabel "metric EvalML text regression" ;
    :category :parameter ;
    skos:broader :metric ;
    :has_datatype :single_value ;
    :parameter_value :rooted_mean_squared_error , :mean_squared_log_error , :rooted_mean_squared_log_error , :r2 , :mean_absolute_error , :mean_squared_error , :median_absolute_error , :max_error , :explained_variance .
:metric_evalml_time_series_regression a :Configuration_item ;
    skos:prefLabel "metric EvalML time series regression" ;
    :category :parameter ;
    skos:broader :metric ;
    :has_datatype :single_value ;
    :parameter_value :mean_absolute_percentage_error .
:metric_mljar_tabular_classification a :Configuration_item ;
    skos:prefLabel "metric MLJAR tabular classification" ;
    :category :parameter ;
    skos:broader :metric ;
    :has_datatype :single_value ;
    :parameter_value :log_loss , :area_under_roc_curve , :f_measure , :accuracy , :precision , :recall , :matthews_correlation_coefficient .
:metric_mljar_tabular_regression a :Configuration_item ;
    skos:prefLabel "metric MLJAR tabular regression" ;
    :category :parameter ;
    skos:broader :metric ;
    :has_datatype :single_value ;
    :parameter_value :mean_absolute_error , :mean_squared_error , :rooted_mean_squared_error , :r2 , :mean_absolute_percentage_error .
:metric_pycaret_tabular_classification a :Configuration_item ;
    skos:prefLabel "metric PyCaret tabular classification" ;
    :category :parameter ;
    skos:broader :metric ;
    :has_datatype :single_value ;
    :parameter_value :accuracy , :area_under_roc_curve , :recall , :precision , :f_measure , :cohens_kappa , :matthews_correlation_coefficient .
:metric_pycaret_tabular_regression a :Configuration_item ;
    skos:prefLabel "metric PyCaret tabular regression" ;
    :category :parameter ;
    skos:broader :metric ;
    :has_datatype :single_value ;
    :parameter_value :mean_absolute_error , :mean_squared_error , :rooted_mean_squared_error , :r2 , :rooted_mean_squared_log_error , :mean_absolute_percentage_error .
:metric_pycaret_time_series_forecasting a :Configuration_item ;
    skos:prefLabel "metric PyCaret time series forecasting" ;
    :category :parameter ;
    skos:broader :metric ;
    :has_datatype :single_value ;
    :parameter_value :mean_absolute_scaled_error , :rooted_mean_squared_scaled_error , :symmetric_mean_absolute_percentage_error , :coverage , :mean_absolute_error , :rooted_mean_squared_error , :mean_absolute_percentage_error , :r2 .
:time_limit a :Configuration_item ;
    skos:prefLabel "time limit" ;
    :category :parameter ;
    :has_datatype :integer .
:time_limit_autosklearn a :Configuration_item ;
    skos:prefLabel "time limit autosklearn" ;
    :category :parameter ;
    :has_datatype :integer .
:time_limit_per_run a :Configuration_item ;
    skos:prefLabel "time limit per run" ;
    :category :parameter ;
    :has_datatype :integer .
:time_limit_per_run_autosklearn a :Configuration_item ;
    skos:prefLabel "time limit per run autosklearn" ;
    :category :parameter ;
    :has_datatype :integer .
:max_model_size a :Configuration_item ;
    skos:prefLabel "max_model_size" ;
    :category :parameter ;
    :has_datatype :integer .
:max_model_size_autokeras a :Configuration_item ;
    skos:prefLabel "max_model_size_autokeras" ;
    :category :parameter ;
    :has_datatype :integer .
:epochs a :Configuration_item ;
    skos:prefLabel "epochs" ;
    :category :parameter ;
    :has_datatype :integer .
:max_trials a :Configuration_item ;
    skos:prefLabel "max_trials" ;
    :category :parameter ;
    :has_datatype :integer .
:max_trials_autokeras a :Configuration_item ;
    skos:prefLabel "max_trials_autokeras" ;
    :category :parameter ;
    skos:broader :max_trials ;
    :has_datatype :integer .
:tuner a :Configuration_item ;
    skos:prefLabel "tuner" ;
    :category :parameter ;
    :has_datatype :single_value .
:tuner_autokeras_tabular_regression a :Configuration_item ;
    skos:prefLabel "tuner autokeras tabular regression" ;
    :category :parameter ;
    skos:broader :tuner ;
    :has_datatype :single_value ;
    :parameter_value :greedy , :bayesian , :random , :hyperband .
:tuner_autokeras_tabular_classification a :Configuration_item ;
    skos:prefLabel "tuner autokeras tabular classification" ;
    :category :parameter ;
    skos:broader :tuner ;
    :has_datatype :single_value ;
    :parameter_value :greedy , :bayesian , :random , :hyperband .
:tuner_autokeras_image_regression a :Configuration_item ;
    skos:prefLabel "tuner autokeras image regression" ;
    :category :parameter ;
    skos:broader :tuner ;
    :has_datatype :single_value ;
    :parameter_value :greedy , :bayesian , :random , :hyperband .
:tuner_autokeras_image_classification a :Configuration_item ;
    skos:prefLabel "tuner autokeras image classification" ;
    :category :parameter ;
    skos:broader :tuner ;
    :has_datatype :single_value ;
    :parameter_value :greedy , :bayesian , :random , :hyperband .
:tuner_autokeras_text_regression a :Configuration_item ;
    skos:prefLabel "tuner autokeras text regression" ;
    :category :parameter ;
    skos:broader :tuner ;
    :has_datatype :single_value ;
    :parameter_value :greedy , :bayesian , :random , :hyperband .
:tuner_autokeras_text_classification a :Configuration_item ;
    skos:prefLabel "tuner autokeras text classification" ;
    :category :parameter ;
    skos:broader :tuner ;
    :has_datatype :single_value ;
    :parameter_value :greedy , :bayesian , :random , :hyperband .
:tuner_autokeras_time_series_forecasting a :Configuration_item ;
    skos:prefLabel "tuner autokeras time series forecasting" ;
    :category :parameter ;
    skos:broader :tuner ;
    :has_datatype :single_value ;
    :parameter_value :greedy , :bayesian , :random , :hyperband .
:tuner_class_evalml a :Configuration_item ;
    skos:prefLabel "tuner class evalml" ;
    :category :parameter ;
    skos:broader :tuner ;
    :has_datatype :single_value ;
    :parameter_value :random , :grid_search , :skopt .
:loss a :Configuration_item ;
    skos:prefLabel "loss" ;
    :category :parameter .
:loss_autokeras_tabular_regression a :Configuration_item ;
    skos:prefLabel "loss autokeras tabular regression" ;
    :category :parameter ;
    skos:broader :loss ;
    :has_datatype :single_value ;
    :parameter_value :mean_squared_error .
:loss_autokeras_tabular_classification a :Configuration_item ;
    skos:prefLabel "loss autokeras tabular classification" ;
    :category :parameter ;
    skos:broader :loss ;
    :has_datatype :single_value ;
    :parameter_value :binary_cross_entropy , :categorical_cross_entropy .
:loss_autokeras_image_regression a :Configuration_item ;
    skos:prefLabel "loss autokeras image regression" ;
    :category :parameter ;
    skos:broader :loss ;
    :has_datatype :single_value ;
    :parameter_value :mean_squared_error .
:loss_autokeras_image_classification a :Configuration_item ;
    skos:prefLabel "loss autokeras image classification" ;
    :category :parameter ;
    skos:broader :loss ;
    :has_datatype :single_value ;
    :parameter_value :binary_cross_entropy , :categorical_cross_entropy .
:loss_autokeras_text_regression a :Configuration_item ;
    skos:prefLabel "loss autokeras text regression" ;
    :category :parameter ;
    skos:broader :loss ;
    :has_datatype :single_value ;
    :parameter_value :mean_squared_error .
:loss_autokeras_text_classification a :Configuration_item ;
    skos:prefLabel "loss autokeras text classification" ;
    :category :parameter ;
    skos:broader :loss ;
    :has_datatype :single_value ;
    :parameter_value :binary_cross_entropy , :categorical_cross_entropy .
:loss_autokeras_time_series_forecasting a :Configuration_item ;
    skos:prefLabel "loss autokeras time series forecasting" ;
    :category :parameter ;
    skos:broader :loss ;
    :has_datatype :single_value ;
    :parameter_value :mean_squared_error .
:loss_mcfly_time_series_classification a :Configuration_item ;
    skos:prefLabel "loss mcfly time series classification" ;
    :category :parameter ;
    skos:broader :loss ;
    :has_datatype :single_value ;
    :parameter_value :categorical_cross_entropy .


# Sheet34
